@prefix dc: <http://purl.org/dc/elements/1.1/> .
@prefix dcat: <http://www.w3.org/ns/dcat#> .
@prefix dct: <http://purl.org/dc/terms/> .
@prefix euvoc: <http://publications.europa.eu/ontology/euvoc#> .
@prefix foaf: <http://xmlns.com/foaf/0.1/> .
@prefix ontolidar: <http://vocab.ieawindtask32.org/wind-lidar-ontology/> .
@prefix org: <http://www.w3.org/ns/org#> .
@prefix owl: <http://www.w3.org/2002/07/owl#> .
@prefix pav: <http://purl.org/pav/> .
@prefix prov: <http://www.w3.org/ns/prov#> .
@prefix qb: <http://purl.org/linked-data/cube#> .
@prefix rdf: <http://www.w3.org/1999/02/22-rdf-syntax-ns#> .
@prefix rdfs: <http://www.w3.org/2000/01/rdf-schema#> .
@prefix schema: <http://schema.org/> .
@prefix sh: <http://www.w3.org/ns/shacl#> .
@prefix skos: <http://www.w3.org/2004/02/skos/core#> .
@prefix skosmos: <http://purl.org/net/skosmos#> .
@prefix skosthes: <http://purl.org/iso25964/skos-thes#> .
@prefix skosxl: <http://www.w3.org/2008/05/skos-xl#> .
@prefix xsd: <http://www.w3.org/2001/XMLSchema#> .

<http://vocab.ieawindtask32.org/wind-lidar-ontology/> a skos:ConceptScheme;
  dct:creator <http://orcid.org/0000-0002-9381-9693>, <https://orcid.org/0000-0001-9698-5083>,
    <https://orcid.org/0000-0003-1318-9677>;
  dct:description "Ontological representation of wind lidar supporting development of modular tools and processes for wind lidars."@en,
    "Ontologische Darstellung von Wind-Lidar zur Unterstützung der Entwicklung von modularen Werkzeugen und Prozessen für Wind-Lidar."@cn,
    "Ontologische Darstellung von Wind-Lidar zur Unterstützung der Entwicklung von modularen Werkzeugen und Prozessen für Wind-Lidar."@de,
    "Ontologische Darstellung von Wind-Lidar zur Unterstützung der Entwicklung von modularen Werkzeugen und Prozessen für Wind-Lidar."@es;
  dct:title "IEA Wind Task 32 Wind Lidar Ontologie"@cn, "IEA Wind Task 32 Wind Lidar Ontologie"@de,
    "IEA Wind Task 32 Wind Lidar Ontologie"@es, "IEA Wind Task 32 Wind Lidar Ontology"@en;
  pav:createdOn "2020-11-06T00:00:00+01:00"@en;
  pav:lastUpdatedOn "2021-01-13T00:00:00+01:00"@en;
  pav:version "0.1"@en;
  skos:editorialNote "This ontology is produced and maintained by IEA Wind Task 32."@en;
  skos:hasTopConcept ontolidar:DataCommunication, ontolidar:DataFormats, ontolidar:DataProcessing,
    ontolidar:Design, ontolidar:Devices, ontolidar:Installation, ontolidar:Instances,
    ontolidar:MeasurementPrinciples, ontolidar:MeasurementSetup, ontolidar:Parameters,
    ontolidar:UseCase;
  skos:historyNote "Suggestions for additions or changes should be made through the glossary repository at https://github.com/IEA-Wind-Task-32/wind-lidar-glossary."@en;
  skos:prefLabel "IEA Wind Task 32 Wind Lidar Ontology"@en .

ontolidar:Units a rdf:Property;
  rdfs:label "units"@en;
  skos:definition "A unit for parameter or variable being defined."@en, "Unidades de medida para un parámetro o varible."@es,
    "Unità di misura per una quantità fisica o un parametro"@it, "参数、变量等物理量的单位。"@cn;
  skos:prefLabel "Unidades"@es, "Unità"@it, "units"@en, "单位"@cn .

ontolidar:VelocityAzimuthDisplay a skos:Concept;
  skos:altLabel "VAD"@en;
  skos:broader ontolidar:WindfieldReconstruction;
  skos:definition "Un particolare metodo di analisi dati di un lidar a geometria conica. Data una scansione completa del cono ad una specifica altezza, i punti di misurazione contigui l'uno all'altro nello spazio vengono combinati secondo metodi statistici di interpolazione per ricostruire la velocità del vento."@it,
    "VAD es un método de análisis de datos provenientes de un escaneo de geometría cónica en el que varios puntos azimutales estrechamente espaciados son muestreados por el lidar. Dichos datos se utilizan para estimar la velocidad del viento a una determinada altura utilizando métodos de ajuste estadísticos."@es,
    "VAD is a method of analyzing data from a complete conical scan whereby many closely spaced azimuthal points may be sampled by the lidar, and the data are used to estimate the wind speed at each height using a statistical fitting method."@en,
    "VAD是一种测风激光雷达的测量方法，通过倒圆锥形的扫描方式，雷达可以对许多间隔很近的方位角点进行采样，然后使用统计拟合方法将数据用于推算每个高度的风速。"@cn;
  skos:editorialNote "El método VAD se describe en Lhermitte (1996) y en Browning and Wexler (1968)"@es,
    "Il metodo VAD è descritto in Lhermitte (1966) e Bowning e Wexler (1968)."@it, "The VAD method is described in Lhermitte (1966) and Browning and Wexler (1968)."@en;
  skos:inScheme <http://vocab.ieawindtask32.org/wind-lidar-ontology/>;
  skos:prefLabel "Campionamento di velocità in azimut"@it, "Geschwindigkeits-Azimut-Anzeige"@de,
    "Muestreo de velocidad en azimut"@es, "VAD测量法"@cn, "Velocity azimuth display"@en .

ontolidar:UseCase a skos:Concept;
  skos:definition "Formas en las que el lidar de viento puede ser utilizado. Combinación de tres elementos: 1. Requisitos de datos orientados a los resultados (en contraposición a los requisitos orientados a las restricciones, véase sensor de primera generación / mediciones de primera generación); 2. Método de medición seleccionado para cumplirlos; 3. Las condiciones de operación que determinan el rendimiento del método con respecto a la precisión del mismo."@es,
    "Tipici esempi di utilizzo di un wind lidar."@it, "Typical uses of a wind lidar."@en,
    "测风激光雷达的常见用法"@cn;
  skos:inScheme <http://vocab.ieawindtask32.org/wind-lidar-ontology/>;
  skos:narrower ontolidar:AdditionalSensor, ontolidar:MetmastPerformanceVerification,
    ontolidar:PerformanceVerification, ontolidar:TurbineCertification, ontolidar:WindCharacterisation,
    ontolidar:WindPlantControl, ontolidar:WindTunnelMeasurements, ontolidar:WindTurbineControl,
    ontolidar:YawAlignment;
  skos:prefLabel "Anwendungsfall"@de, "Casi di uso"@it, "Caso de uso"@es, "Use case"@en,
    "应用场景"@cn;
  skos:topConceptOf <http://vocab.ieawindtask32.org/wind-lidar-ontology/> .

ontolidar:AdditionalSensor a skos:Concept;
  skos:broader ontolidar:UseCase;
  skos:definition "Anemómetros y veleta montados sobre torre meteorológica."@es, "Lidar based measurement in addition to standard anemometry for a turbine/wind farm."@en,
    "Misurazioni lidar effettuate in aggiunta a quelle da anemometri tradizionali solitamente presenti su turbine e in parchi eolici."@it,
    "除用传统标准的风速仪测量外，对风力发电机组/风电场进行基于激光雷达的测量。"@cn;
  skos:inScheme <http://vocab.ieawindtask32.org/wind-lidar-ontology/>;
  skos:prefLabel "Additional sensor"@en, "Sensor adicional"@es, "Sensore aggiuntivo"@it,
    "Zusätzlicher Sensor"@de, "额外的传感器"@cn .

ontolidar:WindCharacterisation a skos:Concept;
  skos:broader ontolidar:UseCase;
  skos:definition "Lidar based measurement to identify the specific features of a local wind field."@en,
    "Medida lidar utilizada para identificar características locales del viento."@es,
    "Misurazioni lidar volte a definire le proprietà locali del vento."@it, "基于激光雷达的测量，确定测量区域内风的流场特征"@cn;
  skos:inScheme <http://vocab.ieawindtask32.org/wind-lidar-ontology/>;
  skos:narrower ontolidar:IecStandard61400121;
  skos:prefLabel "Caracterización de las propiedades del viento"@es, "Charakterisierung des Windes"@de,
    "Identificazione delle proprietà del vento"@it, "Wind characterisation"@en, "风的特性"@cn .

ontolidar:IecStandard61400121 a skos:Concept;
  skos:broader ontolidar:WindCharacterisation;
  skos:definition "Directrices internacionales para la medición del rendimiento energético de las turbinas eólicas productoras de electricidad."@es,
    "International guidelines for Power performance measurements of electricity producing wind turbines."@en,
    "Standard interanzionali di riferimento per turbine eoliche, strumenti eolici e strumentazioni di misurazione del vento"@it,
    "风力发电机组功率特性测试国际标准"@cn;
  skos:inScheme <http://vocab.ieawindtask32.org/wind-lidar-ontology/>;
  skos:prefLabel "IEC Standard 61400-12-1"@en, "IEC-Norm 61400-12-1"@de, "IEC标准61400-12-1"@cn,
    "Norma IEC 61400-12-1"@es, "Standard IEC 61400-12-1"@it .

ontolidar:TurbineCertification a skos:Concept;
  skos:broader ontolidar:UseCase;
  skos:definition "Proceso mediante el que se definen los niveles de garantía de calidad y tipo de elemento para generadores eólicos. Es un requerimiento para la comercialización de turbinas eólicas."@es,
    "Process of definition of the levels of quality warranty and object class for wind turbine generators. It is required for turbines' commercialization."@en,
    "Processo di definizione dei livelli di garanzia e classe di operatività per generatori eolici. E' necessario per la commercializzazione delle turbine."@it,
    "旨在验证风力发电机的设计、测试和制造符合规定的风力等级，并符合国际认证标准以及所有其他适用的标准和法规要求，是风力发电机组商业化的前提。"@cn;
  skos:inScheme <http://vocab.ieawindtask32.org/wind-lidar-ontology/>;
  skos:prefLabel "Certificación de la turbina eólica"@es, "Certificazione per turbine eoliche"@it,
    "Turbine certification"@en, "Zertifizierung von Turbinen"@de, "风力发电机组认证"@cn .

ontolidar:PerformanceVerification a skos:Concept;
  skos:broader ontolidar:UseCase;
  skos:definition "Proceso mediante el que se verifica el rendimiento de la turbina eólica en cuanto a la producción de potencia, normalmente en función de las garantías emitidas por el fabricante."@es,
    "Process of verification of turbines' power production performances, typically against the warranties issued by the turbine manufacturer."@en,
    "Processo di verifica delle prestazioni di produzione delle turbine. Il riferimento sono le garanzie rilasciate dal costruttore delle turbine."@it,
    "测试风力发电机组性能（功率特性）的过程，通常是为了验证风电机组的实际运行性能与制造商设定性能之间的差异"@cn;
  skos:inScheme <http://vocab.ieawindtask32.org/wind-lidar-ontology/>;
  skos:narrower ontolidar:IecStandard61400502, ontolidar:IecStandard61400503, ontolidar:Task32RecommendedPractices;
  skos:prefLabel "Leistungsüberprüfung"@de, "Performance verification"@en, "Verifica delle performances"@it,
    "Verificación del rendimiento"@es, "性能测试"@cn .

ontolidar:IecStandard61400502 a skos:Concept;
  skos:broader ontolidar:PerformanceVerification;
  skos:definition "Estándares de medición del rendimiento en la generación de potencia de una turbina eólica que están basados en las mediciones de lidares montados en tierra."@es,
    "Standard interanzionali di riferimento per misurazioni della prestazione delle turbine basata su lidar montati a terra."@it,
    "Wind turbine's power performance measurement standards based on ground based lidars."@en,
    "基于地面式测风激光雷达的风力发电机组功率特性测试国际标准"@cn;
  skos:inScheme <http://vocab.ieawindtask32.org/wind-lidar-ontology/>;
  skos:prefLabel "IEC Standard 61400-50-2"@en, "IEC Standard 61400-50-2"@it, "IEC-Norm 61400-50-2"@de,
    "IEC标准61400-50-2"@cn, "Norma IEC 61400-50-2"@es .

ontolidar:IecStandard61400503 a skos:Concept;
  skos:broader ontolidar:PerformanceVerification;
  skos:definition "Estándares de medición del rendimiento en la generación de potencia de una turbina eólica que están basados en las mediciones de lidares montados en góndola."@es,
    "Standard interanzionali di riferimento per misurazioni della prestazione delle turbine basata su lidar montati sulla turbina."@it,
    "Wind turbine's power performance measurement standards based on nacelle mounted lidars."@en,
    "基于机舱式测风激光雷达的风力发电机组功率特性测试国际标准"@cn;
  skos:inScheme <http://vocab.ieawindtask32.org/wind-lidar-ontology/>;
  skos:prefLabel "IEC Standard 61400-50-3"@en, "IEC Standard 61400-50-3"@it, "IEC-Norm 61400-50-3"@de,
    "IEC标准61400-50-3"@cn, "Norma IEC 61400-50-3"@es .

ontolidar:Task32RecommendedPractices a skos:Concept;
  skos:broader ontolidar:PerformanceVerification;
  skos:definition "IEA Task32对海上风力发电机组功率特性的建议做法--测试/复杂的地形"@cn, "Raccomandazioni sulle procedure per misurazioni della perfomance in produzione offshore ed in terreni complessi."@it,
    "Recomendaciones prácticas propuestas por Task32 para la medición del rendimiento en la producción de potencia de una turbina eólica offshore o en terreno complejo."@es,
    "Task 32 Reccomended practices for Offshore Power Performance - Testing/Complex terrain."@en;
  skos:inScheme <http://vocab.ieawindtask32.org/wind-lidar-ontology/>;
  skos:prefLabel "Raccomandazioni della IEA Task32"@it, "Recomendaciones Task32"@es,
    "Task32 Empfohlene Vorgehensweisen"@de, "Task32 Recommended practices"@en, "Task32 推荐做法"@cn .

ontolidar:WindTurbineControl a skos:Concept;
  skos:broader ontolidar:UseCase;
  skos:definition "Lidar based techniques to control a wind turbine generator."@en,
    "Tecniche di controllo di una turbina eolica basate su misurazioni da lidar."@it,
    "Técnicas de control de una turbina eólica basadas en la información extraída de un lidar."@es,
    "基于激光雷达来控制风力发电机组的技术。"@cn;
  skos:inScheme <http://vocab.ieawindtask32.org/wind-lidar-ontology/>;
  skos:narrower <http://vocab.ieawindtask32.org/wind-lidar-ontology/Turbulence(ControlInPresenceOf)>,
    <http://vocab.ieawindtask32.org/wind-lidar-ontology/Wakes(ControlOf)>;
  skos:prefLabel "Controllo dei generatori eolici"@it, "Steuerung von Windkraftanlagen"@de,
    "Técnicas de control de la turbina eólica"@es, "Wind turbine control"@en, "风力发电机组控制"@cn .

<http://vocab.ieawindtask32.org/wind-lidar-ontology/Turbulence(ControlInPresenceOf)>
  a skos:Concept;
  skos:broader ontolidar:WindTurbineControl;
  skos:definition "Lidar based techniques to control a wind turbine generator in presence of turbulence."@en,
    "Tecniche di controllo di una turbina eolica in presenza di forte turbolenza basate su misurazioni da lidar."@it,
    "Técnicas basadas en datos lidar para el control de una turbina eólica en presencia de turbulencia atmosférica."@es,
    "基于激光雷达在湍流情况下控制风力发电机组的技术。"@cn;
  skos:inScheme <http://vocab.ieawindtask32.org/wind-lidar-ontology/>;
  skos:prefLabel "Turbolenza (controllo in presenza di)"@it, "Turbulence (control in presence of)"@en,
    "Turbulencia"@es, "Turbulenz (Kontrolle in Gegenwart von)"@de, "湍流（存在时的控制）"@cn .

<http://vocab.ieawindtask32.org/wind-lidar-ontology/Wakes(ControlOf)> a skos:Concept;
  skos:broader ontolidar:WindTurbineControl;
  skos:definition "Lidar based techniques to control the wakes from turbines."@en, "Tecniche di controllo delle scie di una turbina eolica basate su misurazioni da lidar."@it,
    "Técnicas basadas en datos lidar para el control de estelas creadas por la turbina eólica."@es,
    "基于激光雷达来控制风力发电机组尾流的技术。"@cn;
  skos:inScheme <http://vocab.ieawindtask32.org/wind-lidar-ontology/>;
  skos:prefLabel "Estelas"@es, "Scie (controllo delle)"@it, "Wakes (Steuerung von)"@de,
    "Wakes (control of)"@en, "尾流（控制）"@cn .

ontolidar:WindPlantControl a skos:Concept;
  skos:broader ontolidar:UseCase;
  skos:definition "Estrategias basadas en información lidar para el control colectivo de turbinas eólicas en un mismo parque eólico."@es,
    "Lidar based strategies for collective control of wind generators in the same park."@en,
    "Tecniche di controllo collettivo di turbine eoliche nello stesso parco basate su misurazioni da lidar."@it,
    "基于激光雷达，对于同一个风电场内的风力发电机组进行集体控制的技术。"@cn;
  skos:inScheme <http://vocab.ieawindtask32.org/wind-lidar-ontology/>;
  skos:prefLabel "Control de parque eólico"@es, "Controllo del parco eolico"@it, "Steuerung von Windkraftanlagen"@de,
    "Wind plant control"@en, "风电场控制"@cn .

ontolidar:YawAlignment a skos:Concept;
  skos:broader ontolidar:UseCase;
  skos:definition "Alineamiento de la turbina eólica con la dirección del viento obtenido mediante datos lidar."@es,
    "Allineamento della navicella di una turbina con la direzione del vento basata su misurazioni da lidar."@it,
    "Lidar based alignment of the yaw of the turbine. Aimed at pointing the generator directly into the wind."@en,
    "基于激光雷达对风力发电机组的偏航角进行调整，旨在使机组对风更加准确。"@cn;
  skos:inScheme <http://vocab.ieawindtask32.org/wind-lidar-ontology/>;
  skos:prefLabel "Allineamento della turbina"@it, "Alneamiento de guiñada"@es, "Ausrichtung des Gierens"@de,
    "Yaw alignment"@en, "偏航校准"@cn .

ontolidar:MetmastPerformanceVerification a skos:Concept;
  skos:broader ontolidar:UseCase;
  skos:definition "Lidar based measurements to verify the quality of measurments from met mast instrumentations."@en,
    "Medidas lidar para veificar la calidad de medidas tomadas por sensores montados sobre una torre meteorológica."@es,
    "Misurazioni lidar volte a verificare la qualità delle misurazioni effettuate da anemometri posizionati su torri meteorologiche."@it,
    "基于激光雷达的测量，以验证测风塔上测风仪器的测量质量。"@cn;
  skos:inScheme <http://vocab.ieawindtask32.org/wind-lidar-ontology/>;
  skos:prefLabel "Metmast performance verification"@en, "Verifica delle torri anemometriche"@it,
    "Verificación del rendimiento de la torre meteorológica"@es, "Verifizierung der Metmast-Leistung"@de,
    "测风塔性能验证"@cn .

ontolidar:WindTunnelMeasurements a skos:Concept;
  skos:broader ontolidar:UseCase;
  skos:definition "Lidar based measurments in wind tunnels."@en, "Medidas lidar tomadas en un tunel de viento."@es,
    "Misurazioni lidar effettuate in gallerie del vento."@it, "风洞中基于激光雷达的测量"@cn;
  skos:inScheme <http://vocab.ieawindtask32.org/wind-lidar-ontology/>;
  skos:prefLabel "Medidas en túnel de viento"@es, "Misurazioni in galleria del vento"@it,
    "Wind tunnel measurements"@en, "Windkanal-Messungen"@de, "风洞测量"@cn .

ontolidar:VirtualMetMast a skos:Concept;
  skos:altLabel "Crossed RHI"@en;
  skos:broader ontolidar:MultiLidar;
  skos:definition "A series of wind measurements made at discrete vertical locations, mimicking a met mast. These can be implemented using many approaches including Crossed RHI (XRHI) and other dual- or triple-lidar measurement."@en,
    "Series de medición del viento localizadas en puntos concretos de la vertical, imitando un mástil meteorológico. Se pueden llevar a cabo utilizando muvhos enfoques, como RHI cruzado (XRHI) y otras mediciones utilizando dos o tres lidares conjuntamente."@es,
    "Una serie di misurazioni effettuate a varie altezze discrete da terra, in un modo del tutto simile alla distribuzione delle misurazioni dagli anemometri di una torre metereologica. Queste misurazioni possono essere effettuate utilizzando diversi approcci, inclusi il Crossed RHI (XRHI) ed altri sistemi di misurazione a due o tre sistemi laser."@it,
    "类似于测风塔，在竖直方向、离散的不同高度进行的测风。包括许多实现方法，如交叉 RHI (XRHI)方法，双雷达测量或三雷达测量等"@cn;
  skos:inScheme <http://vocab.ieawindtask32.org/wind-lidar-ontology/>;
  skos:prefLabel "Torre meteorologica virtuale"@it, "Torre meteorológica virtual"@es,
    "Virtual met mast"@en, "Virtueller Messmast"@de, "虚拟测风塔"@cn .

ontolidar:Design a skos:Concept;
  skos:definition "Descrizione delle componenti generali di un lidar e del raccordo fra di esse."@it,
    "Estructura de diseño genérico del lidar de viento. Componentes genéricos y conexión entre ellos."@es,
    "Wind lidar generic design structure."@en, "测风激光雷达通用设计结构"@cn;
  skos:editorialNote "Definición basada en el proyecto OpenLidar: https://github.com/e-WindLidar/OpenLidarModuleDefinitions"@es,
    "Definition based on the OpenLidar module definitions at https://github.com/e-WindLidar/OpenLidarModuleDefinitions"@en,
    "Definizione basata sulla definizione di modulo del progetto OpenLidar. Vedasi https://github.com/e-WindLidar/OpenLidarModuleDefinitions"@it;
  skos:inScheme <http://vocab.ieawindtask32.org/wind-lidar-ontology/>;
  skos:narrower ontolidar:ChassisModule, ontolidar:ControlModule, ontolidar:InterlocksModule,
    ontolidar:LocationDetection, ontolidar:MotionDetection, ontolidar:OpticsModule, ontolidar:PhotonicsModule,
    ontolidar:PowerModule, ontolidar:ScannerModule;
  skos:prefLabel "Design"@en, "Diseño"@es, "Entwurf"@de, "Struttura generale"@it, "设计"@cn;
  skos:topConceptOf <http://vocab.ieawindtask32.org/wind-lidar-ontology/> .

ontolidar:ChassisModule a skos:Concept;
  skos:broader ontolidar:Design;
  skos:definition "El módulo que representa el chásis representa las diversas soluciones de montaje del lidar, incluyendo (pero sin estar limitado a) montaje sobre góndola, torre meteorológica, sobre suelo, plataforma flotante o estructua móvil."@es,
    "Modulo di ancoraggio del sistema lidar per ognuna delle sue possibili applicazioni. Include, ma non si limita alle varie soluzioni di montaggio sulla navicella di una turbina, su una torre metereologica, a terra, su una piattaforma flottante o su una struttura mobile."@it,
    "Refers to the main lidar structure, designed to protect and house the different lidar components. Its design may vary depending on lidar mounting solutions, including, but not limited to, mounting on a nacelle, a meteorological tower, the ground, a floating platform or a mobile structure."@en,
    "激光雷达的主要结构，旨在保护和容纳不同的激光雷达组件。其设计可能因激光雷达安装解决方案而异，包括但不限于安装在机舱、气象塔、地面、浮动平台或其他移动结构上。"@cn;
  skos:editorialNote "Definición basada en el proyecto OpenLidar: https://github.com/e-WindLidar/OpenLidarModuleDefinitions"@es,
    "Definition based on the OpenLidar module definitions at https://github.com/e-WindLidar/OpenLidarModuleDefinitions"@en,
    "Definizione basata sulla definizione di modulo del progetto OpenLidar. Vedasi https://github.com/e-WindLidar/OpenLidarModuleDefinitions"@it;
  skos:inScheme <http://vocab.ieawindtask32.org/wind-lidar-ontology/>;
  skos:narrower ontolidar:EnvironmentalConditionsDetection;
  skos:prefLabel "Chassis module"@en, "Chassis-Modul"@de, "Módulo de chasis"@es, "Telaio"@it,
    "底盘模块"@cn .

ontolidar:LocationDetection a skos:Concept;
  skos:broader ontolidar:Design;
  skos:definition "Componentes y métodos asociados para obtener la posición exacta del lidar y, por tanto derivar correctamente las posiciones de los puntos de medición."@es,
    "Devices and associated methods to retrieve the exact position and orientation of the lidar, and thus the correct measurement points."@en,
    "Sistema per l'identificazione della posizione esatta e l'orientamento del lidar e, di conseguenza, della posizione dei punti di misurazione"@it,
    "读取激光雷达准确位置和朝向的设备和相关方法，从而保证可以获得准确的测量位置信息。"@cn;
  skos:inScheme <http://vocab.ieawindtask32.org/wind-lidar-ontology/>;
  skos:narrower ontolidar:Gps, ontolidar:Inclinometer;
  skos:prefLabel "Localización"@es, "Localizzazione"@it, "Location detection"@en, "Standort-Erkennung"@de,
    "位置检测"@cn .

ontolidar:Gps a skos:Concept;
  skos:broader ontolidar:LocationDetection;
  skos:definition "Global Positioning System that uniquely defines the position of the lidar."@en,
    "Sistema de posicionamiento global que define de forma única la posición del lidar."@es,
    "Sistema di posizionamento globale. Sistema di posizionamento del lidar."@it, "全球定位系统，可准确地描述激光雷达的位置。"@cn;
  skos:inScheme <http://vocab.ieawindtask32.org/wind-lidar-ontology/>;
  skos:prefLabel "GPS"@cn, "GPS"@de, "GPS"@en, "GPS"@es, "GPS"@it .

ontolidar:Inclinometer a skos:Concept;
  skos:broader ontolidar:LocationDetection;
  skos:definition "Lidar orientation system affixed to the bracket structure. In turn, the bracket structure is affixed to the ground or to another structure, like the nacelle. of Lidar orientation measurement system."@en,
    "Sistema de medida de la orientación del lidar."@es, "Sistema di misurazione dell'orientazione del lidar."@it,
    "贴在激光雷达支架结构上的定位系统，用于测量物体相对于重力方向的倾斜、仰角或俯角角度。而支架结构被固定在地面或其他结构上，如机舱。"@cn;
  skos:inScheme <http://vocab.ieawindtask32.org/wind-lidar-ontology/>;
  skos:prefLabel "Inclinometer"@en, "Inclinometro"@it, "Inclinómetros"@es, "Neigungsmesser"@de,
    "倾斜仪"@cn .

ontolidar:MotionDetection a skos:Concept;
  skos:broader ontolidar:Design;
  skos:definition "Sistema destinado a detectar y compensar el movimiento/vibraciones del lidar debido, por ejemplo, al movimiento ya sea de la góndola o de la boya para lidares marinos. Su resultado se utiliza en la etapa de procesamiento de datos del lidar para rectificar sus mediciones y compensar el movimiento de la plataforma."@es,
    "Sistema per la misurazione e la compensazione del moto del idar e delle sue vibrazioni. Questi movimenti possono esser dovuti al moto del supporto dove il lidar è montato - sia esso una navicella o una boa per i lidar marini. Le misurazioni di questo sistema sono usate per rettificare le misurazioni del vento."@it,
    "System meant to detect and compensate for the lidar motion/vibrations due to, e.g. nacelle or buoy motion in offshore mounted lidars. Its output is used in the lidar data processing stage to rectify its measurements and compensate for platform motion."@en,
    "该系统旨在检测和补偿由于机舱或浮标安装的激光雷达的运动/振动，例如机舱或浮标运动。它的输出被用于激光雷达数据处理阶段，以纠正其测量结果并补偿平台的运动。"@cn;
  skos:inScheme <http://vocab.ieawindtask32.org/wind-lidar-ontology/>;
  skos:narrower ontolidar:Accelerometer, ontolidar:Gyrometer;
  skos:prefLabel "Bewegungserkennung"@de, "Detección de movimiento"@es, "Motion detection"@en,
    "Sensore di moto"@it, "运动检测"@cn .

ontolidar:Accelerometer a skos:Concept;
  skos:broader ontolidar:MotionDetection;
  skos:definition "Sensor to measure the motion of the lidar with respect to the inertial local system. In combination with the gyrometer provides us with an array of information that helps us to either filter of correct the lidar data due to the motion of the lidar."@en,
    "Sensor utilizado para medir el movimiento del lidar con respecto al sistema local inercial. En combinación con el girómetro nos proporciona información que nos ayuda a filtrar o corregir los datos del lidar debido al movimiento del mismo."@es,
    "Sensori atti alla misurazione del moto del lidar rispetto al suo sistema inerziale locale. In combinazione con i dati dai giroscopi, supporta il filtraggio e la correzione delle misurazioni del vento."@it,
    "用于测量激光雷达相对于当地惯性系统运动的传感器。与陀螺仪结合，提供了一系列的信息，用于过滤或纠正受雷达设备运动影响而产生的激光雷达数据。"@cn;
  skos:inScheme <http://vocab.ieawindtask32.org/wind-lidar-ontology/>;
  skos:prefLabel "Accelerometer"@en, "Accelerometro"@it, "Acelerómetro"@es, "Beschleunigungsmesser"@de,
    "加速器"@cn .

ontolidar:Gyrometer a skos:Concept;
  skos:broader ontolidar:MotionDetection;
  skos:definition "Sensor used to determine the orientation of the lidar with respect to the local Earth's gravity vector, thus the orientation of the laser beam. In combination with the accelerometer provides us with an array of information that helps us to either filter of correct the lidar data due to the motion of the lidar."@en,
    "Sensor utilizado para determinar la orientación del lidar con respecto al vector de gravedad local de la Tierra, y por tanto la orientación del rayo láser. En combinación con el acelerómetro nos proporciona información que nos ayuda a filtrar o corregir los datos del lidar debido al movimiento del mismo."@es,
    "Sensori atti alla misurazione dell'orientazione del lidar rispetto al vettore di gravità terrestre locale.. In combinazione con i dati dagli accelerometri, supporta il filtraggio e la correzione delle misurazioni del vento."@it,
    "用于测量激光雷达相对于当地地球重力矢量方向的传感器，从而确定激光束的方向。与加速度计相结合，提供一系列的信息，用于过滤或纠正受雷达设备运动影响而产生的激光雷达数据。"@cn;
  skos:inScheme <http://vocab.ieawindtask32.org/wind-lidar-ontology/>;
  skos:prefLabel "Girometro"@it, "Girómetro"@es, "Gyrometer"@de, "Gyrometer"@en, "陀螺仪"@cn .

ontolidar:EnvironmentalConditionsDetection a skos:Concept;
  skos:broader ontolidar:ChassisModule;
  skos:definition "Condiciones meteorológicas en el punto de instalación del lidar."@es,
    "Condizioni metereologiche nel luogo di installazione del lidar."@it, "System to detect the meteorological conditions on the lidar spot."@en,
    "激光雷达所在位置的气象条件的检测系统。"@cn;
  skos:inScheme <http://vocab.ieawindtask32.org/wind-lidar-ontology/>;
  skos:narrower ontolidar:LocalMetstation;
  skos:prefLabel "Detección de condiciones medioambientales"@es, "Environmental conditions detection"@en,
    "Erkennung von Umgebungsbedingungen"@de, "Rilevamento delle condizioni ambientali"@it,
    "环境条件检测"@cn .

ontolidar:LocalMetstation a skos:Concept;
  skos:broader ontolidar:EnvironmentalConditionsDetection;
  skos:definition "Estación meteorológica local integrada en el chasis del lidar. Ofrece información sobre las condiciones atmosféricas en las que trabaja el lidar."@es,
    "Local meteorology station integrated in the lidar chassis module. Reports the meteorological conditions under which the lidar is working."@en,
    "Stazione meteo locale integrata nella scocca del lidar. Riporta le condizioni meteo in cui il lidar sta operando."@it,
    "集成在激光雷达底盘模块的本地气象站，用于记录或报告激光雷达工作时的气象条件。"@cn;
  skos:inScheme <http://vocab.ieawindtask32.org/wind-lidar-ontology/>;
  skos:prefLabel "Estación meteorológica local"@es, "Local MetStation"@en, "Lokale Messstation"@de,
    "Stazione meteorologica locale"@it, "本地气象站"@cn .

ontolidar:ControlModule a skos:Concept;
  skos:broader ontolidar:Design;
  skos:definition "El módulo de control representa la interfaz entre el controlador externo (humano o máquina) y el sistema lidar."@es,
    "Modulo di interfaccia fra l'utente di controllo esterno (umano per controllo manuale o un software per un controllo automatico) ed il sistema lidar."@it,
    "The control module is the interface between the external controller (human or machine) and the lidar system."@en,
    "控制模块是外部控制器（人或机器）和激光雷达系统之间的接口"@cn;
  skos:editorialNote "Definición basada en el proyecto OpenLidar: https://github.com/e-WindLidar/OpenLidarModuleDefinitions"@es,
    "Definition based on the OpenLidar module definitions at https://github.com/e-WindLidar/OpenLidarModuleDefinitions"@en,
    "Definizione basata sulla definizione di modulo del progetto OpenLidar. Vedasi https://github.com/e-WindLidar/OpenLidarModuleDefinitions"@it;
  skos:inScheme <http://vocab.ieawindtask32.org/wind-lidar-ontology/>;
  skos:narrower ontolidar:CommunicationsModule, ontolidar:SignalProcessingModule, ontolidar:StorageModule;
  skos:prefLabel "Componente di controllo"@it, "Control module"@en, "Módulo de control"@es,
    "Steuermodul"@de, "控制模块"@cn .

ontolidar:CommunicationsModule a skos:Concept;
  skos:broader ontolidar:ControlModule;
  skos:definition "Modulo (composto da parti hardware e software) che trasmette e riceve dati e comandi, da e per il sistema lidar."@it,
    "Sistema de dispositivos y software que transmite y recibe datos."@es, "The system of devices and software that transmit and receive data and commands to and from the lidar device."@en,
    "向激光雷达设备发送和接收数据和命令的设备和软件系统"@cn;
  skos:editorialNote "Definición basada en el proyecto OpenLidar:https://github.com/e-WindLidar/OpenLidarModuleDefinitionss"@es,
    "Definition based on the OpenLidar module definitions at https://github.com/e-WindLidar/OpenLidarModuleDefinitions"@en,
    "Definizione basata sulla definizione di modulo del progetto OpenLidar. Vedasi https://github.com/e-WindLidar/OpenLidarModuleDefinitions"@it;
  skos:inScheme <http://vocab.ieawindtask32.org/wind-lidar-ontology/>;
  skos:prefLabel "Communications module"@en, "Componente di comunicazione"@it, "Componentes de comunicación"@es,
    "Kommunikations-Modul"@de, "通讯模块"@cn .

ontolidar:SignalProcessingModule a skos:Concept;
  skos:broader ontolidar:ControlModule;
  skos:definition "El módulo de procesamiento de datos se utiliza para convertir los datos adquridos por el lidar en datos finales."@es,
    "Modulo utilizzato per convertire i dati acquisiti dal lidar nei dati finali richiesti."@it,
    "The signal processing module is used to convert the data acquired by the lidar into a data product."@en,
    "信号处理模块用于将激光雷达采集到的原始数据转化为（输出的）数据产品"@cn;
  skos:editorialNote "Definición basada en el proyecto OpenLidar:https://github.com/e-WindLidar/OpenLidarModuleDefinitionss"@es,
    "Definition based on the OpenLidar module definitions at https://github.com/e-WindLidar/OpenLidarModuleDefinitions"@en,
    "Definizione basata sulla definizione di modulo del progetto OpenLidar. Vedasi https://github.com/e-WindLidar/OpenLidarModuleDefinitions"@it;
  skos:inScheme <http://vocab.ieawindtask32.org/wind-lidar-ontology/>;
  skos:narrower ontolidar:AnalogToDigitalConverter, ontolidar:Filter, ontolidar:FrequencyAnalyser;
  skos:prefLabel "Componente di processamento dati"@it, "Modul zur Signalverarbeitung"@de,
    "Módulo de procesamiento de señal"@es, "Signal processing module"@en, "信号处理模块"@cn;
  skos:related ontolidar:DataProcessing .

ontolidar:AnalogToDigitalConverter a skos:Concept;
  skos:altLabel "ADC"@en;
  skos:broader ontolidar:SignalProcessingModule;
  skos:definition "Convertitore del segnale analogico del fotodetettore in segnale digitale per l'analizzatore di frequenza."@it,
    "Device that converts the analog signal from the photodetector into a digital signal to properly be analised by the frequency analyser."@en,
    "Dispositivo que convierte la señal analógica proveniente del fotodetector en una señal digital, con lo que puede ser analizada adecuadamente por el analizador de frecuencias."@es,
    "将光电探测器的模拟信号转换为数字信号的装置，以便由频率分析器进行合理地分析"@cn;
  skos:inScheme <http://vocab.ieawindtask32.org/wind-lidar-ontology/>;
  skos:narrower ontolidar:NumberOfBits;
  skos:prefLabel "Analog to digital converter"@en, "Analog-Digital-Wandler"@de, "Convertidor analógico-digital"@es,
    "Convertitore analogico-digitale"@it, "模拟数字转换器"@cn .

ontolidar:NumberOfBits a skos:Concept;
  skos:broader ontolidar:AnalogToDigitalConverter;
  skos:definition "Number of bits of the analog to digital converter."@en, "Numero di bit del convertitore analogico-digitale"@it,
    "Número de bits del convertidor analógico-digital."@es, "模拟数字转换器的比特数。"@cn;
  skos:editorialNote "Define la resolución del convertidos analógico-digital y representa el número de valores o \"niveles\" en que la señal puede ser cuantizada."@es,
    "Defines the resolution of the analog to digital converter, and represents the number of values or \"levels\" in which the signal can be quantised."@en,
    "Definisce la risoluzione del convertitore analogico-digitale e rappresenta il numero di valori (livelli) in cui il segnale viene separato"@it;
  skos:inScheme <http://vocab.ieawindtask32.org/wind-lidar-ontology/>;
  skos:prefLabel "Anzahl der Bits"@de, "Number of bits"@en, "Numero di bit"@it, "比特数"@cn .

ontolidar:Filter a skos:Concept;
  skos:broader ontolidar:SignalProcessingModule;
  skos:definition "Filtro pasa-baja."@es, "Filtro passa-basso."@it, "Low pass filter."@en,
    "低通滤波器。"@cn;
  skos:editorialNote "El ruido aleatorio de la señal debida al hardware y luz retrodispersada se filtra aplicando un umbral que define qué parte de la señal corresponde a información sobre las características del viento y qué parte es simplemente ruido de señal ."@es,
    "Segnala la presenza di rumore dall'hardware, da backscatter non legato al vento Tipicamente il filtro e' costituito da una semplice soglia sul livello di rumore."@it,
    "Signal random noise from hardware and unwanted backscattered light is whitenned and a threshold is applied to filter out undesired signal noise."@en;
  skos:inScheme <http://vocab.ieawindtask32.org/wind-lidar-ontology/>;
  skos:prefLabel "Filter"@de, "Filter"@en, "Filtro"@es, "Filtro"@it, "滤波器"@cn .

ontolidar:FrequencyAnalyser a skos:Concept;
  skos:broader ontolidar:SignalProcessingModule;
  skos:definition "Device that processes the signal from the analog-to-digital converter and calculates the Doppler spectra."@en,
    "Dispositivo que procesa la señal proveniente del convertidor analógico-digital y computa el espectro de frecuencias."@es,
    "Sistema che converte il segnale digitale in uscita dal convertitore analogico-digitale in spettri Doppler."@it,
    "处理来自模拟数字转换器的信号并生成多普勒光谱的设备。"@cn;
  skos:editorialNote "Once the analog signal is converted to a digital signal, a frequency analyser is used to determine its frequency spectra. This device yields the frequency spectrum of the dowmixed signal (original signal from the laser source + backscattered signal), therefore the Doppler frequency shift."@en,
    "Questo apparezzio produce lo spettro di potenza del segnale di battimento fra la sorgente laser originale ed il segnale di backscatter."@it,
    "Una vez que la señal analógica se convierte en una señal digital, se utiliza un analizador de frecuencias para determinar su espectro de frecuencias. Este aparato proporciona el espectro de frecuencias de la señal mezclada (señal original de la fuente láser + señal retrodispersada), y por tanto el desplazamiento de frecuencia Doppler."@es;
  skos:inScheme <http://vocab.ieawindtask32.org/wind-lidar-ontology/>;
  skos:narrower ontolidar:FastFourierTransform, ontolidar:FrequencyAnalyserSampleRate,
    ontolidar:PeakIdentification;
  skos:prefLabel "Analizador de frecuencia"@es, "Analizzatore della frequenza"@it, "Frequency analyser"@en,
    "Frequenz-Analysator"@de, "频率分析器"@cn .

ontolidar:PeakIdentification a skos:Concept;
  skos:broader ontolidar:FrequencyAnalyser;
  skos:definition "Detección de pico se refiere al método utilizado por el analizador de frecuencias para obtener la frecuencia Doppler."@es,
    "Metodo di determinazione della frequenza di shift Doppler dagli spettri di potenza."@it,
    "Refers to the method used to retrieve the Doppler frequency shift from the frequency spectra."@en,
    "用于从频谱中检索多普勒频移的方法。"@cn;
  skos:editorialNote "Common methods to detect the peak are the maximum, the median and the centroid function of the frequency spectrum."@en,
    "Los métodos más comunes par la detección del pico son el máximo, la media o el centroide del espectro de frecuencias."@es,
    "Metodi comuni di identificazione del picco in una distribuzione di frequenza."@it;
  skos:inScheme <http://vocab.ieawindtask32.org/wind-lidar-ontology/>;
  skos:prefLabel "Detección de pico"@es, "Identificazione del picco"@it, "Peak identification"@en,
    "Peak-Identifizierung"@de, "峰值识别"@cn;
  skos:related ontolidar:DopplerSpectra .

ontolidar:FastFourierTransform a skos:Concept;
  skos:altLabel "FFT"@en;
  skos:broader ontolidar:FrequencyAnalyser;
  skos:definition "Fast fourier transform. Methodology to transform the lidar data time series into their power spectra."@en,
    "Transformada de Fourier rápida. Método para transformar las series temporales de datos lidar en su espectro de potencias."@es,
    "Trasformata di Fourier rapida. Metodo per trasformare la serie temporale dei dati nel suo spettro di potenza."@it,
    "快速傅里叶变换。将激光雷达数据时间序列转化为其功率频谱的方法。"@cn;
  skos:inScheme <http://vocab.ieawindtask32.org/wind-lidar-ontology/>;
  skos:prefLabel "FFT"@cn, "FFT"@it, "Fast fourier transform"@en, "Schnelle Fourier-Transformation"@de,
    "Transformada de Fourier rápida"@es .

ontolidar:FrequencyAnalyserSampleRate a skos:Concept;
  ontolidar:units "Hz"@en;
  skos:broader ontolidar:FrequencyAnalyser;
  skos:definition "Frequenza di campionamento della velocità radiale. E' l'inverso del numero di spettri che vengono combinati per tale misurazione."@it,
    "Number of frequency spectra the lidar computes (to obtain the radial velocity) during the time of one single realisation."@en,
    "Número de espectros de frecuencia que el lidar computa durante el tiempo necesario para una sola estimación de la velocidad radial."@es,
    "激光雷达计算的频率谱的数量，以获得一个单一实现的径向速度。"@cn;
  skos:inScheme <http://vocab.ieawindtask32.org/wind-lidar-ontology/>;
  skos:prefLabel "Abtastrate des Frequenzanalysators"@de, "Frequency analyser sample rate"@en,
    "Frequenza di campionamento dell'analizzatore"@it, "Tasa de muestreo"@es, "频率分析器采样率"@cn .

ontolidar:StorageModule a skos:Concept;
  skos:broader ontolidar:ControlModule;
  skos:definition "El módulo de almacenamiento se ocupa del almacenaje de datos que serán utilizados por el usuario en el futuro."@es,
    "Sistema di memoria dati del lidar. Utilizzato per avere accesso ai dati in ogni momento, su richiesta dell'utente."@it,
    "The storage module is responsible for saving data in the lidar system which will be accessed by users at some future time."@en,
    "存储模块负责将数据保存在激光雷达系统中，用户将来可以访问这些数据。"@cn;
  skos:editorialNote "Definición basada en el proyecto OpenLidar: https://github.com/e-WindLidar/OpenLidarModuleDefinitions"@es,
    "Definition based on the OpenLidar module definitions at https://github.com/e-WindLidar/OpenLidarModuleDefinitions"@en,
    "Definizione basata sulla definizione di modulo del progetto OpenLidar. Vedasi https://github.com/e-WindLidar/OpenLidarModuleDefinitions"@it;
  skos:inScheme <http://vocab.ieawindtask32.org/wind-lidar-ontology/>;
  skos:prefLabel "Componente di memorizzazione dati"@it, "Módulo de almacenamiento"@es,
    "Speichermodul"@de, "Storage module"@en, "存储模块"@cn .

ontolidar:OpticsModule a skos:Concept;
  skos:broader ontolidar:Design;
  skos:definition "El módulo óptico está diseñado para modificar el rayo láser original y converirlo en radiación con las especificiones deseadas (modos) que pueda ser enviada al objetivo y racibida por el detector de forma adecuada."@es,
    "Parte del lidar che trasforma le proprietà della luce laser da quelle della sorgente a quelle ottimali per essere inviate sul target e poi raccolte dal ricevitore."@it,
    "The optics module is designed to alter the original laser beam into radiation with desired specification that can be sent to the target and received by the detector properly."@en,
    "光学模块旨在将原始激光束转换为具有所需规格的辐射，可以将其发送到目标并由探测器正确接收。”"@cn;
  skos:editorialNote "Definición basada en el proyecto OpenLidar: https://github.com/e-WindLidar/OpenLidarModuleDefinitions"@es,
    "Definition based on the OpenLidar module definitions at https://github.com/e-WindLidar/OpenLidarModuleDefinitions"@en,
    "Definizione basata sulla definizione di modulo del progetto OpenLidar. Vedasi https://github.com/e-WindLidar/OpenLidarModuleDefinitions"@it;
  skos:inScheme <http://vocab.ieawindtask32.org/wind-lidar-ontology/>;
  skos:narrower ontolidar:Telescope;
  skos:prefLabel "Componenti ottiche"@it, "Módulo óptico"@es, "Optics module"@en, "Optik-Modul"@de,
    "光学模块"@cn .

ontolidar:Telescope a skos:Concept;
  skos:broader ontolidar:OpticsModule;
  skos:definition "Il sistema di lenti, specchi ed altri elementi ottici e meccanici che in un lidar emettono e ricevono luce laser."@it,
    "Sistema de lente, espejos y otros componentes ópticos y mecánicos que emiten y reciben el rayo láser."@es,
    "The system of lenses, mirrors and other optical and mechanical components that emit and receive laser light."@en,
    "发射和接收激光的透镜、反射镜和其他光学和机械组件的系统"@cn;
  skos:inScheme <http://vocab.ieawindtask32.org/wind-lidar-ontology/>;
  skos:narrower ontolidar:EndFibreToLensDistance, ontolidar:FocalLength, ontolidar:Lense,
    ontolidar:TelescopeApertureDiameter;
  skos:prefLabel "Fernrohr"@de, "Telescope"@en, "Telescopio"@es, "Telescopio"@it, "望远镜"@cn .

ontolidar:TelescopeApertureDiameter a skos:Concept;
  ontolidar:units "meters"@en;
  skos:broader ontolidar:Telescope;
  skos:definition "Characteristic optical diameter of the lidar telescope. The aperture through which laser light is emitted and received."@en,
    "Diametro ottico del telescopio del lidar. La finestra attraverso cui il laser viene emesso e ricevuto fra lo spazio interno del lidar e l'ambiente esterno."@it,
    "Diámetro de la apertura del telescopio. La aperture a través de la cual se emite y recibe la luz láser."@es,
    "激光雷达望远镜的特征光学直径. 发射和接收激光的孔径"@cn;
  skos:inScheme <http://vocab.ieawindtask32.org/wind-lidar-ontology/>;
  skos:prefLabel "Diametro dell'apertura del telescopio"@it, "Diámetro de apertura del telescopio"@es,
    "Telescope aperture diameter"@en, "Öffnungsdurchmesser des Teleskops"@de, "望远镜光圈直径"@cn .

ontolidar:FocalLength a skos:Concept;
  skos:broader ontolidar:Telescope;
  skos:definition "Distancia focal del telescopio. Distancia entre la lente y su distancia focal."@es,
    "Distanza fra il centro della lente ed il suo punto focale."@it, "Focal length of the telescope. Distance between the lense and its focal lenght."@en,
    "镜头与目标之间的距离。"@cn;
  skos:inScheme <http://vocab.ieawindtask32.org/wind-lidar-ontology/>;
  skos:prefLabel "Brennweite"@de, "Focal length"@en, "Lunghezza focale"@it, "焦距"@cn;
  skos:related ontolidar:ProbeVolume .

ontolidar:EndFibreToLensDistance a skos:Concept;
  skos:broader ontolidar:Telescope;
  skos:definition "Distance between the end-fibre and the lens."@en, "Distancia entre el punto final de la fibra óptica y la lente del telescopio."@es,
    "Distanza fra il punto terminale della fibra ottica ed il centro della lente."@it,
    "末端纤维和透镜之间的距离。连续波激光雷达使用这个距离来改变焦距。"@cn;
  skos:editorialNote "Continuous wave lidars use this distance to vary the focal length."@en,
    "In sistemi a luce continua, parametro di controllo per la distanza di puntamento del sistema laser."@it,
    "Los lidares de onda continua utilizan esta distancia para variar la distancia focal."@es;
  skos:inScheme <http://vocab.ieawindtask32.org/wind-lidar-ontology/>;
  skos:prefLabel "Abstand von der Endfaser zur Linse"@de, "Distanza fra il termine della fibra ottica e la la lente"@it,
    "End-fibre to lens distance"@en, "端部纤维到镜头的距离"@cn;
  skos:related ontolidar:ProbeVolume .

ontolidar:Lense a skos:Concept;
  skos:broader ontolidar:Telescope;
  skos:definition "Optical system to expand the outgoing beam and collimate the backscattered one."@en,
    "Sistema ottico per espandere e collimare un fascio di luce."@it, "Sistema óptico utilizado para expandir y colimar un hay de luz."@es,
    "扩大出射光束，并使后方散射光束准直。"@cn;
  skos:inScheme <http://vocab.ieawindtask32.org/wind-lidar-ontology/>;
  skos:prefLabel "Lense"@en, "Lente"@it, "Lente del telescopio"@es, "Linse"@de, "镜片"@cn .

ontolidar:PhotonicsModule a skos:Concept;
  skos:broader ontolidar:Design;
  skos:definition "El módulo fotónico es la fuente de emisión de luz utilizada para efectuar las medidas."@es,
    "Modulo sorgente della luce laser utilizzato per le misurazioni."@it, "The photonics module is the source of emitted light that will be used for the measurements."@en,
    "光子模块是用于测量的发射光的光源。"@cn;
  skos:editorialNote "Definición basada en el proyecto OpenLidar: https://github.com/e-WindLidar/OpenLidarModuleDefinitions"@es,
    "Definition based on the OpenLidar module definitions at https://github.com/e-WindLidar/OpenLidarModuleDefinitions"@en,
    "Definizione basata sulla definizione di modulo del progetto OpenLidar. Vedasi https://github.com/e-WindLidar/OpenLidarModuleDefinitions"@it;
  skos:inScheme <http://vocab.ieawindtask32.org/wind-lidar-ontology/>;
  skos:narrower ontolidar:AcoustoOpticModulator, ontolidar:BackscatteredLight, ontolidar:Detector,
    ontolidar:EmittedLight, ontolidar:Interfaces, ontolidar:LaserSource;
  skos:prefLabel "Componente fotonica"@it, "Módulo de fotónica"@es, "Photonics module"@en,
    "Photonik-Modul"@de, "光子模块"@cn .

ontolidar:LaserSource a skos:Concept;
  skos:broader ontolidar:PhotonicsModule;
  skos:definition "An assembly to generate and manage laser light."@en, "Conjunto de dispositivos para generar y regular el rayo de luz láser."@es,
    "Un sistema di generazione e controllo della luce laser."@it, "一种产生和控制激光的组件。"@cn;
  skos:inScheme <http://vocab.ieawindtask32.org/wind-lidar-ontology/>;
  skos:narrower ontolidar:LaserDiode, ontolidar:LaserMode, ontolidar:LaserWavelength;
  skos:prefLabel "Fuente láser"@es, "Laser source"@en, "Laserquelle"@de, "Sorgente laser"@it,
    "激光源"@cn .

ontolidar:LaserDiode a skos:Concept;
  skos:broader ontolidar:LaserSource;
  skos:definition "A semiconductor component to generate laser light of a defined frequency."@en,
    "Componente semiconductor destinado a generar luz láser de frecuencia definida."@es,
    "Un dispositivo optoelettronico a semiconduttore che genera luce laser monocromatica."@it,
    "一种半导体元件，用于产生规定频率的激光。"@cn;
  skos:inScheme <http://vocab.ieawindtask32.org/wind-lidar-ontology/>;
  skos:prefLabel "Diodo laser"@it, "Diodo láser"@es, "Laser diode"@en, "Laserdiode"@de,
    "激光二极管"@cn .

ontolidar:LaserMode a skos:Concept;
  skos:broader ontolidar:LaserSource;
  skos:definition "Integer characterising the relation between wavelength and laser cavity length."@en,
    "Numeri interi dati dal rapporto fra la lunghezza d'onda della luce emessa e la lunghezza della cavità laser emettitrice."@it,
    "Números enteros dados por la relación entre la longitud de onda de la luz emitida y la longitud de la cavidad del láser."@es,
    "表征波长和激光腔体长度之间关系的整数。是激光光和激光谐振腔特性的组合。给定一个特定的波长和激光腔的长度，只允许有某些模式。"@cn;
  skos:editorialNote "Combinazione di luce laser e risonanza laser in cavita'."@it,
    "Dada una cierta longitud de onda de la luz y una longitud de la cavidad láser, sólo ciertos modos son permitidos."@es,
    "Is a combination of laser light and laser resonance cavity characteristics. Given a certain wavelength, and length of the laser cavity only certain modes are permitted."@en;
  skos:inScheme <http://vocab.ieawindtask32.org/wind-lidar-ontology/>;
  skos:narrower ontolidar:LaserFrequency, ontolidar:LaserIntensity, ontolidar:LaserPhase,
    ontolidar:LaserPolarisation;
  skos:prefLabel "Laser mode"@en, "Laser-Modus"@de, "Modo del laser"@it, "激光模式"@cn .

ontolidar:LaserFrequency a skos:Concept;
  skos:broader ontolidar:LaserMode;
  skos:definition "Frecuencia de la luz de la fuente láser."@es, "Frequenza della luce della sorgente laser."@it,
    "Light frequency of the laser source."@en, "激光源的光频率。"@cn;
  skos:inScheme <http://vocab.ieawindtask32.org/wind-lidar-ontology/>;
  skos:prefLabel "Frequenza del laser"@it, "Laser frequency"@en, "Laserfrequenz"@de,
    "激光频率"@cn .

ontolidar:LaserPolarisation a skos:Concept;
  skos:broader ontolidar:LaserMode;
  skos:definition "Polarización de la luz de la fuente láser."@es, "Polarization of the laser source signal."@en,
    "Polarizzazione della luce della sorgente laser."@it, "激光源信号的偏振。"@cn;
  skos:inScheme <http://vocab.ieawindtask32.org/wind-lidar-ontology/>;
  skos:prefLabel "Laser polarisation"@de, "Laser polarisation"@en, "Polarizzazione del laser"@it,
    "激光偏振"@cn .

ontolidar:LaserPhase a skos:Concept;
  skos:broader ontolidar:LaserMode;
  skos:definition "Fase de la luz de la fuente láser."@es, "Fase della luce della sorgente laser."@it,
    "Light phase of the laser source."@en, "激光源的光相位。"@cn;
  skos:inScheme <http://vocab.ieawindtask32.org/wind-lidar-ontology/>;
  skos:prefLabel "Fase del laser"@it, "Laser phase"@en, "Laserphase"@de, "激光相位"@cn .

ontolidar:LaserIntensity a skos:Concept;
  skos:broader ontolidar:LaserMode;
  skos:definition "Intensidad de la luz de la fuente láser."@es, "Intensità della luce della sorgente laser."@it,
    "Light intensity of the laser source."@en, "激光源的光强度。"@cn;
  skos:inScheme <http://vocab.ieawindtask32.org/wind-lidar-ontology/>;
  skos:prefLabel "Intensità del laser"@it, "Laser intensity"@en, "Laserintensität"@de,
    "激光强度"@cn .

ontolidar:LaserWavelength a skos:Concept;
  ontolidar:units "meters"@en;
  skos:broader ontolidar:LaserSource;
  skos:definition "La lunghezza d'onda nominale della sorgente laser. Definita in unità di lunghezzza (metri): ad esempio 1450E-9 m per una sorgente laser nel vicino infrarosso."@it,
    "Longitud de onda nominal del láser."@es, "The nominal wavelength of the laser source."@en,
    "激光源的标称波长。这是以米为单位定义的，例如，对于近红外激光源，1450E-9米。"@cn;
  skos:editorialNote "In unita' di metri."@it, "This is defined in units of meters, e.g., 1450e-9 m for a near-infrared laser source."@en,
    "Unidad en metros"@es;
  skos:inScheme <http://vocab.ieawindtask32.org/wind-lidar-ontology/>;
  skos:prefLabel "Laser wavelength"@en, "Laser-Wellenlänge"@de, "Longitud de onda del diodo láser"@es,
    "Lunghezza d'onda del laser"@it, "激光二极管波长"@cn .

ontolidar:AcoustoOpticModulator a skos:Concept;
  skos:altLabel "AOM"@en, "Bragg cell"@en;
  skos:broader ontolidar:PhotonicsModule;
  skos:definition "Celda de Bragg utilizada para difractar y trasladar la frecuencia de la luz mediante el uso de ondas sonoras de radiofrecuencia. Produce un rayo pulsado a la salida."@es,
    "Cella di Bragg per diffrangere e traslare in frequenza la luce utilizzando onde sonore a radiofrequenza. Produce un fascio pulsato in uscita."@it,
    "Device using the acousto-optic effect to change the frequency of the light beam by means of sound waves, usually radiofrequency. It is used in pulsed lidars to create the pulse from the continuously emmited light by the laser source. Usually referred as Bragg cell."@en,
    "布拉格单元利用声波（射频）对光进行衍射和移频。产生一个脉冲输出光束。"@cn;
  skos:editorialNote "Only pulsed lidar"@en, "Sólo válido para lidar pulsado"@es, "Valido solo per sistemi lidar impulsati"@it;
  skos:inScheme <http://vocab.ieawindtask32.org/wind-lidar-ontology/>;
  skos:narrower ontolidar:InsertionLoss, ontolidar:Pulsedmethod, ontolidar:RadioFrequency;
  skos:prefLabel "Acousto-optic modulator"@en, "Akusto-optischer Modulator"@de, "Modulador acusto-óptico"@es,
    "Modulatore acusto-ottico"@it, "声光调制器"@cn .

ontolidar:RadioFrequency a skos:Concept;
  skos:broader ontolidar:AcoustoOpticModulator;
  skos:definition "Frequenza radio usata dal modulatore acustico per modulare l'impulso luminoso (per lidar impulsati)"@it,
    "Radio frecuencia utilizada por el modulador acústico-óptico para modular el pulso de luz. Sólo para lídares pulsados."@es,
    "Radio frequency used by the acoustic modulator to modulate the pulse (for pulsed lidars)."@en,
    "声学调制器用于调制脉冲的无线电频率（对于脉冲激光雷达）。"@cn;
  skos:inScheme <http://vocab.ieawindtask32.org/wind-lidar-ontology/>;
  skos:prefLabel "AOM 无线电频率"@cn, "Frequenza radio AOM"@it, "Radio frequency"@en, "Radiofrequenz"@de .

ontolidar:Pulsedmethod a skos:Concept;
  skos:broader ontolidar:AcoustoOpticModulator;
  skos:definition "Method used to shape the pulse in pulsed lidars"@en, "Metodo per regolare la forma dell'impulso in lidar impulsati."@it,
    "Método para regular la forma de un pulso de luz."@es, "用来塑造脉冲的方法"@cn;
  skos:inScheme <http://vocab.ieawindtask32.org/wind-lidar-ontology/>;
  skos:narrower ontolidar:Qswitching;
  skos:prefLabel "AOM 脉冲法"@cn, "Metodo impulsato AOM"@it, "PulsedMethod"@en, "Pulsierungsmethode"@de .

ontolidar:Qswitching a skos:Concept;
  skos:broader ontolidar:Pulsedmethod;
  skos:definition "Technique by which short light pulses can be obtained from a continuous wave laser source, with a given pulse repetition rate controlled via a modulator."@en,
    "Tecnica di produzione di impulsi brevi di luce a partire da una sorgente laser di luce continua. La frequenza dell'impulso è regolata da un modulatore."@it,
    "Técnica para la formación de pulsos de luz a partir the una fuente láser de radiación continua. Un modulador regula la frecuencia en la emisión del pulso."@es,
    "可从连续波激光源获得短光脉冲的技术，尖端为纳秒，通过调制器控制特定的脉冲重复率。"@cn;
  skos:inScheme <http://vocab.ieawindtask32.org/wind-lidar-ontology/>;
  skos:prefLabel "AOM QSwitching"@cn, "QSwitch AOM"@it, "QSwitching"@de, "QSwitching"@en .

ontolidar:InsertionLoss a skos:Concept;
  skos:broader ontolidar:AcoustoOpticModulator;
  skos:definition "Perdita di potenza dovuta alla presenza di un modulatore acustico."@it,
    "Power loss due to the insertion of the acousto-optic modulator."@en, "Pérdida de potencia debido a la inserción del modulador acústico-óptico."@es,
    "由于插入了声学调制器而造成的功率损失。"@cn;
  skos:inScheme <http://vocab.ieawindtask32.org/wind-lidar-ontology/>;
  skos:prefLabel "AOM插入损耗"@cn, "Insertion loss"@en, "Leistungsverlust"@de, "Perdita di potenza AOM"@it .

ontolidar:EmittedLight a skos:Concept;
  skos:broader ontolidar:PhotonicsModule;
  skos:definition "Características de la luz emitida: intensidad, frecuencia/longitud de onda y polarización. Los lidares pueden clasificarse según distintos parámetros de diseño. Una de las posibles clasificaciones se basa en la diferencia de luz emitida: continua o pulsada."@es,
    "Caratterisiche della luce emessa: intensità, frequenza (o lunghezza d'onda), polarizzazione. Non da ultimo, tipo di sorgente luminosa: pulsata o continua."@it,
    "Characteristics of the emitted light, namely: intensity, frequency/wavelength and polarisation. Lidar can be classified differently according to different design parameters. One of the possible classifications is based on the difference of emmited light: pulsed or continuous wave."@en,
    "发出的光的特性，即：强度、频率/波长和偏振。根据不同的设计参数，激光雷达可以有不同的分类。其中一个可能的分类是基于发射光的差异。在这个意义上，激光雷达可以被描述为脉冲激光雷达，即激光雷达发射脉冲光或连续波激光雷达，即激光雷达以连续形式发射光。"@cn;
  skos:inScheme <http://vocab.ieawindtask32.org/wind-lidar-ontology/>;
  skos:narrower ontolidar:ContinuousWaveLidar, ontolidar:PulsedLidar;
  skos:prefLabel "Ausgestrahltes Licht"@de, "Emitted light"@en, "Luce emessa"@it, "发出的光"@cn;
  skos:related ontolidar:AcoustoOpticModulator .

ontolidar:ContinuousWaveLidar a skos:Concept;
  skos:broader ontolidar:EmittedLight;
  skos:definition "Caracterización de los lidares basada en el tipo de luz emitida. Los lidares de onda continua (CW) se caracterizan por su emisión continua de radiación."@es,
    "Lidar characterisation based on the emitted type of light. Continuous wave lidars (CW) are characterised by its continuous emission of radiation."@en,
    "Lidar la cui luce è emessa in modo continuo."@it, "发出的光的类型，其特点是连续发射"@cn;
  skos:inScheme <http://vocab.ieawindtask32.org/wind-lidar-ontology/>;
  skos:prefLabel "Continuous Wave lidar"@en, "Kontinuierliches Lidar"@de, "Lidar ad onda continua"@it,
    "连续波激光雷达"@cn .

ontolidar:PulsedLidar a skos:Concept;
  skos:broader ontolidar:EmittedLight;
  skos:definition "Caracterización del lidar basada en el tipo de luz emitida. Este tipo de lidar se caracteriza por su emisión pulsada de radiación. La señal lidar emitida originalmente de forma continua se modula para obtener una radiación de duración determinada emitida a un ritmo determinado, a diferencia de la emisión continua."@es,
    "Lidar characterisation based on the emitted type of light. This type of lidar is characterised by its pulsed emission of radiation. The originally continuously emitted lidar signal is modulated to obtain radiation of specified duration emitted at a certain rate, as opposed to continuous emission."@en,
    "Lidar la cui luce è modulata nella forma di impulsi."@it, "发出的光被调制成脉冲发射的激光雷达。"@cn;
  skos:inScheme <http://vocab.ieawindtask32.org/wind-lidar-ontology/>;
  skos:narrower ontolidar:PulseDuration, ontolidar:PulseSampleRate, ontolidar:PulseShape;
  skos:prefLabel "Gepulstes Lidar"@de, "Lidar pulsati"@it, "Pulsed lidar"@en, "脉冲激光雷达"@cn .

ontolidar:PulseDuration a skos:Concept;
  skos:broader ontolidar:PulsedLidar;
  skos:definition "Duración del pulso luminoso. Caracteriza la longitud del volumen de medición del lidar."@es,
    "Durata dell'impulso emesso. Caratterizza la lunghezza della sonda."@it, "Duration of the light pulse. Characterises the length of the probe volume."@en,
    "光脉冲的持续时间。表明探测体积的长度。"@cn;
  skos:editorialNote "Lidars do not measure in a single point but rather whithin a probe volume. The full width at half maximum (FWHM) of the function characterising the pulse shape defines the probe volume whithin which the lidar is measuring. Therefore, the pulse duration directly impacts lidar estimations, since higher pulse durations give rise to longer probe volumes."@en,
    "Los lidares no miden en un solo punto, sino a lo largo de un volumen en la dirección del rayo. La anchura a media altura ( o FWHM por sus siglas en inglés) de la función que caracteriza la forma del pulso define el volumen de la sonda dentro del cual el lidar está midiendo. Por lo tanto, la duración del pulso influye directamente en las estimaciones del lidar, ya que una mayor duración del pulso da lugar a volúmenes de medición mayores."@es;
  skos:inScheme <http://vocab.ieawindtask32.org/wind-lidar-ontology/>;
  skos:narrower ontolidar:FullWidthAtHalfMaximum;
  skos:prefLabel "Dauer des Pulses"@de, "Durata dell'impulso"@it, "Pulse duration"@en,
    "脉冲持续时间"@cn .

ontolidar:FullWidthAtHalfMaximum a skos:Concept;
  skos:altLabel "FWHM"@en;
  skos:broader ontolidar:PulseDuration;
  skos:definition "En una distribución, la anchuraa media altura representa la distancia entre los dos valores de la variable independiente (eje x) cuando el valor de la variable dependiente (eje y) es la mitad de su valor máximo."@es,
    "In a distribution, the full width at half maximum represents the distance between the two values of the independent variable (x axis) when the value of the dependent variable (y axis) is half of its maximum value."@en,
    "In una distribuzione, distanza fra due valori di ascissa che producono un'ordinata pari a meta' del valore massimo delle ordinate."@it,
    "是指在函数的一个峰当中，前后两个函数值等于峰值一半的点之间的距离"@cn;
  skos:inScheme <http://vocab.ieawindtask32.org/wind-lidar-ontology/>;
  skos:prefLabel "Anchura a media altura"@es, "Full width at half maximum"@en, "Larghezza a meta' altezza"@it,
    "Volle Breite bei halbem Maximum"@de, "半峰全宽"@cn .

ontolidar:PulseSampleRate a skos:Concept;
  skos:broader ontolidar:PulsedLidar;
  skos:definition "Espacio de tiempo entre dos pulsos enviados por un lidar pulsado para muestrear el viento."@es,
    "Tempo fra due impulsi laser inviati nell'ambiente da un lidar pulsato."@it, "Time slot between two pulses sent by a pulsed lidar to sample the wind."@en,
    "发送的脉冲之间的时隙，以对风进行采样。"@cn;
  skos:inScheme <http://vocab.ieawindtask32.org/wind-lidar-ontology/>;
  skos:prefLabel "Frequenza di campionamento del laser pulsato"@it, "Puls-Abtastrate"@de,
    "Pulse sample rate"@en, "脉冲采样率"@cn .

ontolidar:PulseShape a skos:Concept;
  skos:broader ontolidar:PulsedLidar;
  skos:definition "Forma del pulso emitido."@es, "Forma dell'impulso emesso."@it, "Shape of the emitted pulse."@en,
    "发射脉冲的形状"@cn;
  skos:editorialNote "Continuous wave light can be modulated (e.g. with an acousto-optic-modulator or AOM) to obtain pulses at high power intensities altering the transmitted power and concentrating this energy in a short space. The power intensity around this area can be described as a gaussian function centered around the frequency of interest, which is commonly used to describe the shape of the pulse."@en,
    "La luz de onda continua puede modularse (por ejemplo, con un modulador acústico-óptico o AOM) para obtener pulsos a altas intensidades de potencia alterando la potencia transmitida y concentrando esta energía en un espacio corto. La intensidad de la potencia alrededor de esta zona puede describirse como una función gaussiana centrada en la frecuencia de interés y se suele utilizar para describir la forma del pulso."@es;
  skos:inScheme <http://vocab.ieawindtask32.org/wind-lidar-ontology/>;
  skos:prefLabel "Form des Pulses"@de, "Forma dell'impulso"@it, "Pulse shape"@en, "脉冲形状"@cn .

ontolidar:BackscatteredLight a skos:Concept;
  skos:broader ontolidar:PhotonicsModule;
  skos:definition "Backscattered light reaching the lidar detector."@en, "Luce che raggiunge il fotorivelatore del lidar."@it,
    "Luz retrodispersada que alcanza el detector del lidar."@es, "到达激光雷达探测器的反向散射光。"@cn;
  skos:inScheme <http://vocab.ieawindtask32.org/wind-lidar-ontology/>;
  skos:narrower ontolidar:DesiredBackscatteredLight, ontolidar:NonDesiredBackscatteredLight;
  skos:prefLabel "Backscattered light"@en, "Luce riflessa"@it, "Rückgestreutes Licht"@de,
    "背向散射光"@cn .

ontolidar:DesiredBackscatteredLight a skos:Concept;
  skos:broader ontolidar:BackscatteredLight;
  skos:definition "Porción de señal lidar retrodispersada con componentes de frecuencia y polarización deseados. Señal que se debe al movimiento del viento."@es,
    "Portion of the backscattered light with desired frequency and polarization, reaching the detector."@en,
    "Porzione della luce che raggiunge il fotorivelatore proveniente dal moto ventoso (tipicamente polarizzata)."@it,
    "到达检测器，具有所需频率和偏振的部分反向散射光。"@cn;
  skos:inScheme <http://vocab.ieawindtask32.org/wind-lidar-ontology/>;
  skos:prefLabel "Desired backscattered light"@en, "Gewünschtes Rückstreulicht"@de,
    "Luce riflessa portatrice di segnale"@it, "希望的背向散射光"@cn .

ontolidar:NonDesiredBackscatteredLight a skos:Concept;
  skos:broader ontolidar:BackscatteredLight;
  skos:definition "Non-desired light from atmosphere (non polarised) reaching the detector."@en,
    "Porción de la luz que llega al detector lidar que no se debe al movimiento del viento (normalmente no polarizada)."@es,
    "Porzione della luce che raggiunge il fotorivelatore non dovuta al moto ventoso (tipicamente non polarizzata)."@it,
    "到达检测器的，来自大气（非偏振）的非期望光信号。"@cn;
  skos:inScheme <http://vocab.ieawindtask32.org/wind-lidar-ontology/>;
  skos:prefLabel "Luce riflessa portatrice di rumore ambientale"@it, "Nicht erwünschtes Rückstreulicht"@de,
    "Non-desired backscattered light"@en, "非期望的后向散射光"@cn .

ontolidar:Detector a skos:Concept;
  skos:broader ontolidar:PhotonicsModule;
  skos:definition "An assembly to gather and detect incident light."@en, "Conjunto de dispositivos encargados de recoger y detectar la luz incidente."@es,
    "Gruppo di sistemi per ricevere, rilevare e misurare la luce incidente."@it, "收集和检测入射光的组件"@cn;
  skos:inScheme <http://vocab.ieawindtask32.org/wind-lidar-ontology/>;
  skos:narrower ontolidar:BeamSplitter, ontolidar:OpticalAmplifier, ontolidar:Photodetector;
  skos:prefLabel "Detector"@en, "Detector"@es, "Detektor"@de, "Rilevatore"@it, "探测器"@cn .

ontolidar:OpticalAmplifier a skos:Concept;
  skos:broader ontolidar:Detector;
  skos:definition "An assembly to amplify the outgoing laser light signal."@en, "Conjunto de dispositivos utilizados para amplificar la luz del láser emitido sin convertirlo previemente en señal eléctrica."@es,
    "Sistema di amplificazione della potenza ottica della luce laser emessa."@it, "用于放大输出激光信号的组件。"@cn;
  skos:editorialNote "Definición basada en el artícule de wikipedia: https://en.wikipedia.org/wiki/Optical_amplifier"@es,
    "Definition based on Wikipedia entry at https://en.wikipedia.org/wiki/Optical_amplifier"@en,
    "Definizione basata sulla definizione di modulo del progetto OpenLidar. Vedasi https://github.com/e-WindLidar/OpenLidarModuleDefinitions"@it;
  skos:inScheme <http://vocab.ieawindtask32.org/wind-lidar-ontology/>;
  skos:narrower ontolidar:OpticalAmplifierBandwidth, ontolidar:OpticalAmplifierGain;
  skos:prefLabel "Amplificador óptico"@es, "Amplificatore ottico"@it, "Optical amplifier"@en,
    "Optischer Verstärker"@de, "光放大器"@cn .

ontolidar:OpticalAmplifierGain a skos:Concept;
  skos:broader ontolidar:OpticalAmplifier;
  skos:definition "Ganancia de potencia debida a la amplificación óptica."@es, "Guadagno di potenza dovuto all'amplificazione ottica"@it,
    "Power gain due to the optical amplification."@en, "光放大带来的功率增益"@cn;
  skos:inScheme <http://vocab.ieawindtask32.org/wind-lidar-ontology/>;
  skos:prefLabel "Guadagno dell'amplificatore ottico"@it, "Optical amplifier gain"@en,
    "Verstärkung des optischen Verstärkers"@de, "光放大器增益"@cn .

ontolidar:OpticalAmplifierBandwidth a skos:Concept;
  skos:broader ontolidar:OpticalAmplifier;
  skos:definition "Ancho de banda de la frecuencia de trabajo del amplificador óptico."@es,
    "Banda di frequenza attiva nell'amplificatore ottico."@it, "Working bandwith of the optical amplifier."@en,
    "光放大器的工作带宽"@cn;
  skos:inScheme <http://vocab.ieawindtask32.org/wind-lidar-ontology/>;
  skos:prefLabel "Bandbreite des optischen Verstärkers"@de, "Larghezza d'onda dell'amplificatore ottico"@it,
    "Optical amplifier bandwidth"@en, "光放大器带宽"@cn .

ontolidar:BeamSplitter a skos:Concept;
  skos:altLabel "beamsplitter"@en;
  skos:broader ontolidar:Detector;
  skos:definition "An optical assembly to split the laser beam into two or more beams (multi beams)."@en,
    "Sistema óptico para dividir el rayo láser en dos o más rayos."@es, "Un sistema ottico per la divisione di un fascio laser in due o più fasci."@it,
    "一种将激光束分成两束或更多束的光学组件。"@cn;
  skos:editorialNote "En un lidar, el haz de la fuente láser se divide en dos haces diferentes. Uno se envía a la atmósfera para detectar el movimiento de los aerosoles. El otro se envía al fotodetector, donde se utilizará como referencia local para identificar el cambio de frecuencia del haz retrodispersado. Por lo general, el divisor de haz también polariza el haz para que se pueda distinguir de la luz de fondo atmosférica, típicamente no polarizada."@es,
    "In a lidar, the laser source beam is split into two different beams. One is sent out to the atmosphere to detect the aerosols motion. The other one is sent to the photodetector, where it will be used as a local reference to identify the frequency shift of the backscattered beam. Usually the beam splitter also polarises the beam so that it is distinguishable from the atmospheric background light."@en;
  skos:inScheme <http://vocab.ieawindtask32.org/wind-lidar-ontology/>;
  skos:prefLabel "Beam splitter"@en, "Divisor de haz"@es, "Sdoppiatore ottico"@it, "Strahlteiler"@de,
    "分束器"@cn .

ontolidar:Photodetector a skos:Concept;
  skos:broader ontolidar:Detector;
  skos:definition "Fotosensore a semi-conduttori."@it, "Semiconductor light sensor."@en,
    "Sensor de luz semiconductor."@es, "半导体光传感器。"@cn;
  skos:inScheme <http://vocab.ieawindtask32.org/wind-lidar-ontology/>;
  skos:prefLabel "Fotodetector"@es, "Fotorivelatore"@it, "Photodetector"@en, "Photodetektor"@de,
    "光电探测器"@cn .

ontolidar:PhotodetectorGain a skos:Concept;
  skos:broader ontolidar:PhotoDetector;
  skos:definition "Guadagno dell'amplificatore a transimpedenza del fotodetettore."@it,
    "Ratio between the output current of the photodetector and the current generated by the photons reaching its active area."@en,
    "Relación entre la corriente de salida del fotodetector y la corriente generada por los fotones que llegan a su zona activa."@es,
    "光电探测器的输出电流与到达其有效区域的光子所产生的电流之间的比率。"@cn;
  skos:inScheme <http://vocab.ieawindtask32.org/wind-lidar-ontology/>;
  skos:prefLabel "Ganancia del fotodetector"@es, "Guadagno del fotorivelatore"@it, "Photodetector gain"@en,
    "Verstärkung des Photodetektors"@de, "光电探测器增益"@cn .

ontolidar:PhotodetectorActiveArea a skos:Concept;
  skos:broader ontolidar:PhotoDetector;
  skos:definition "Area del fotodiodo dove la luce di backscatter viene convogliata per produrre un segnale elettrico via effetto fotoelettrico. La sua dimensione e forma possono variare molto, da meno di un millimetro quadrato a più di un centimetro quadrato. La sensività del fotodetettore è influenzata dalla sua area attiva, siccome l'area attiva produce migliore (inferiore) sensività."@it,
    "Photodiode area where the backscattered light is focused onto (and the photoelectric effect occurs) in order to convert it into an electrical signal. Photodetector sensitivity is affected by the active area, since larger active areas yield better (lower) sensitivity."@en,
    "Área del fotodiodo donde se enfoca la luz retrodispersada (y se produce el efecto fotoeléctrico) para convertirla en una señal eléctrica. La sensibilidad del fotodetector depende del área activa, ya que las áreas activas más grandes proporcionan una mejor (menor) sensibilidad."@es,
    "光电二极管区域，背向散射光被聚焦到这里（并发生光电效应），以便将其转换为电信号。光电探测器的灵敏度受有源区的影响，因为更大的有源区产生更好（更低）的灵敏度。"@cn;
  skos:editorialNote "E.G.: sensitivity of 1nW means that I can distinguish 1mW signal from noise, which is better than a sensitivity of 1W"@en,
    "Por ejemplo, una sensibilidada de 1nW significa que puedo distinguir una señal de 1mW con respecto al ruido, lo cual corresponde a una sensibilidad mejor que 1W"@es;
  skos:inScheme <http://vocab.ieawindtask32.org/wind-lidar-ontology/>;
  skos:prefLabel "Aktive Fläche des Photodetektors"@de, "Area attiva del fotorivelatore"@it,
    "Photodetector active area"@en, "光电探测器的有效面积"@cn .

ontolidar:PhotodetectorSnr a skos:Concept;
  skos:broader ontolidar:PhotoDetector;
  skos:definition "Photodetector signal to noise ratio. Main contributors are: Thermal noise, shot noise and dark current noise."@en,
    "Rapporto segnale/rumore del fotodetettore. I principali contributi al rumore sono il rumore termico, il sumore di shot ed il rumore da correnti nere."@it,
    "Relación señal /ruido del fotodetector. Principales contribuciones al ruido son la temperatura, el ruido de disparo (o shot noise en inglés) y la corriente de oscuridad ( o dark current in inglés)."@es,
    "光电探测器的信噪比。噪声的主要来源包括：热噪声、射击噪声和暗电流噪声。"@cn;
  skos:inScheme <http://vocab.ieawindtask32.org/wind-lidar-ontology/>;
  skos:prefLabel "Photodetector SNR"@en, "Photodetektor SNR"@de, "SNR del fotorivelatore"@it,
    "光电探测器SNR"@cn .

ontolidar:PhotodetectorVoltageNoise a skos:Concept;
  skos:broader ontolidar:PhotoDetector;
  skos:definition "Ruido de voltaje del fotodetector."@es, "Rumore di tensione dell'amplificatore a transimpedenza del fotodetettore."@it,
    "The voltage noise of the photodetector."@en, "光电探测器的电压噪声。"@cn;
  skos:inScheme <http://vocab.ieawindtask32.org/wind-lidar-ontology/>;
  skos:prefLabel "Photodetector voltage noise"@en, "Ruido de voltaje del fotodetector"@es,
    "Rumore di tensione del fotorivelatore"@it, "Spannungsrauschen des Photodetektors"@de,
    "光电探测器电压噪声"@cn .

ontolidar:Interfaces a skos:Concept;
  skos:broader ontolidar:PhotonicsModule;
  skos:definition "Beam transmission system."@en, "Sistema de transmisión de la señal lidar."@es,
    "Sistema di trasmissione del lidar."@it, "光束传输系统"@cn;
  skos:editorialNote "True if lidar is all-fibre"@en, "True si el lidar es all-fibre"@es,
    "Vero per sistemi all-fibre"@it;
  skos:inScheme <http://vocab.ieawindtask32.org/wind-lidar-ontology/>;
  skos:narrower ontolidar:Fibre;
  skos:prefLabel "Interfacce"@it, "Interfaces"@en, "Schnittstellen"@de, "接口"@cn .

ontolidar:Fibre a skos:Concept;
  skos:broader ontolidar:Interfaces;
  skos:definition "Sistema de transmisión de la rayo lidar basado en fibra óptica."@es,
    "Sistema di trasmissione del fascio laser basato du un sistema di fibra ottica."@it,
    "Transmission system for the laser beam based on fibre optic."@en, "基于光纤的激光束传输系统。"@cn;
  skos:editorialNote "El hardware del lidar se conecta entre sí mediante fibra óptica para la transmisión del láser. El uso de fibra óptica es especialmente importante en el módulo óptico, ya que evita el costoso proceso de alineamiento del láser."@es,
    "Lidar hardware components are connected to each other by fibre optics to guide the laser beam along its path. Specially for the telescope module, using fibre optics makes possible to avoid costly and cumbersome alignment processes."@en;
  skos:inScheme <http://vocab.ieawindtask32.org/wind-lidar-ontology/>;
  skos:prefLabel "Faser"@de, "Fibra"@it, "Fibre"@en, "光纤"@cn .

ontolidar:PowerModule a skos:Concept;
  skos:broader ontolidar:Design;
  skos:definition "El módulo de potencia (o de alimentación) es responsable de abastecer al lidar de la energía necesaria para el funcionamiento del sistema, incluyendo motores, láser, sensores, detectores y cualquier elemento activo que requiera electricidad."@es,
    "Modulo di rifornimento e distribuzione dell'energia in ogni parte del sistema lidar, inclusi i motori, il laser, i sensori ed il ricevitore."@it,
    "The Power Module is responsible for supplying power to the entire lidar system, including motors, lasers, sensors, detectors and active elements."@en,
    "电源模块负责为整个激光雷达系统供电，包括对电机、激光器、传感器和探测器等的供电。"@cn;
  skos:editorialNote "Definición basada en el proyecto OpenLidar: https://github.com/e-WindLidar/OpenLidarModuleDefinitions"@es,
    "Definition based on the OpenLidar module definitions at https://github.com/e-WindLidar/OpenLidarModuleDefinitions"@en,
    "Definizione basata sulla definizione di modulo del progetto OpenLidar. Vedasi https://github.com/e-WindLidar/OpenLidarModuleDefinitions"@it;
  skos:inScheme <http://vocab.ieawindtask32.org/wind-lidar-ontology/>;
  skos:narrower ontolidar:PowerConverter, ontolidar:UninterruptablePowerSupply;
  skos:prefLabel "Componente di alimentazione"@it, "Módulo de alimentación"@es, "Netzteil"@de,
    "Power module"@en, "电源模块"@cn .

ontolidar:PowerConverter a skos:Concept;
  skos:broader ontolidar:PowerModule;
  skos:definition "Device used to convert the voltage, frequency or a combination of both from an external source into the volltage and frequency usable by the lidar and its various componets."@en,
    "Dispositivo utilizado para convertir el voltaje, la frecuencia o una combinación de ambos de una fuente externa en el voltaje y la frecuencia utilizables por el lidar y sus diversos componentes."@es;
  skos:editorialNote "Lidar can operate in DC current."@en;
  skos:inScheme <http://vocab.ieawindtask32.org/wind-lidar-ontology/>;
  skos:prefLabel "Converter di potenza"@it, "Convertidor de potencia"@es, "Power converter"@en,
    "Wechselrichter"@de, "电源转换器"@cn .

ontolidar:UninterruptablePowerSupply a skos:Concept;
  skos:broader ontolidar:PowerModule;
  skos:definition "A device provided with batteries and a transformer ensuring a continuous and reliable power supply. This device allows the lidar to work off-line."@en,
    "Gruppo di continuità (UPS)."@it, "Sistema de alimentación ininterrumpida (SAI)."@es,
    "一个配有电池和变压器的装置，确保了持续和可靠的电力供应。这个装置保证激光雷达短暂脱离供电线后依然可以工作。"@cn;
  skos:inScheme <http://vocab.ieawindtask32.org/wind-lidar-ontology/>;
  skos:prefLabel "Gruppo di continuità (UPS)"@it, "Sistema de alimentación ininterrumpida o SAI"@es,
    "Uninterruptable power supply"@en, "Unterbrechungsfreie Stromversorgung"@de, "不间断电源(UPS)"@cn .

ontolidar:UpsBatteryVoltage a skos:Concept;
  ontolidar:units "volts"@en;
  skos:broader ontolidar:UninterruptiblePowerSupply;
  skos:definition "Il voltaggio della batteria (in unità di Volt)."@it, "The battery voltage."@en,
    "Voltaje de la batería."@es, "电池电压。"@cn;
  skos:inScheme <http://vocab.ieawindtask32.org/wind-lidar-ontology/>;
  skos:prefLabel "UPS battery voltage"@en, "UPS电池电压"@cn, "USV-Batteriespannung"@de,
    "Voltaggio della batteria dell'UPS"@it, "Voltaje de batería del SAI"@es .

ontolidar:UpsBatteryCapacity a skos:Concept;
  ontolidar:units "Ah"@en;
  skos:broader ontolidar:UninterruptiblePowerSupply;
  skos:definition "La capacidad máxima del sistema de alimentación ininterrumpida en unidades de amperio-hora (Ah)."@es,
    "La capacità massima del gruppo di continuità (in unità di Ampere-ora (Ah))."@it,
    "The maximum capacity of the uninterruptable power supplier in units of Ampere-hour."@en,
    "电池电压中存储的总能量，单位是安培小时 (Ah)"@cn;
  skos:inScheme <http://vocab.ieawindtask32.org/wind-lidar-ontology/>;
  skos:prefLabel "Capacidad de la batería del SAI"@es, "Capacità della batteria dell'UPS"@it,
    "UPS battery capacity"@en, "UPS电池容量"@cn, "USV-Batteriekapazität"@de .

ontolidar:UpsBatteryPower a skos:Concept;
  ontolidar:units "W"@en;
  skos:broader ontolidar:UninterruptiblePowerSupply;
  skos:definition "Lidar working power provided by the UPS when working off-line."@en,
    "Potencia de trabajo lidar proporcionada por el sistema de alimentación ininterrumpida cuando el lidar trabaja desconectado de la red eléctrica."@es,
    "Potenza emessa dal gruppo di continuità per garantire l'operabilità del lidar quando disconnesso dalla rete elettrica."@it,
    "在未接电网工作时，不间断电源提供给激光雷达的电功率"@cn;
  skos:inScheme <http://vocab.ieawindtask32.org/wind-lidar-ontology/>;
  skos:prefLabel "Potenza"@it, "UPS battery power"@en, "UPS电池功率"@cn, "USV-Batteriebetrieb"@de .

ontolidar:UpsBatteryIntensity a skos:Concept;
  ontolidar:units "A"@en;
  skos:broader ontolidar:UninterruptiblePowerSupply;
  skos:definition "Intensidad de la corriente de trabajo lidar proporcionada por el sistema de alimentación ininterrumpida cuando el lidar trabaja desconectado de la red eléctrica."@es,
    "Intensità della corrente elettrica provvigionata dal gruppo di continuità."@it, "Lidar working current intensity provided by the UPS when working off-line."@en,
    "在未接电网工作时，不间断电源提供的激光雷达工作电流强度"@cn;
  skos:inScheme <http://vocab.ieawindtask32.org/wind-lidar-ontology/>;
  skos:prefLabel "Intensità"@it, "UPS battery intensity"@en, "UPS电池强度"@cn, "USV-Batterieintensität"@de .

ontolidar:ScannerModule a skos:Concept;
  skos:broader ontolidar:Design;
  skos:definition "El escáner orienta el rayo láser con respecto al alojamiento y otros elementos del sistema. El escáner puede tener uno o más grados de libertad."@es,
    "Modulo che muove il fascio laser rispetto all'asse principale ed alle altre parti del sistema. Può essere dotato di uno o più gradi di libertà."@it,
    "The scanner orients the beam with respect to the housing and other parts of the lidar system. The scanner may be capable of one or more degrees of freedom."@en,
    "扫描器使光束相对于外壳和激光雷达系统的其他部分定向。扫描仪可以有一个或多个自由度。"@cn;
  skos:editorialNote "Definición basada en el proyecto OpenLidar: https://github.com/e-WindLidar/OpenLidarModuleDefinitions"@es,
    "Definition based on the OpenLidar module definitions at https://github.com/e-WindLidar/OpenLidarModuleDefinitions"@en,
    "Definizione basata sulla definizione di modulo del progetto OpenLidar. Vedasi https://github.com/e-WindLidar/OpenLidarModuleDefinitions"@it;
  skos:inScheme <http://vocab.ieawindtask32.org/wind-lidar-ontology/>;
  skos:narrower ontolidar:ScannerAzimuthPositioningServo, ontolidar:ScannerElevationPositioningServo,
    ontolidar:ScannerMirrors, ontolidar:ScanningSampleRate;
  skos:prefLabel "Componente di scansione"@it, "Módulo del escáner"@es, "Scanner module"@en,
    "Scanner-Modul"@de, "扫描器模块"@cn;
  skos:related ontolidar:ScanGeometry .

ontolidar:ScannerAzimuthPositioningServo a skos:Concept;
  skos:broader ontolidar:ScannerModule;
  skos:definition "El servomotor ayimutal gestiona el escáner en la dirección azimutal."@es,
    "Servomotore dedicato a muovere il modulo di scansione nel piano azimutale."@it, "The azimuth servo motor that drives the scanner in the azimuthal direction."@en,
    "方位角伺服马达驱动扫描器在方位角方向上变化。"@cn;
  skos:inScheme <http://vocab.ieawindtask32.org/wind-lidar-ontology/>;
  skos:narrower ontolidar:AzimuthAngle, ontolidar:AzimuthSlewRate;
  skos:prefLabel "Azimut-Positionierservo des Scanners"@de, "Scanner azimuth positioning servo"@en,
    "Servomotor de posicionamiento azimut del escáner"@es, "Servomotore per la scansione nella direzione azimutale"@it,
    "扫描器方位定位伺服"@cn .

ontolidar:AzimuthAngle a skos:Concept;
  ontolidar:units "degrees"@en;
  skos:altLabel "Azimuth"@en;
  skos:broader ontolidar:ScannerAzimuthPositioningServo;
  skos:definition "Angulo subtendido entre la línea de visión (line-of-sight o LOS, por sus siglas en inglés) del lidar y el vector de referencia del plano de referencia."@es,
    "L'angolo fra la direzione del fascio laser ed un vettore di riferimento in un piano di riferimento."@it,
    "The angle between the line of sight of the lidar and a reference vector on the reference coordinate system."@en,
    "激光雷达的视线与基准平面上的参考向量之间的夹角。"@cn;
  skos:editorialNote "El vector de referencia desde el que se define el ángulo azimut es a menudo el eje de coordenadas correspondiente al norte geográfico, pero cualquier otra definición es válida siempre y cuando la definición del sistema de coordenadas sea consistente."@es,
    "Il vettore di riferimento dell'angolo di azimith è spesso quello che indica il nord geografico. Un qualsiasi altro vettore, in realtà, potrebbe analogamente servire allo scopo."@it,
    "The reference vector from which the azimuth is defined is often true north, but could be some other defined vector."@en;
  skos:inScheme <http://vocab.ieawindtask32.org/wind-lidar-ontology/>;
  skos:prefLabel "Azimut"@es, "Azimut"@it, "Azimut-Winkel"@de, "Azimuth angle"@en, "方位角"@cn .

ontolidar:AzimuthSlewRate a skos:Concept;
  ontolidar:units "degrees per second"@en;
  skos:broader ontolidar:ScannerAzimuthPositioningServo;
  skos:definition "Massima velocità di operazione del servomotore nel piano azimutale."@it,
    "The maximum rate of operation of the servo motor in the azimuthal direction."@en,
    "Velocidad máxima de funcionamiento del servomotor en la dirección azimutal."@es,
    "伺服电机在方位角方向的最大运行速率"@cn;
  skos:inScheme <http://vocab.ieawindtask32.org/wind-lidar-ontology/>;
  skos:prefLabel "Azimut-Anstiegsrate"@de, "Azimuth slew rate"@en, "Velocidad de giro azimutal"@es,
    "Velocità massima azimutale"@it, "方位角回转率"@cn .

ontolidar:ScannerElevationPositioningServo a skos:Concept;
  skos:broader ontolidar:ScannerModule;
  skos:definition "El servomotor de elevación acciona el escáner en la dirección de elevación."@es,
    "Servomotore dedicato a modificare l'altezza sull'orizzonte del fascio laser."@it,
    "The elevation servo motor that drives the scanner in the elevation direction."@en,
    "仰角伺服电机在仰角方向驱动扫描仪"@cn;
  skos:inScheme <http://vocab.ieawindtask32.org/wind-lidar-ontology/>;
  skos:narrower ontolidar:ElevationAngle, ontolidar:ElevationSlewRate;
  skos:prefLabel "Scanner Höhenpositionierungsservo"@de, "Scanner elevation positioning servo"@en,
    "Servomotor del posicionamiento de elevación del escáner"@es, "Servomotore per la scansione nella direzione di elevazione"@it,
    "扫描仪仰角定位伺服"@cn .

ontolidar:ElevationAngle a skos:Concept;
  ontolidar:units "degrees"@en;
  skos:altLabel "Elevation"@en;
  skos:broader ontolidar:ScannerElevationPositioningServo;
  skos:definition "Angulo subtendido entre la línea de visión (line-of-sight o LOS, por sus siglas en inglés) del lidar y el plano de referencia."@es,
    "L'angolo fra la direzione del fascio laser e un piano di riferimento."@it, "The angle between the line of sight of the lidar and the reference coordinate system."@en,
    "激光雷达的视线与基准平面之间的夹角。"@cn;
  skos:inScheme <http://vocab.ieawindtask32.org/wind-lidar-ontology/>;
  skos:prefLabel "Elevación"@es, "Elevation angle"@en, "Elevationswinkel"@de, "Elevazione"@it,
    "仰角"@cn .

ontolidar:ElevationSlewRate a skos:Concept;
  ontolidar:units "degrees per second"@en;
  skos:broader ontolidar:ScannerElevationPositioningServo;
  skos:definition "Massima velocità di modifica dell'altezza del fascio laser."@it,
    "The maximum rate of operation of the servo motor in the elevation direction."@en,
    "Velocidad máxima de funcionamiento del servomotor en la dirección de elevación."@es,
    "伺服电机在仰角方向的最大运行速率"@cn;
  skos:inScheme <http://vocab.ieawindtask32.org/wind-lidar-ontology/>;
  skos:prefLabel "Elevation slew rate"@en, "Höhenanstiegsrate"@de, "Velocidad de giro de elevación"@es,
    "Velocità massima di elevazione"@it, "仰角回转率"@cn .

ontolidar:ScannerMirrors a skos:Concept;
  skos:altLabel "ScanModule"@en;
  skos:broader ontolidar:ScannerModule;
  skos:definition "Espejos destinados a modificar la trayectoria del haz entre el telescopio y la atmósfera."@es,
    "Scanner components intended to modify the beam trajectories of both, the laser beam and the backscattered one. The scanner mirrors steer the outgoing beam towards the atmosphere and the backscattered incoming beam towards the receiver. Usually,some of these mirrors are coupled with servo motors, enabling the lidar to perform measurements in differents orientations by varying the mirror angles."@en,
    "Specchi per modificare il cammino ottico del fascio laser fra il telescopio e l'atmosfera esterna."@it,
    "修改望远镜和大气层之间光束路径的镜子。"@cn;
  skos:inScheme <http://vocab.ieawindtask32.org/wind-lidar-ontology/>;
  skos:prefLabel "Scanner mirrors"@en, "Scanner-Spiegel"@de, "Specchi dello scanner"@it,
    "扫描镜"@cn .

ontolidar:ScanningSampleRate a skos:Concept;
  rdfs:label "Hz"@en;
  skos:broader ontolidar:ScannerModule;
  skos:definition "Frecuencia del patrón de escaneo. Tiempo que tarda en completarse un patrón de escaneo."@es,
    "Frequency of the scanning pattern. Time the scanner takes to complete a measuring pattern."@en,
    "Frequenza della sequenza di scansionamento. Tempo che lo scanner impiega per concludere un ciclo."@it,
    "扫描模式的频率，即扫描器完成一次扫描采样所需的时间"@cn;
  skos:inScheme <http://vocab.ieawindtask32.org/wind-lidar-ontology/>;
  skos:prefLabel "Frequenza di campionamento"@it, "Scan-Abtastrate"@de, "Scanning sample rate"@en,
    "Tasa de muestreo del escáner"@es, "扫描采样率"@cn .

ontolidar:InterlocksModule a skos:Concept;
  skos:broader ontolidar:Design;
  skos:definition "Las interconexiones son un conjunto de sistemas de seguridad instalados a lo largo de los componentes del lidar que impiden o mitigan las actividades potencialmente peligrosas."@es,
    "Meccanismi di sicurezza diffusi nel sistema lidar, atti a prevenire o mitigare le conseguenze di possibili malfunzionamenti."@it,
    "The interlocks are a dispersed set of safety systems that prevent or mitigate potentially dangerous activities."@en,
    "联锁装置是一组分散的安全系统，可防止或降低潜在的危险。"@cn;
  skos:editorialNote "Definición basada en el proyecto OpenLidar: https://github.com/e-WindLidar/OpenLidarModuleDefinitions"@es,
    "Definition based on the OpenLidar module definitions at https://github.com/e-WindLidar/OpenLidarModuleDefinitions"@en,
    "Definizione basata sulla definizione di modulo del progetto OpenLidar. Vedasi https://github.com/e-WindLidar/OpenLidarModuleDefinitions"@it;
  skos:inScheme <http://vocab.ieawindtask32.org/wind-lidar-ontology/>;
  skos:prefLabel "Dispositivi di sicurezza"@it, "Dispositivos de seguidad"@es, "Interlocks module"@en,
    "Verriegelungs-Modul"@de, "安全联锁"@cn .

ontolidar:Devices a skos:Concept;
  skos:definition "Implementaciones específicas de la tecnología del lidar de viento."@es,
    "Particolari realizzazioni di tecnologie lidar per applicazioni eoliche. Quelle che ci sono venute in mente di prim'acchito."@it,
    "Specific implementations of wind lidar technologies. The ones that we thought off first."@en,
    "测风激光雷达技术的具体实现设备。"@cn;
  skos:editorialNote "Envíe por favor información relativa al dispositivo que no esté presente en esta lista todavía."@es,
    "Per favore, inviate informazioni relative a sistemi non presenti in questa lista."@it,
    "Please send info for the devices not present in this list yet."@en;
  skos:inScheme <http://vocab.ieawindtask32.org/wind-lidar-ontology/>;
  skos:narrower ontolidar:Epsiline, ontolidar:GalionG250, ontolidar:Halophotonics, ontolidar:Leice,
    ontolidar:Movelaser, ontolidar:Vindicator, ontolidar:WindarPhotonics, ontolidar:Windcube,
    ontolidar:Windscanner, ontolidar:Zephir;
  skos:note "Per favore, inviate informazioni sui devices che volete vedere inclusi in questa lista."@it;
  skos:prefLabel "Devices"@en, "Dispositivi lidar"@it, "Dispositivos"@es, "Geräte"@de,
    "设备"@cn;
  skos:topConceptOf <http://vocab.ieawindtask32.org/wind-lidar-ontology/> .

ontolidar:Windscanner a skos:Concept;
  skos:broader ontolidar:Devices;
  skos:definition "One of many different types of system that can be used to perform convergent scan geometries. Originally referred to the DTU-led windscanner.eu project."@en,
    "Uno de los varios tipos de sistemas que se pueden utilizar para realizar escaneos de geometría convergente. Originariamente hace referencia al proyecto windscanner.eu de DTU."@es,
    "Uno dei vari tipi di sistemi che possono essere utilizzati per effettuare scansioni su geometrie convergenti. Originariamente noto come il progetto windscanner.eu project di DTU."@it,
    "一种激光雷达测风系统，可用于进行会聚扫描的几何形状。最初是指DTU领导的winddscanner.eu项目。"@cn;
  skos:inScheme <http://vocab.ieawindtask32.org/wind-lidar-ontology/>;
  skos:prefLabel "Escáner de viento"@es, "Lidar 'WindScanner'"@it, "Windscanner"@de,
    "Windscanner"@en, "Windscanner测风雷达"@cn .

ontolidar:Windcube a skos:Concept;
  skos:broader ontolidar:Devices;
  skos:definition "Famiglia di lidars prodotti da Leosphere - a Vaisala company. Per maggiori informazioni, visitare https://www.vaisala.com/en/wind-lidars/wind-energy."@it,
    "Familia de lidares de viento producidos por Leosphere - a Vaisala company. Véase: https://www.vaisala.com/en/wind-lidars/wind-energy"@es,
    "Family of wind lidars produced by Leosphere - a Vaisala company. Please refer to https://www.vaisala.com/en/wind-lidars/wind-energy."@en,
    "Leosphere--Vaisala公司生产的风速仪系列。请参考https://www.vaisala.com/en/wind-lidars/wind-energy。"@cn;
  skos:inScheme <http://vocab.ieawindtask32.org/wind-lidar-ontology/>;
  skos:narrower ontolidar:WindcubeNacelle, ontolidar:WindcubeScan, ontolidar:Windcubev2;
  skos:prefLabel "Lidar 'WindCube'"@it, "WindCube"@es, "Windcube"@cn, "Windcube"@de,
    "Windcube"@en .

ontolidar:Windcubev2 a skos:Concept;
  skos:broader ontolidar:Windcube;
  skos:definition "Lidar verticale prodotto da Leosphere - a Vaisala company."@it, "Perfilador vertical producido por Leosphere - a Vaisala company."@es,
    "Vertical profiler manufactured by Leosphere - a Vaisala company."@en, "由维萨拉公司的Leosphere公司生产的垂直剖面仪。"@cn;
  skos:inScheme <http://vocab.ieawindtask32.org/wind-lidar-ontology/>;
  skos:prefLabel "Lidar 'WindCube'"@it, "WindCube"@es, "Windcube"@cn, "WindcubeV2"@de,
    "WindcubeV2"@en .

ontolidar:WindcubeScan a skos:Concept;
  skos:broader ontolidar:Windcube;
  skos:definition "Lidar de largo alcance producido por Leosphere - a Vaisala company."@es,
    "Long range scannig lidar manufactured by Leosphere - a Vaisala company."@en, "Scanner a lungo raggio prodotto da Leosphere - a Vaisala company."@it,
    "由Leosphere-维萨拉公司生产的长距离扫描激光雷达。"@cn;
  skos:inScheme <http://vocab.ieawindtask32.org/wind-lidar-ontology/>;
  skos:prefLabel "Lidar 'WindCube Scan'"@it, "WindCube Scan"@cn, "WindCube Scan"@de,
    "WindCube Scan"@en, "WindCube Scan"@es .

ontolidar:WindcubeNacelle a skos:Concept;
  skos:broader ontolidar:Windcube;
  skos:definition "Lidar de góndola producido por Leosphere - a Vaisala company."@es,
    "Lidar per navicella prodotto da Leosphere - a Vaisala company."@it, "Nacelle mounted lidar manufactured by Leosphere - a Vaisala company."@en,
    "由Leosphere--一家Vaisala公司制造的安装在机舱内的激光雷达。"@cn;
  skos:inScheme <http://vocab.ieawindtask32.org/wind-lidar-ontology/>;
  skos:prefLabel "Lidar 'WindCube Nacelle'"@it, "WindCube Nacelle"@cn, "WindCube Nacelle"@de,
    "WindCube Nacelle"@en, "WindCube Nacelle"@es .

ontolidar:Zephir a skos:Concept;
  skos:broader ontolidar:Devices;
  skos:definition "Famiglia di lidars prodotti da ZX lidars. Per maggiori informazioni, visitare https://www.zxlidars.com/our-wind-lidars/"@it,
    "Familia de lidares de viento producidos por Leosphere - a Vaisala company. Véase: https://www.zxlidars.com/our-wind-lidars/"@es,
    "Family of wind lidars produced by ZX lidars. Please refer to https://www.zxlidars.com/our-wind-lidars/."@en,
    "由ZX激光雷达公司生产的风力激光雷达家族。请参考https://www.zxlidars.com/our-wind-lidars/。"@cn;
  skos:inScheme <http://vocab.ieawindtask32.org/wind-lidar-ontology/>;
  skos:narrower ontolidar:Zx300, ontolidar:Zxtm;
  skos:prefLabel "Lidar 'Zephir'"@it, "Zephir"@cn, "Zephir"@de, "Zephir"@en, "Zephir"@es .

ontolidar:Zx300 a skos:Concept;
  skos:broader ontolidar:Zephir;
  skos:definition "Perfilador vertical producido por ZX lidars."@es, "Seconda generazione di lidar verticali compatti prodotti da ZX lidars."@it,
    "Vertical profiler manufactured by ZX lidars."@en, "由ZX激光雷达公司制造的垂直剖面仪。"@cn;
  skos:inScheme <http://vocab.ieawindtask32.org/wind-lidar-ontology/>;
  skos:prefLabel "Lidar 'ZX300'"@it, "ZX300"@cn, "ZX300"@de, "ZX300"@en, "ZX300"@es .

ontolidar:Zxtm a skos:Concept;
  skos:broader ontolidar:Zephir;
  skos:definition "Lidar de góndola producido por ZX lidars."@es, "Lidar per navicella prodotto da ZX lidars."@it,
    "Nacelle mounted lidar manufactured by ZX lidars."@en, "由ZX激光雷达公司制造的机舱安装激光雷达。"@cn;
  skos:inScheme <http://vocab.ieawindtask32.org/wind-lidar-ontology/>;
  skos:prefLabel "Lidar 'ZXTM'"@it, "ZXTM"@cn, "ZXTM"@de, "ZXTM"@en, "ZXTM"@es .

ontolidar:WindarPhotonics a skos:Concept;
  skos:broader ontolidar:Devices;
  skos:definition "Famiglia di lidars prodotti da Windar Photonics. Per maggiori informazioni, visitare https://www.windarphotonics.com/."@it,
    "Familia de lidares de viento producidos por Windar Photonics. Véase: https://www.windarphotonics.com/"@es,
    "Family of wind lidars produced by Windar Photonics. Please refer to https://www.windarphotonics.com/."@en,
    "Windar Photonics公司生产的风雷达系列。请参考https://www.windarphotonics.com/。"@cn;
  skos:inScheme <http://vocab.ieawindtask32.org/wind-lidar-ontology/>;
  skos:narrower ontolidar:WindEye, ontolidar:WindVision;
  skos:prefLabel "Lidar 'Windar Photonics'"@it, "Windar Photonics"@cn, "Windar Photonics"@de,
    "Windar Photonics"@en, "Windar Photonics"@es .

ontolidar:WindEye a skos:Concept;
  skos:broader ontolidar:WindarPhotonics;
  skos:definition "Lidar de góndola producido por Windar Photonics."@es, "Lidar per navicella prodotto da Windar Photonics."@it,
    "Nacelle mounted lidar manufactured by Windar Photonics."@en, "Windar Photonics公司生产的机舱式激光雷达。"@cn;
  skos:inScheme <http://vocab.ieawindtask32.org/wind-lidar-ontology/>;
  skos:prefLabel "Lidar 'Wind Eye'"@it, "Wind Eye"@cn, "Wind Eye"@en, "Wind Eye"@es,
    "Windauge"@de .

ontolidar:WindVision a skos:Concept;
  skos:broader ontolidar:WindarPhotonics;
  skos:definition "Lidar de góndola producido por Windar Photonics."@es, "Lidar per navicella prodotto da Windar Photonics."@it,
    "Nacelle mounted lidar manufactured by Windar Photonics."@en, "Windar Photonics公司生产的机舱激光雷达。"@cn;
  skos:inScheme <http://vocab.ieawindtask32.org/wind-lidar-ontology/>;
  skos:prefLabel "Lidar 'Wind Vision'"@it, "Wind Vision"@cn, "Wind Vision"@en, "Wind Vision"@es,
    "Wind-Vision"@de .

ontolidar:Epsiline a skos:Concept;
  skos:broader ontolidar:Devices;
  skos:definition "Epsiline公司生产的风雷达系列。请参考http://www.epsiline.com/。"@cn, "Famiglia di lidars prodotti da Epsiline. Per maggiori informazioni, visitare http://www.epsiline.com/."@it,
    "Familia de lidares de viento producidos por Epsiline. Véase: http://www.epsiline.com/"@es,
    "Family of wind lidars produced by Epsiline. Please refer to http://www.epsiline.com/."@en;
  skos:inScheme <http://vocab.ieawindtask32.org/wind-lidar-ontology/>;
  skos:narrower ontolidar:WindEagle;
  skos:prefLabel "Epsiline"@cn, "Epsiline"@en, "Epsiline"@es, "Lidar 'Epsiline'"@de,
    "Lidar 'Epsiline'"@it .

ontolidar:WindEagle a skos:Concept;
  skos:broader ontolidar:Epsiline;
  skos:definition "Epsiline公司生产的机舱激光雷达。"@cn, "Lidar de góndola producido por Epsiline."@es,
    "Lidar per navicella prodotto da Epsiline."@it, "Nacelle mounted lidar manufactured by Epsiline."@en;
  skos:inScheme <http://vocab.ieawindtask32.org/wind-lidar-ontology/>;
  skos:prefLabel "Lidar 'Wind Eagle'"@de, "Lidar 'Wind Eagle'"@it, "Wind Eagle"@cn,
    "Wind Eagle"@en, "Wind Eagle"@es .

ontolidar:Movelaser a skos:Concept;
  skos:broader ontolidar:Devices;
  skos:definition "Famiglia di lidars prodotti da Nanjing MoveLaser. Per maggiori informazioni, visitare https://mgwtradenservice.com.au/wind-measurement-lidars/."@it,
    "Familia de lidares de viento producidos por Nanjing MoveLaser. Véase: https://mgwtradenservice.com.au/wind-measurement-lidars/"@es,
    "Family of wind lidars produced by Nanjing MoveLaser. Please refer to https://mgwtradenservice.com.au/wind-measurement-lidars/."@en,
    "南京MoveLaser公司生产的风雷达家族。请参考https://mgwtradenservice.com.au/wind-measurement-lidars/。"@cn;
  skos:inScheme <http://vocab.ieawindtask32.org/wind-lidar-ontology/>;
  skos:prefLabel "Lidar 'MoveLaser'"@de, "Lidar 'MoveLaser'"@it, "MoveLaser"@cn, "MoveLaser"@en,
    "MoveLaser"@es .

ontolidar:MolasB300 a skos:Concept;
  skos:broader ontolidar:MoveLaser;
  skos:definition "Lidar verticale prodotto da Nanjing MoveLaser."@it, "Perfilador vertical producido por Nanjing MoveLaser."@es,
    "Vertical profiler manufactured by Nanjing MoveLaser."@en, "南京MoveLaser公司生产的垂直剖面仪。"@cn;
  skos:inScheme <http://vocab.ieawindtask32.org/wind-lidar-ontology/>;
  skos:prefLabel "Lidar 'Molas B300'"@de, "Lidar 'Molas B300'"@it, "Molas B300"@cn,
    "Molas B300"@en, "Molas B300"@es .

ontolidar:MolasNl a skos:Concept;
  skos:broader ontolidar:MoveLaser;
  skos:definition "Lidar de góndola producido por Nanjing MoveLaser."@es, "Lidar per navicella prodotto da Nanjing MoveLaser."@it,
    "Nacelle mounted lidar manufactured by Nanjing MoveLaser."@en, "南京MoveLaser公司生产的机舱式激光雷达。"@cn;
  skos:inScheme <http://vocab.ieawindtask32.org/wind-lidar-ontology/>;
  skos:prefLabel "Lidar 'Molas NL'"@it, "Molas NL"@cn, "Molas NL"@de, "Molas NL"@en,
    "Molas NL"@es .

ontolidar:Leice a skos:Concept;
  skos:broader ontolidar:Devices;
  skos:definition "Famiglia di lidars prodotti da Leice. Per maggiori informazioni, visitare http://www.leice-lidar.com/en/index.html."@it,
    "Familia de lidares de viento producidos por Leice. Véase: http://www.leice-lidar.com/en/index.html"@es,
    "Family of wind lidars produced by Leice. Please refer to http://www.leice-lidar.com/en/index.html."@en,
    "Leice公司生产的风向激光雷达系列。请参考http://www.leice-lidar.com/en/index.html。"@cn;
  skos:inScheme <http://vocab.ieawindtask32.org/wind-lidar-ontology/>;
  skos:narrower ontolidar:Wind3D, ontolidar:Windhorizon, ontolidar:Windmast;
  skos:prefLabel "Leice"@cn, "Leice"@en, "Leice"@es, "Lidar 'Leice'"@de, "Lidar 'Leice'"@it .

ontolidar:Windmast a skos:Concept;
  skos:broader ontolidar:Leice;
  skos:definition "Lidar verticale prodotto da Leice."@it, "Perfilador vertical producido por Leice."@es,
    "Vertical profiler manufactured by Leice."@en, "莱斯公司生产的垂直剖面仪。"@cn;
  skos:inScheme <http://vocab.ieawindtask32.org/wind-lidar-ontology/>;
  skos:prefLabel "Lidar 'WindMast'"@it, "WindMast"@cn, "WindMast"@de, "WindMast"@en,
    "WindMast"@es .

ontolidar:Windhorizon a skos:Concept;
  skos:broader ontolidar:Leice;
  skos:definition "Lidar de góndola producido por Leice."@es, "Lidar per navicella prodotto da Leice."@it,
    "Nacelle mounted lidar manufactured by Leice."@en, "莱斯公司生产的机舱式激光雷达。"@cn;
  skos:inScheme <http://vocab.ieawindtask32.org/wind-lidar-ontology/>;
  skos:prefLabel "Lidar 'WindHorizon'"@it, "WindHorizon"@cn, "WindHorizon"@de, "WindHorizon"@en,
    "WindHorizon"@es .

ontolidar:Wind3D a skos:Concept;
  skos:broader ontolidar:Leice;
  skos:definition "Lidar de escaneo producido por Leice."@es, "Scanner a lungo raggio prodotto da Leice."@it,
    "Scanning lidar manufactured by Leice."@en, "莱斯公司生产的扫描激光雷达。"@cn;
  skos:inScheme <http://vocab.ieawindtask32.org/wind-lidar-ontology/>;
  skos:prefLabel "Lidar 'Wind3D'"@it, "Wind3D"@cn, "Wind3D"@de, "Wind3D"@en, "Wind3D"@es .

ontolidar:Halophotonics a skos:Concept;
  skos:broader ontolidar:Devices;
  skos:definition "Famiglia di lidars prodotti da HaloPhotonics. Per maggiori informazioni, visitare https://halo-photonics.com/."@it,
    "Familia de lidares de viento producidos por HaloPhotonics. Véase: https://halo-photonics.com/"@es,
    "Family of wind lidars produced by HaloPhotonics. Please refer to https://halo-photonics.com/."@en,
    "HaloPhotonics公司生产的风雷达系列。请参考https://halo-photonics.com/。"@cn;
  skos:inScheme <http://vocab.ieawindtask32.org/wind-lidar-ontology/>;
  skos:prefLabel "HaloPhotonics"@cn, "HaloPhotonics"@en, "HaloPhotonics"@es, "HaloPhotonik"@de,
    "Lidar 'HaloPhotonics'"@it .

ontolidar:Windpro a skos:Concept;
  skos:broader ontolidar:HaloPhotonics;
  skos:definition "HaloPhotonics公司生产的垂直剖面仪。"@cn, "Lidar verticale prodotto da Halophotonics."@it,
    "Perfilador vertical producido por Halo Photonics."@es, "Vertical profiler manufactured by HaloPhotonics."@en;
  skos:inScheme <http://vocab.ieawindtask32.org/wind-lidar-ontology/>;
  skos:prefLabel "Lidar 'WindMast'"@it, "WindMast"@es, "WindPro"@cn, "WindPro"@de, "WindPro"@en .

ontolidar:Verticalpro a skos:Concept;
  skos:broader ontolidar:HaloPhotonics;
  skos:definition "HaloPhotonics公司生产的垂直剖面仪。"@cn, "Lidar verticale prodotto da Halophotonics."@it,
    "Perfilador vertical producido por Halo Photonics."@es, "Vertical profiler manufactured by HaloPhotonics."@en;
  skos:inScheme <http://vocab.ieawindtask32.org/wind-lidar-ontology/>;
  skos:prefLabel "Lidar 'VerticalPro'"@it, "VerticalPro"@cn, "VerticalPro"@de, "VerticalPro"@en,
    "VerticalPro"@es .

ontolidar:Streamline a skos:Concept;
  skos:broader ontolidar:HaloPhotonics;
  skos:definition "HaloPhotonics公司生产的扫描激光雷达。"@cn, "Lidar de escaneo producido por Halo Photonics."@es,
    "Scanner a lungo raggio prodotto da HaloPhotonics."@it, "Scanning lidar manufactured by HaloPhotonics."@en;
  skos:inScheme <http://vocab.ieawindtask32.org/wind-lidar-ontology/>;
  skos:prefLabel "Lidar 'StreamLine'"@it, "StreamLine"@cn, "StreamLine"@en, "StreamLine"@es,
    "Stromlinie"@de .

ontolidar:GalionG250 a skos:Concept;
  skos:broader ontolidar:Devices;
  skos:definition "Famiglia di lidars prodotti da Galion. Per maggiori informazioni, visitare https://www.woodplc.com/solutions/expertise/a-z-list-of-our-expertise/software-and-products/galion-lidar-unit."@it,
    "Familia de lidares de viento producidos por Wood. Véase: https://www.woodplc.com/solutions/expertise/a-z-list-of-our-expertise/software-and-products/galion-lidar-unit"@es,
    "Family of wind lidars produced by Wood. Please refer to https://www.woodplc.com/solutions/expertise/a-z-list-of-our-expertise/software-and-products/galion-lidar-unit"@en,
    "伍德公司生产的风力激光雷达系列。请参考https://www.woodplc.com/solutions/expertise/a-z-list-of-our-expertise/software-and-products/galion-lidar-unit"@cn;
  skos:inScheme <http://vocab.ieawindtask32.org/wind-lidar-ontology/>;
  skos:prefLabel "Galion G250"@cn, "Galion G250"@de, "Galion G250"@en, "Galion G250"@es,
    "Galion G250"@it .

ontolidar:GalionScanningLidarG4000 a skos:Concept;
  skos:broader ontolidar:Galion;
  skos:definition "Familia de lidares de viento producidos por Wood. Véase: https://www.woodplc.com/solutions/expertise/a-z-list-of-our-expertise/software-and-products/galion-lidar-unit"@es,
    "Family of wind lidars produced by Wood. Please refer to https://www.woodplc.com/solutions/expertise/a-z-list-of-our-expertise/software-and-products/galion-lidar-unit."@en,
    "Scanner a lungo raggio prodotto da Galion. Per maggiori informazioni, visitare https://www.woodplc.com/solutions/expertise/a-z-list-of-our-expertise/software-and-products/galion-lidar-unit"@it,
    "伍德公司生产的风向激光雷达家族。请参考https://www.woodplc.com/solutions/expertise/a-z-list-of-our-expertise/software-and-products/galion-lidar-unit"@cn;
  skos:inScheme <http://vocab.ieawindtask32.org/wind-lidar-ontology/>;
  skos:prefLabel "Galion Scanning Lidar G4000"@cn, "Galion Scanning Lidar G4000"@de,
    "Galion Scanning Lidar G4000"@en, "Galion Scanning Lidar G4000"@es, "Galion Scanning Lidar G4000"@it .

ontolidar:Vindicator a skos:Concept;
  skos:broader ontolidar:Devices;
  skos:definition "Catch the Wind https://news.softpedia.com/news/A-Good-Mix-LIDAR-and-Wind-Turbines-138511.shtml"@en,
    "Catch the Wind https://news.softpedia.com/news/A-Good-Mix-LIDAR-and-Wind-Turbines-138511.shtml"@it,
    "Catch the Wind: https://news.softpedia.com/news/A-Good-Mix-LIDAR-and-Wind-Turbines-138511.shtml"@es,
    "捕捉风https://news.softpedia.com/news/A-Good-Mix-LIDAR-and-Wind-Turbines-138511.shtml"@cn;
  skos:inScheme <http://vocab.ieawindtask32.org/wind-lidar-ontology/>;
  skos:prefLabel "Lidar Vindicator'"@de, "Lidar Vindicator'"@it, "Vindicator"@cn, "Vindicator"@en .

ontolidar:Instances a skos:Concept;
  skos:definition "Cada uno de los objetos lidar."@es, "Each single wind lidar object."@en,
    "Ogni singolo esemplare di lidar eolici."@it, "测风激光雷达实例"@cn;
  skos:inScheme <http://vocab.ieawindtask32.org/wind-lidar-ontology/>;
  skos:narrower <http://vocab.ieawindtask32.org/wind-lidar-ontology/LidarType(ExtendedDefinition)>,
    <http://vocab.ieawindtask32.org/wind-lidar-ontology/SerialNumber(ExtendedDefinition)>;
  skos:prefLabel "Esempi di lidars"@it, "Instances"@en, "Instancias"@es, "Instanzen"@de,
    "激光雷达示例"@cn;
  skos:topConceptOf <http://vocab.ieawindtask32.org/wind-lidar-ontology/> .

<http://vocab.ieawindtask32.org/wind-lidar-ontology/SerialNumber(ExtendedDefinition)>
  a skos:Concept;
  skos:broader ontolidar:Instances;
  skos:definition "Numero di serie univoco identificativo del lidar."@it, "Número de serie del lidar de viento."@es,
    "Unique identification number for each wind lidar."@en, "测风激光雷达序列号"@cn;
  skos:inScheme <http://vocab.ieawindtask32.org/wind-lidar-ontology/>;
  skos:prefLabel "Numero seriale"@it, "Número de serie"@es, "Serial number (extended definition)"@en,
    "Seriennummer (erweiterte Definition)"@de, "序列号"@cn .

<http://vocab.ieawindtask32.org/wind-lidar-ontology/LidarType(ExtendedDefinition)>
  a skos:Concept;
  skos:broader ontolidar:Instances;
  skos:definition "The type of lidar device (ground based, nacelle mounted, etc)."@en,
    "Tipo de dispositivo lidar."@es, "Tipologia di lidar (verticale, da navicella, etc)."@it,
    "激光雷达设备类型"@cn;
  skos:inScheme <http://vocab.ieawindtask32.org/wind-lidar-ontology/>;
  skos:prefLabel "Lidar type (extended definition)"@en, "Lidar-Typ (erweiterte Definition)"@de,
    "Tipo de lidar"@es, "Tipologia di lidar"@it, "激光雷达类型"@cn;
  skos:related ontolidar:Devices .

ontolidar:DataProcessing a skos:Concept;
  skos:definition "Métodos aplicables a los datos lidar para extraer información útil."@es,
    "Processo di estrazione di informazioni utili dai dati grezzi di un lidar."@it, "Ways that wind lidar data can be processed to extract useful data."@en,
    "通过测风激光雷达数据处理，提取有用的数据信息"@cn;
  skos:inScheme <http://vocab.ieawindtask32.org/wind-lidar-ontology/>;
  skos:narrower ontolidar:CoordinateSystemTransformation, ontolidar:DataFiltering, ontolidar:RadialVelocity,
    ontolidar:WindfieldReconstruction;
  skos:prefLabel "Data processing"@en, "Datenverarbeitung"@de, "Processamento dati"@it,
    "数据处理"@cn;
  skos:topConceptOf <http://vocab.ieawindtask32.org/wind-lidar-ontology/> .

ontolidar:RadialVelocity a skos:Concept;
  skos:altLabel "Radial wind speed"@en;
  skos:broader ontolidar:DataProcessing;
  skos:definition "The radial velocity is the projection of the wind velocity vector onto the line of sight, directly measured by observing the Doppler shift of the backscattered laser pulse emitted along the line of sight."@en,
    "Una misurazione intermedia (vedasi intermediate data), specificamente la componente del vettore velocità del vento nella direzione del raggio laser emesso dal lidar (line of sight). La sua derivazione è immediata a partire dalla misurazione dello shift Doppler del raggio riflesso dall'atmosfera rispetto alla frequenza del raggio emesso dal lidar."@it,
    "Variable intermedia (véase datos intermedios). La velocidad radial es la componente radial del vector de velicidad del viento, relativo a la localización del lidar que realiza la medida. Es la proyección del vector de velocidad del viento sobrel la línea de visión (line-of-sight o LOS, por sus siglas en inglés) medida directamente mediante la observación del desplazamiento Doppler del pulso láser retrodispersado, y que fue previamente emitido a lo largo de la línea de visión."@es,
    "径向速度是风速矢量在激光雷达视线方向上的投影，通过分析沿视线方向激光反射脉冲产生的多普勒频移直接获得"@cn;
  skos:inScheme <http://vocab.ieawindtask32.org/wind-lidar-ontology/>;
  skos:narrower ontolidar:DopplerSpectra;
  skos:prefLabel "Radial velocity"@en, "Radialgeschwindigkeit"@de, "Velocidad radial"@es,
    "Velocità radiale"@it, "径向速率"@cn .

ontolidar:DopplerSpectra a skos:Concept;
  skos:broader ontolidar:RadialVelocity;
  skos:definition "Distribución de frecuencias de la potencia de la señal recibida."@es,
    "Distribuzione di frequenza della luce in backscatter."@it, "Frequency distribution of the power of the received signals."@en,
    "接收信号的功率的频率分布"@cn;
  skos:inScheme <http://vocab.ieawindtask32.org/wind-lidar-ontology/>;
  skos:narrower ontolidar:CentroidPowerValue, ontolidar:DopplerPeak, ontolidar:MaximumPowerValue,
    ontolidar:MeanPowerValue, ontolidar:SystemNoiseThreshold, ontolidar:TimeIntegration,
    ontolidar:WeightingFunction;
  skos:prefLabel "Doppler Spectra"@en, "Doppler-Spektrum"@de, "Espectro Doppler"@es,
    "Spettri Doppler"@it, "多普勒光谱"@cn .

ontolidar:TimeIntegration a skos:Concept;
  skos:broader ontolidar:DopplerSpectra;
  skos:definition "Aggregation period of individual Doppler spectra."@en, "Periodo de agregación de los espectros Doppler individuales."@es,
    "Periodo di aggregazione di spettri Doppler singoli."@it, "单个多普勒频谱的积分时间"@cn;
  skos:editorialNote "Tiempo durante el cual el analizador de frecuencia se programa para acumula espectros de frecuencia individulaes provenientes de la señal lidar retrodispersada. Estos espectros son promediados para obtener el espectro Doppler que el lidar utiliza para estimar la velocidad radial del viento."@es,
    "Time whithin which the frequency analyser accumulates individual frequency spectra generated by the frequency analyser. Then it averages them to obtain the Doppler spectra the lidar uses to estimate the wind radial velocity."@en;
  skos:inScheme <http://vocab.ieawindtask32.org/wind-lidar-ontology/>;
  skos:prefLabel "Integración de tiempo"@es, "Integrazione temporale"@it, "Time integration"@en,
    "Zeitliche Integration"@de, "时间积分"@cn .

ontolidar:CentroidPowerValue a skos:Concept;
  skos:altLabel "Median"@en;
  skos:broader ontolidar:DopplerSpectra;
  skos:definition "El valor de potencia calculado como el centroide del espectro Doppler, que finalmente se identifica con la velocidad radial medida por el lidar."@es,
    "The power value calculated as the centroid of the Doppler spectrum which eventually is identified with the radial velocity measured by the lidar."@en,
    "Valore dello spettro Doppler corrispondente al centroide della distribuzione."@it;
  skos:editorialNote "The centroid corresponds to the arithmetic mean of the averaged frequency spectrum yielded by the lidar frequency analiser"@en;
  skos:inScheme <http://vocab.ieawindtask32.org/wind-lidar-ontology/>;
  skos:prefLabel "Centroid power value"@en, "Centroide"@es, "Centroide"@it, "Wert der Schwerpunktleistung"@de,
    "中心值"@cn;
  skos:related ontolidar:PeakIdentification .

ontolidar:MeanPowerValue a skos:Concept;
  skos:broader ontolidar:DopplerSpectra;
  skos:definition "El valor medio de la potencia en el espectro Doppler que finalmente se identifica con la velocidad radial medida por el lidar."@es,
    "The mean power value in the Doppler spectrum which eventually is identified with the radial velocity measured by the lidar."@en,
    "Valore medio dello spettro Doppler."@it;
  skos:inScheme <http://vocab.ieawindtask32.org/wind-lidar-ontology/>;
  skos:prefLabel "Mean power value"@en, "Media"@it, "Mittlerer Leistungswert"@de, "平均值"@cn;
  skos:related ontolidar:PeakIdentification .

ontolidar:MaximumPowerValue a skos:Concept;
  skos:broader ontolidar:DopplerSpectra;
  skos:definition "El valor máximo de potencia en el espectro Doppler que finalmente se identifica con la velocidad radial medida por el lidar."@es,
    "The maximum power value in the Doppler spectrum which eventually is identified with the radial velocity measured by the lidar."@en,
    "Valore massimo dello spettro Doppler."@it;
  skos:inScheme <http://vocab.ieawindtask32.org/wind-lidar-ontology/>;
  skos:prefLabel "Massimo"@it, "Maximaler Leistungswert"@de, "Maximum power value"@en,
    "最大值"@cn;
  skos:related ontolidar:PeakIdentification .

ontolidar:WeightingFunction a skos:Concept;
  skos:broader ontolidar:DopplerSpectra;
  skos:definition "Función utilizada para ponderar la frecuencia de las diferentes señales que se retrodispersan a lo largo del volumen de medición. La contribución a la estimación de la frecuencia Doppler es tanto mayor cuanto menor es la distancia al punto bajo medición. En general, se puede aproximar a una función Lorentziana."@es,
    "Function used to weight the backscattered intensity from the probe volume. The closer to the focused point, the higher contribution to the estimation of the Doppler frequency at that point. In general, it can be approximated by a Lorentzian function."@en,
    "Pesi relativi al volume della sonda da applicare all'intensità della luce di backscatter. Più si è prossimi al punto focale, maggiore è il contributo alla formazione del picco Doppler."@it,
    "用于加权探测体积中反射光强度的函数。离聚焦点越近，该点对多普勒频率的贡献就越大。一般来说，它可以用洛伦兹函数来近似。"@cn;
  skos:inScheme <http://vocab.ieawindtask32.org/wind-lidar-ontology/>;
  skos:prefLabel "Función de ponderación"@es, "Funzione di ponderazione"@it, "Gewichtungsfunktion"@de,
    "Weighting function"@en, "加权函数"@cn;
  skos:related ontolidar:ProbeVolume .

ontolidar:SystemNoiseThreshold a skos:Concept;
  skos:broader ontolidar:DopplerSpectra;
  skos:definition "El valor mínimo de potencia en el espectro de frecuencias, por encima del ruido del instrumento, que se acepta como señal relativa al viento."@es,
    "Minimo valore di potenza nello spettro Doppler perche' il segnale sia distinguibile dal rumore di fondo."@it,
    "The minimum power value in the frequency spectrum, above the instrument noise, that is accepted as a signal relative to the wind."@en,
    "频谱中被接受为风信号超过仪器噪声的最小功率值"@cn;
  skos:inScheme <http://vocab.ieawindtask32.org/wind-lidar-ontology/>;
  skos:prefLabel "Geräuschschwelle des Systems"@de, "Soglia di rumore del sistema"@it,
    "System noise threshold"@en, "系统噪声阈值"@cn .

ontolidar:WindfieldReconstruction a skos:Concept;
  skos:altLabel "Wind field reconstruction"@en;
  skos:broader ontolidar:DataProcessing;
  skos:definition "Métodos de procesamiento de datos lidar para estimar el vector de viento en uno o varios puntos en el dominio muestreado por el dispositivo lidar."@es,
    "Processo di derivazione del vettore campo del vento in uno o più punti dello spazio spazzato dal wind lidar."@it,
    "The approach to processing wind lidar data to estimate a wind vector at one or more points sampled by the lidar."@en,
    "通过处理测风激光雷达测得的数据，推算测风区域内一个或多个点处的风矢量的方法"@cn;
  skos:inScheme <http://vocab.ieawindtask32.org/wind-lidar-ontology/>;
  skos:narrower ontolidar:FilteringStrategy, ontolidar:Outputs, ontolidar:ScanGeometry,
    ontolidar:VelocityAzimuthDisplay, ontolidar:WindFieldModel;
  skos:prefLabel "Reconstrucción del campo de vientos"@es, "Ricostruzione del campo di vento"@it,
    "Windfeld-Rekonstruktion"@de, "Windfield Reconstruction"@en, "气流（风）流场重构"@cn .

ontolidar:WindFieldModel a skos:Concept;
  skos:broader ontolidar:WindfieldReconstruction;
  skos:definition "Il modello che è utilizzato per descrivere le caratteristiche del campo di vento."@it,
    "Los modelos de base matemática utilizados para describir las características del campo de viento."@es,
    "The mathematical-based models used to describe the wind field characteristics."@en,
    "描述气流（风）流场特性的数学模型"@cn;
  skos:inScheme <http://vocab.ieawindtask32.org/wind-lidar-ontology/>;
  skos:narrower ontolidar:MotionCompensation, ontolidar:WindTurbineModel;
  skos:prefLabel "Modello di campo eolico"@it, "Modelo de campo de viento"@es, "Wind field model"@en,
    "Windfeld-Modell"@de, "气流（风）流场模型"@cn .

ontolidar:WindTurbineModel a skos:Concept;
  skos:broader ontolidar:WindFieldModel;
  skos:definition "El modelo que se utiliza para describir la turbina eólica, la zona de inducción, la zona de influencia de la estela, etc."@es,
    "Il modello utilizzato per descrivere la turbina eolica, la sua zona di induzione, l'area influenzata dalla sua scia etc."@it,
    "The model that is used to describe the wind turbine, e.g. the induction zone, wake influence area, etc."@en,
    "描述风力发电机组的模型，包括感应区、尾流影响区等。模型将影响气流（风）的流场特性。"@cn;
  skos:inScheme <http://vocab.ieawindtask32.org/wind-lidar-ontology/>;
  skos:narrower ontolidar:ComplexFlow, ontolidar:SimpleFlow;
  skos:prefLabel "Modell einer Windkraftanlage"@de, "Modello di turbina eolica"@it,
    "Modelo de aerogenerador"@es, "Wind turbine model"@en, "风力发电机组模型"@cn .

ontolidar:SimpleFlow a skos:Concept;
  skos:altLabel "Simple Flow"@en;
  skos:broader ontolidar:WindTurbineModel;
  skos:definition "Flujo de viento definido como horizontal homogéneo, sin turbulencia o turbulencia despreciable que se suele utilizar para los modelos de campo de viento en terreno plano o en alta mar."@es,
    "Flusso ventoso in assenza di turbolenza o in presenza di debole turbolenza. E' solitamente utilizzato per modelli di vento in terreno piatto o offshore."@it,
    "Horizontal-homogeneous wind flow, no turbulence or little turbulence that can be neglected, which is usually used for wind field models in flat terrain or offshore."@en,
    "水平方向均质的气流，不含有湍流或只含有可以忽略的小湍流，该气流（风）流场模型通常适用于平坦地形或海上。"@cn;
  skos:inScheme <http://vocab.ieawindtask32.org/wind-lidar-ontology/>;
  skos:prefLabel "Einfacher Ablauf"@de, "Flusso semplice"@it, "Simple flow"@en, "flujo sencillo"@es,
    "简单气流"@cn .

ontolidar:ComplexFlow a skos:Concept;
  skos:altLabel "Complex Flow"@en;
  skos:broader ontolidar:WindTurbineModel;
  skos:definition "Flujo de viento horizontalmento no homogéneo con turbulencia significativa, que suele utilizarse para el modelo de campo de viento en terrenos complejos."@es,
    "Flusso ventoso in presenza di significativa turbolenza. E' solitamente utilizzato per modelli di vento in terreno complesso."@it,
    "Non-horizontal-homogeneous wind flow with significant turbulence, which usually used for wind field model in complex terrain."@en,
    "有明显湍流的非水平、均质的气流（风），该模型通常适用于复杂地形。"@cn;
  skos:inScheme <http://vocab.ieawindtask32.org/wind-lidar-ontology/>;
  skos:prefLabel "Complex flow"@en, "Flusso complesso"@it, "Komplexer Ablauf"@de, "flujo complejo"@es,
    "复杂气流"@cn .

ontolidar:MotionCompensation a skos:Concept;
  skos:broader ontolidar:WindFieldModel;
  skos:definition "Metodo di correzione dei dati registrati dal lidar per il moto della sorgente di luce stessa o del supporto dove essa si situa. Algoritmi cruciali per floating lidars o lidars montati su piattaforme mobili."@it,
    "Métodos de corrección de datos lidar durante el proceso de reconstrucción del campo de vientos. Para la corrección se incluyen datos sobre el movimiento del lidar registrados mediante el propio lidar u otras unidades de medición inercial. Típicamente utilizado para lidares flotantes u otras plataformas móviles como barcos."@es,
    "The methods that correct the reconstructed wind field with motion information from lidar or other inertial measurement units, typically for floating lidars or lidars mounted on a floating platform or vessel."@en,
    "用传感器测的的激光雷达运动信息修正或重构气流（风）流场的方法，通常用于漂浮式激光雷达或安装在浮动平台或船上的激光雷达"@cn;
  skos:inScheme <http://vocab.ieawindtask32.org/wind-lidar-ontology/>;
  skos:prefLabel "Bewegungskompensation"@de, "Compensación de movimiento"@es, "Compensazione del movimento"@it,
    "Motion compensation"@en, "运动补偿"@cn .

ontolidar:ScanGeometry a skos:Concept;
  skos:altLabel "Scan pattern"@en;
  skos:broader ontolidar:MeasurementSetup, ontolidar:WindfieldReconstruction;
  skos:definition "1. Serie de configuraciones de medidas realizadas por un lidar de escaneo que requieren que el haz lidar sea escaneado o barrido entre un número de orientacions diferentes. La geometría de barrido asegura que se adquieran mediciones en un volumen suficiente para posibilitar la reconstrucción del campo de viento. La secuencia de orientaciones del haz puede repetirse para adquirir una serie temporalde datos finales, adquiridos en cada iteración. Los escaneos pueden realizarse en modo stop-stare o sweep-stare. 2. La colección de líneas de visión (line-of-sight o LOS, por sus siglas en inglés) del haz a lo largo de las cuales el lidar está programado para emitir su sondeo."@es,
    "1. The arrangement of a sequence of scanning lidar configurations that require the lidar beam to be scanned or swept between a number of different orientations. The scan geometry ensures measurements are acquired throughout the measurement volume sufficient for wind field reconstruction. The sequence of beam orientations may be repeated to acquire a time series of final data acquired from each iteration. Scans may be performed in stop-stare or sweep-stare mode. 2. The collection of lines of sight / beam orientations along which the lidar is programmed to emit its probe."@en,
    "1. Una serie di configurazioni di misuraizone per uno scanning lidar che definisce come il fascio laser debba essere mosso e spostato fra una serie di posizioni pre-definite. Questa serie garantisce l'acquisizione in misura sufficiente di dati per ricostruire il campo di vento. La sequenza delle orientazioni può essere ripetuta per registrare una serie temporale della stessa quantità misurata. Il movimento da una posizione di misurazione alla successiva può essere effettuato in modalità stop-stare o sweep-stare. 2. L'insieme delle direzioni di misurazione / orientazioni del fascio laser in cui il lidar emette la sua sonda."@it,
    "1. 激光雷达扫描方式（顺序）的安排，要求激光雷达光束在一些不同的方向之间扫描或扫过。扫描的几何路径确保在整个测量范围内获得足够的测量结果以重建气流（风）流场。对应的光束方向的可以重复进行扫描，通过迭代扫描获得时间序列的数据集。扫描可以在停滞或扫掠模式下进行。2. 激光雷达的扫描光束方向，沿着雷达程序设定的发射其探测信号的方向。"@cn,
    "Secuencia de posicionamientos del rayo láser lidar en el espacio, que requiere que el rayo lidar escanee o barra una serie de orientaciones diferentes."@es,
    "Sequence of lidar laser beam placements in space, which require the lidar beam to be scanned or swept between a number of different orientations."@en,
    "Sequenza dei posizionamenti del raggio laser del lidar nello spazio."@it, "测风激光雷达光束在空间中扫过的位置，通常需要在若干不同方向上进行扫描。"@cn;
  skos:editorialNote "La tassonomia della geometria di scansione è basata sulla figura 3 di NREL/TP-5000-64634 https://www.nrel.gov/docs/fy16osti/64634.pdf"@it,
    "La taxonomía de la geometría de escaneo está basada en la Figura 3 de NREL/TP-5000-64634 https://www.nrel.gov/docs/fy16osti/64634.pdf"@es,
    "The scanning geometry taxonomy is based on Figure 3 in NREL/TP-5000-64634 https://www.nrel.gov/docs/fy16osti/64634.pdf"@en;
  skos:inScheme <http://vocab.ieawindtask32.org/wind-lidar-ontology/>;
  skos:narrower ontolidar:MeasurementVolume, ontolidar:MultiLidar, ontolidar:NonStatic,
    ontolidar:SingleLidar, ontolidar:Static;
  skos:prefLabel "Geometria di scansionamento"@it, "Geometria di scansione"@it, "Geometría de escaneo"@es,
    "Scan geometry"@en, "Scan-Geometrie"@de, "扫描的几何路径"@cn, "扫描路径"@cn;
  skos:related ontolidar:ScanGeometry .

ontolidar:Static a skos:Concept;
  skos:broader ontolidar:ScanGeometry;
  skos:definition "A lidar scan geometry with fixed lidar beam orientations in space."@en,
    "Geometria di scansionamento con il raggio laser fisso nello spazio."@it, "Geometría de escaneo lidar de orientaciones fijas del haz lidar."@es,
    "测风激光雷达工作时，光束在空间中扫描方向固定的扫描路径"@cn;
  skos:inScheme <http://vocab.ieawindtask32.org/wind-lidar-ontology/>;
  skos:prefLabel "Static"@en, "Statico"@it, "Statisch"@de, "静态扫描"@cn .

ontolidar:NonStatic a skos:Concept;
  skos:broader ontolidar:ScanGeometry;
  skos:definition "A lidar scan geometry that with dynamic lidar beam orientations in space."@en,
    "Geometria di scansionamento con il raggio laser in moto nello spazio."@it, "Una geometría de escaneo lidar que deorientaciones dinámicas del haz lidar."@es,
    "测风激光雷达工作时，光束在空间中扫描方向非固定的扫描路径"@cn;
  skos:inScheme <http://vocab.ieawindtask32.org/wind-lidar-ontology/>;
  skos:prefLabel "Nicht statisch"@de, "Non statico"@it, "Non-static"@en, "非静态扫描"@cn .

ontolidar:FilteringStrategy a skos:Concept;
  skos:broader ontolidar:WindfieldReconstruction;
  skos:definition "Los métodos de filtrado que se aplican para procesar los datos brutos del lidar, para producir conjuntos de datos lidar más fiables, listos para la reconstrucción del campo de viento u otros fines."@es,
    "Strategia di rigetto dei dati grezzi del lidar, per produrre misurazioni finali piu' accurate e precise."@it,
    "The filtering methods that applied to process lidar raw data, to produce more reliable lidar datasets ready for wind field reconstruction or other purposes."@en,
    "测风激光雷达原始数据的过滤方法，过滤异常、不确定的数据以生成可靠的数据集，用于气流（风）流场重建等。"@cn;
  skos:inScheme <http://vocab.ieawindtask32.org/wind-lidar-ontology/>;
  skos:narrower ontolidar:PreProcessedData, ontolidar:ProcessedData, ontolidar:RawData;
  skos:prefLabel "Filtering strategy"@en, "Filterstrategie"@de, "Strategia di filtraggio dati"@it,
    "数据过滤方法"@cn .

ontolidar:RawData a skos:Concept;
  skos:broader ontolidar:FilteringStrategy;
  skos:definition "Data output from the lidar ADC(Analog Digital Converter), before any filtering and post-processing algorithm."@en,
    "Dati in uscita dalla DSP del lidar, prima di qualsiasi filtraggio ed algoritmo di post-processamento."@it,
    "Salida de datos del convertidor analógico-digital (ADC ) del lidar, previo a la aplicación de cualquier algoritmo de filtrado o post-procesamiento."@es,
    "从激光雷达DSP输出，未经过任何数据过滤和后处理的数据"@cn;
  skos:inScheme <http://vocab.ieawindtask32.org/wind-lidar-ontology/>;
  skos:prefLabel "Raw data"@en, "RawData"@it, "Rohdaten"@de, "原始数据"@cn .

ontolidar:PreProcessedData a skos:Concept;
  skos:broader ontolidar:FilteringStrategy;
  skos:definition "Data that generated after filtering raw data by applying CNR thresholds and removing outliers."@en,
    "Dati ottenuti dopo aver applicato ai dati grezzi le soglie CNR ed averli puliti dalle anomalie."@it,
    "Datos generados tras filtrar los datos brutos aplicando umbrales CNR y eliminando los valores atípicos."@es,
    "通过应用CNR阈值和去除异常值对原始数据进行过滤后产生的数据。"@cn;
  skos:inScheme <http://vocab.ieawindtask32.org/wind-lidar-ontology/>;
  skos:narrower ontolidar:CnrThreshold, ontolidar:Outliers;
  skos:prefLabel "Dati pre-processati"@it, "Pre-processed data"@en, "Vorverarbeitete Daten"@de,
    "预处理的数据"@cn .

ontolidar:Outliers a skos:Concept;
  skos:broader ontolidar:PreProcessedData;
  skos:definition "In un gruppo di misurazioni, singole misure dalle caratteristiche particolarmente differenti rispetto alle statistiche principali del gruppo stesso."@it,
    "Observaciones que se encuentran a distancias anómalas de otros valores en una muestra aleatoria de una población. Estas observaciones se consideran inválidas y son descartadas."@es,
    "Observations that lie abnormal distances from other values in a random sample from a population. These observations are regarded as invalid."@en,
    "在人口的随机抽样中，与其他数值存在异常距离的观测值。这些观测值被认为是无效的。"@cn;
  skos:inScheme <http://vocab.ieawindtask32.org/wind-lidar-ontology/>;
  skos:prefLabel "Anomalie"@it, "Ausreißer"@de, "Outliers"@en, "异常值"@cn .

ontolidar:CnrThreshold a skos:Concept;
  skos:broader ontolidar:PreProcessedData;
  skos:definition "El ancho de banda de la CNR dentro del cual la intensidad del pico Doppler es claramente visible con respecto a la intensidad del ruido en el espectro de frecuencias."@es,
    "Soglia minima per distinguere il segnale del picco Doppler dal rumore di fondo."@it,
    "The CNR bandwidth within which the intensity of the Doppler peak is clearly visible with respect to the noise intensity in the freqency spectrum."@en,
    "载噪比带宽（-30dB至10dB），在此带宽内，多普勒峰值相对于频谱噪声来说是清晰可见的。"@cn;
  skos:inScheme <http://vocab.ieawindtask32.org/wind-lidar-ontology/>;
  skos:prefLabel "CNR Threshold"@en, "CNR-Schwellenwert"@de, "Soglia CNR"@it, "载噪比阈值"@cn .

ontolidar:ProcessedData a skos:Concept;
  skos:broader ontolidar:FilteringStrategy;
  skos:definition "Data that generated after processing the pre-processed data by special or case-dependent filtering methods. e.g. Filtering of data for the period when the lidar beam hits the wave."@en,
    "Dati prodotti per applicazione di filtri sui dati pre-processati."@it, "Datos generados tras el procesamiento de los datos pre-procesados mediante métodos especiales de filtrado u otros, en función del propósito."@es,
    "用因地（时）制宜的方法处理后的数据，以获得最终更可靠的数据集。例如，用特殊的方法对光束击中波浪时的数据进行过滤。"@cn;
  skos:inScheme <http://vocab.ieawindtask32.org/wind-lidar-ontology/>;
  skos:prefLabel "Dati post-processati"@it, "Processed data"@en, "Verarbeitete Daten"@de,
    "已处理的数据"@cn .

ontolidar:Outputs a skos:Concept;
  skos:broader ontolidar:WindfieldReconstruction;
  skos:definition "Data that generated after data-processing."@en, "Dati al termine della fase di processamento e filtraggio."@it,
    "Datos generados como producto final del proceso de medición del viento."@es, "经各种方法处理后的雷达数据"@cn;
  skos:inScheme <http://vocab.ieawindtask32.org/wind-lidar-ontology/>;
  skos:narrower ontolidar:TurbulenceIntensity, ontolidar:Uncertainties, ontolidar:WindVelocity;
  skos:prefLabel "Ausgaben"@de, "Outputs"@en, "Risultati"@it, "输出结果"@cn .

ontolidar:WindVelocity a skos:Concept;
  skos:altLabel "Wind speed"@en;
  skos:broader ontolidar:Outputs;
  skos:definition "El vector de velocidad del viento está formado por la velocidad y la dirección del viento para un momento dado."@es,
    "The wind velocity vector consist of wind speed and wind direction in a given time."@en,
    "Vettore della velocita' del vento, dato dalla combinazione di velocita assoluta e direzione."@it,
    "给定时间内的风速和风向"@cn;
  skos:inScheme <http://vocab.ieawindtask32.org/wind-lidar-ontology/>;
  skos:prefLabel "Velocità del vento"@it, "Wind velocity"@en, "Windgeschwindigkeit"@de,
    "风速"@cn .

ontolidar:TurbulenceIntensity a skos:Concept;
  skos:broader ontolidar:Outputs;
  skos:definition "Rapporto dra la deviazione standard e valor medio della velocita' del vento, misurati su un certo intervallo temporale (solitamente 10 o 60 minuti)."@it,
    "Ratio of the wind speed standard deviation to the mean wind speed, determined from the same set of measured data samples of wind speed, and taken over a specified period of time, typically 10min or 60min."@en,
    "Relación entre la desviación estándar de la velocidad del viento y la velocidad media del viento, determinada a partir del mismo conjunto de muestras de datos de viento observado, y tomados durante un periodo de tiempo específico, normalmente 10min o 60min."@es,
    "指定时间段内，风速标准偏差与平均风速的比率，由同一组风速测量数据样本确定，通常为10分钟或60分钟。"@cn;
  skos:inScheme <http://vocab.ieawindtask32.org/wind-lidar-ontology/>;
  skos:prefLabel "Intensità della turbolenza"@it, "Turbulence intensity"@en, "Turbulenzintensität"@de,
    "湍流强度"@cn .

ontolidar:Uncertainties a skos:Concept;
  skos:broader ontolidar:Outputs;
  skos:definition "Cantidades para estimar el error estadístico de los datos de medición del lidar, que afecta a la disponibilidad de los datos del lidar, a su validez, etc."@es,
    "Errore statistico della misurazione."@it, "Quantities to indicate the statistical error from lidar measurement data, which affects the lidar data availability, validility, etc."@en,
    "测风激光雷达测量数据的统计误差的度量，会影响数据的可利用率、有效性等。"@cn;
  skos:inScheme <http://vocab.ieawindtask32.org/wind-lidar-ontology/>;
  skos:prefLabel "Incertezze"@it, "Uncertainties"@en, "Ungewissheiten"@de, "不确定性"@cn .

ontolidar:DataFiltering a skos:Concept;
  skos:broader ontolidar:DataProcessing;
  skos:definition "Data filtering for various environmental factors, such as the detections of hard targets, fog, etc., which affect the CNR value."@en,
    "Métodos de filtrado de datos para diversos factores ambientales, como las detecciones de blanco sólido, niebla, etc., que afectan al ratio portadora/ruido (CNR)."@es,
    "Strategie di filtraggio dati per vari effetti meteorologici ed ambientali."@it, "对环境因素进行识别用于数据过滤，如对硬目标的探测、超净空气、大雾等，这些因素将对CNR的值产生影响。"@cn;
  skos:inScheme <http://vocab.ieawindtask32.org/wind-lidar-ontology/>;
  skos:narrower ontolidar:CleanAirDetection, ontolidar:CloudDetection, ontolidar:FogDetection,
    ontolidar:HardTargetDetection;
  skos:prefLabel "Data filtering"@en, "Filterung von Daten"@de, "Filtraggio dati per qualità"@it,
    "数据过滤"@cn;
  skos:related ontolidar:FilteringStrategy .

ontolidar:HardTargetDetection a skos:Concept;
  skos:broader ontolidar:DataFiltering;
  skos:definition "A range (or a quantity) to indicate the laser beam is reflected from an object, and the corresponding lidar measurement data shall be filtered out during the data processing."@en,
    "Filtro specifico per rimuovere dati spuri dovuti alla presenza di oggetti solidi nel tragitto del raggio laser."@it,
    "Rango (o cantidad) que indica que el rayo láser ha sido reflejado por un blanco sólido, y que los datos de medición lidar correspondientes se filtrarán durante el procesamiento de datos."@es,
    "一个范围（或数值）用来表示激光光束被某个实体反射，在数据处理过程中应将对应的测量数据进行过滤去除。"@cn;
  skos:inScheme <http://vocab.ieawindtask32.org/wind-lidar-ontology/>;
  skos:prefLabel "Hard target detection"@en, "Rilevamento di oggetti solidi"@it, "硬目标识别"@cn .

ontolidar:CloudDetection a skos:Concept;
  skos:broader ontolidar:DataFiltering;
  skos:definition "A range (or a quantity) to indicate the laser beam is reflected from Cloud, and the corresponding lidar measurement data shall be filtered out during the data processing."@en,
    "Filtro specifico per rimuovere dati spuri dovuti alla presenza di nuvole nel tragitto del raggio laser."@it,
    "Rango (o cantidad) para indicar que el rayo láser ha sido reflejado por una nube, y que los datos de medición lidar correspondientes se filtrarán durante el procesamiento de datos."@es,
    "一个范围（或数值）用来表示激光束被云层反射，在数据处理过程中应将对应的测量数据进行过滤去除。"@cn;
  skos:inScheme <http://vocab.ieawindtask32.org/wind-lidar-ontology/>;
  skos:prefLabel "Cloud detection"@en, "Rilevamento di nuvole"@it, "云层识别"@cn .

ontolidar:CleanAirDetection a skos:Concept;
  skos:broader ontolidar:DataFiltering;
  skos:definition "A quantity to indicate the weather is in clean air condition (less aerosols), and the correponsing lidar measurement data shall be specially processed during data filtering."@en,
    "Cantidad que indica condiciones de aire limpio (escasez de aerosoles), y los datos de medición lidar correpondientes serán especialmente procesados durante el filtrado de datos."@es,
    "Filtro specifico per rimuovere dati spuri dovuti alla presenza di aria pulita nel tragitto del raggio laser."@it,
    "一个范围（或数值）用来表示空气中含有较少的气溶胶，在数据过滤过程中应特别处理对应的测量数据。"@cn;
  skos:inScheme <http://vocab.ieawindtask32.org/wind-lidar-ontology/>;
  skos:prefLabel "Clean air detection"@en, "Erkennung sauberer Luft"@de, "Rilevamento di condizione di aria pulita"@it,
    "超净空气识别"@cn .

ontolidar:FogDetection a skos:Concept;
  skos:broader ontolidar:DataFiltering;
  skos:definition "A quantity to indicate the weather is in fog condition, and the correponsing lidar measurement data shall be specially processed during data filtering."@en,
    "Cantidad que indica condiciones de niebla, y los datos de medición lidar correpondientes serán especialmente procesados durante el filtrado de datos."@es,
    "Filtro specifico per rimuovere dati spuri dovuti alla presenza di nebbia nel tragitto del raggio laser."@it,
    "表示天气处于大雾状态的数量，在数据过滤过程中应特别处理相关的激光雷达测量数据。"@cn;
  skos:inScheme <http://vocab.ieawindtask32.org/wind-lidar-ontology/>;
  skos:prefLabel "Fog detection"@en, "Nebel-Erkennung"@de, "Rilevamento di nebbia"@it,
    "大雾天气识别"@cn .

ontolidar:CoordinateSystemTransformation a skos:Concept;
  skos:broader ontolidar:DataProcessing;
  skos:definition "Cambio di coordinate dal sistema solidale con il lidar (tipicamente coordinate sferiche) allo specifico sistema di coordinate richiesto dall'applicazione cui si ha interesse."@it,
    "Proceso matemático de transformación de los datos en el sistema de coordenadas por defecto del lidar (por ejemplo, el sistema de coordenadas esféricas, etc.) al sistema de coordenadas requerido por la aplicación que post procesará los datos (por ejemplo, el sistema inercial de coordenadas cartesianas definido por la regla de la mano derecha)."@es,
    "Transfer the data from the lidar default coordinate system (e.g. spherical coordinate system, etc.) to the coordinate system required by data application (e.g. right hand inertial coordinate system)."@en,
    "将数据从激光雷达默认坐标系（如球面坐标系等）转移到数据应用所需的坐标系（如右手惯性坐标系）。"@cn;
  skos:inScheme <http://vocab.ieawindtask32.org/wind-lidar-ontology/>;
  skos:prefLabel "Coordinate system transformation"@en, "Transformation des Koordinatensystems"@de,
    "Trasformazione del sistema di coordinate"@it, "坐标系统转换"@cn .

ontolidar:MeasurementSetup a skos:Concept;
  skos:inScheme <http://vocab.ieawindtask32.org/wind-lidar-ontology/>;
  skos:narrower ontolidar:MeasurementHeight, ontolidar:Probe, ontolidar:ScanGeometry;
  skos:prefLabel "Aufbau der Messung"@de, "Disposizione di misurazione"@it, "Measurement setup"@en,
    "测量设置"@cn;
  skos:topConceptOf <http://vocab.ieawindtask32.org/wind-lidar-ontology/> .

ontolidar:SingleLidar a skos:Concept;
  skos:broader ontolidar:ScanGeometry;
  skos:definition "A single lidar that returns line-of-sight data that are converted in to windfield characteristics without the use of data from another lidar or wind speed measurement device."@en,
    "Misurazioni effettuate da un lidar singolo."@it, "Un solo lidar aislado que devuelve datos de la línea de visión (line-of-sight o LOS, por sus siglas en inglés) que se convierten en características del campo de viento sin el uso de datos de otro lidar o dispositivo de medición de la velocidad del viento."@es,
    "仅用单独的一个激光雷达，凭其自身测量的视向数据推算出气流（风）特性，而无需使用来自另一个激光雷达或风速测量设备的数据。"@cn;
  skos:inScheme <http://vocab.ieawindtask32.org/wind-lidar-ontology/>;
  skos:narrower ontolidar:ArbitraryTrajectory, ontolidar:CompoundScan, ontolidar:SimpleScan,
    ontolidar:Staring, ontolidar:StopStare, ontolidar:SweepStare;
  skos:prefLabel "Einzelnes Lidar"@de, "Lidar individual"@es, "Lidar singolo"@it, "Single lidar"@en,
    "单个激光雷达"@cn .

ontolidar:SimpleScan a skos:Concept;
  skos:broader ontolidar:SingleLidar;
  skos:definition "A scan geometry which entails a variation in beam orientation in a single degree of freedom."@en,
    "Una geometria di scansione dello spazio dove la posizione del raggio laser dipende da un solo parametro."@it,
    "Una geometría de escaneo simple en que la posición del rayo depende de un solo parámetro."@es,
    "一种简单的扫描路径，通过方向在单个自由度内的控制来改变扫描位置"@cn;
  skos:inScheme <http://vocab.ieawindtask32.org/wind-lidar-ontology/>;
  skos:narrower ontolidar:VariableAzimuthScan, ontolidar:VariableElevationScan;
  skos:prefLabel "Einfacher Scan"@de, "Escaneo simple"@es, "Scansione semplice"@it,
    "Simple scan"@en, "简单扫描"@cn .

ontolidar:VariableAzimuthScan a skos:Concept;
  skos:altLabel "PPI"@en;
  skos:broader ontolidar:SimpleScan;
  skos:definition "A simple scan geometry with variable azimuth angle."@en, "Geometría de escaneo simple que sólo depende del ángulo azimut."@es,
    "Una geometria di scansione dello spazio dipendente solo dall'angolo di azimut del sistema."@it,
    "通过改变方位角来控制扫描位置的简单扫描方式"@cn;
  skos:inScheme <http://vocab.ieawindtask32.org/wind-lidar-ontology/>;
  skos:narrower ontolidar:CompleteCone, ontolidar:ConeSector, ontolidar:DopplerBeamSwinging;
  skos:prefLabel "Escaneo de azimut variable"@es, "Scansione ad azimut variabile"@it,
    "Variable azimuth scan"@en, "Variabler Azimut-Scan"@de, "变方位扫描法"@cn .

ontolidar:CompleteCone a skos:Concept;
  skos:broader ontolidar:VariableAzimuthScan;
  skos:definition "A scan geometry in which the azimuth angle of the beam is varied in increments over the full 360 degree range of possible azimuth angles."@en,
    "Geometría en la que el azimut puede variar a lo largo de un intervalo de 360 grados. Los valores de velocidad y dirección del viento se pueden obertener a través de un proceso de reconstrucción del campo de viento asumiendo, por ejemplo, una dependencia sinusoidal de la velocidad radial con el ángulo azimutal."@es,
    "Una geometria di scansione dello spazio in cui il fascio laser è mosso lungo tutto l'intervallo di 360 gradi dell'angolo azimutale. La velocità e la direzione del vento possono essere ottenute attraverso un processo di ricostruzione del campo ventoso che assume, per esempio, una dipendenza sinusoidale della velocità radiale dall'angolo di azimuth."@it,
    "一种扫描方式，其中光束的方位角在可能方位角的整个 360 度范围内变化。风速和风向值可以通过气流流场重建推算获得，例如通过假定计算值（风速，风向）与方位角存在正弦函数关系。"@cn;
  skos:editorialNote "La velocidad y dirección del viento puedens ser obtenidos mediante un proceso de reconstrucción del campo de vientos, asumiendo por ejemplo una dependencia senoidal con el ángulo azimutal."@es,
    "Wind speed and direction values can be obtained through a wind field reconstruction process, for example by assuming a sinusoidal dependence on azimuth angle."@en;
  skos:inScheme <http://vocab.ieawindtask32.org/wind-lidar-ontology/>;
  skos:prefLabel "Complete cone"@en, "Geometria a cono completo"@it, "Geometía de cono completo"@es,
    "Kompletter Kegel"@de, "完整的锥体扫描法"@cn .

ontolidar:ConeSector a skos:Concept;
  skos:altLabel "PPI"@en, "Plan-position indicator"@en;
  skos:broader ontolidar:VariableAzimuthScan;
  skos:definition "A scan geometry in which the azimuth angle of the beam is varied in increments over less than the full 360 degree range of possible azimuth angles."@en,
    "Geometría de escaneo en la cual el ángulo de escaneo azimutal se varía a lo largo de un intervalo inferior a 360 grados. Los valores de velocidad y dirección del viento se pueden obertener a través de un proceso de reconstrucción del campo de viento asumiendo, por ejemplo, una dependencia sinusoidal de la velocidad radial con el ángulo azimutal."@es,
    "Una geometria di scansione dello spazio in cui il fascio laser è mosso lungo una porzione dell'intervallo di 360 gradi dell'angolo azimutale. La velocità e la direzione del vento possono essere ottenute attraverso un processo di ricostruzione del campo ventoso che assume, per esempio, una dipendenza sinusoidale della velocità radiale dall'angolo di azimuth."@it,
    "一种扫描方式，其中光束的方位角在小于360 度范围内变化。风速和风向值可以通过气流流场重建推算获得，例如通过假定计算值（风速，风向）与方位角存在正弦函数关系。"@cn;
  skos:editorialNote "La velocidad y dirección del viento puedens ser obtenidos mediante un proceso de reconstrucción del campo de vientos, asumiendo por ejemplo una dependencia senoidal con el ángulo azimutal."@es,
    "Wind speed and direction values can be obtained through a wind field reconstruction process, for example by assuming a sinusoidal dependence on azimuth angle."@en;
  skos:inScheme <http://vocab.ieawindtask32.org/wind-lidar-ontology/>;
  skos:prefLabel "Cone sector"@en, "Geometria a settore di cono"@it, "Geometría de cono sectorial"@es,
    "Kegel-Sektor"@de, "锥体扇形扫描法"@cn .

ontolidar:DopplerBeamSwinging a skos:Concept;
  skos:altLabel "DBS"@en;
  skos:broader ontolidar:VariableAzimuthScan;
  skos:definition "A scan measurement principle in which the wind velocity reconstruction algorithm calculates wind velocity vector components immediately upon a new radial wind velocity becoming available. This technique provides the maximum sampling rate of the wind velocity components and consequently the wind velocity vector, which is desirable for instance in turbulence measurements."@en,
    "Geometría de escaneo en la cual el ángulo de escaneo azimutal se varía en intervalos de 90 grados a lo largo de los 360 grados posibles del ángulo azimutal. Los valores de velocidad y dirección del viento se pueden obertener a través de un proceso de reconstrucción del campo de viento asumiendo, por ejemplo, una dependencia sinusoidal de la velocidad radial con el ángulo azimutal."@es,
    "Una geometria di scansione dello spazio in cui il fascio laser è mosso in intervalli di 90 gradi lungo l'angolo azimutale. La velocità e la direzione del vento possono essere ottenute attraverso un processo di ricostruzione del campo ventoso che assume, per esempio, una dipendenza sinusoidale della velocità radiale dall'angolo di azimuth."@it,
    "一种扫描方式，其中光束的方位角在可能的方位角的整个 360 度范围内间隔90度变化。风速和风向值可以通过气流流场重建推算获得，例如通过假定计算值（风速，风向）与方位角存在正弦函数关系。"@cn;
  skos:editorialNote "Reference: Kelberlau, F. and Mann, J. “Cross-contamination effect on turbulence spectra from Doppler beam swinging wind lidar”, Wind Energ. Sci., 5, 519–541, 2020"@en,
    "Referencias: Kelberlau, F. and Mann, J. “Cross-contamination effect on turbulence spectra from Doppler beam swinging wind lidar”, Wind Energ. Sci., 5, 519–541, 2020"@es;
  skos:inScheme <http://vocab.ieawindtask32.org/wind-lidar-ontology/>;
  skos:prefLabel "Doppler beam swinging"@en, "Geometria ad oscillazione del fascio laser"@it,
    "Geometría de oscilación del haz Doppler"@es, "多普勒光束摆动扫描法"@cn .

ontolidar:VariableElevationScan a skos:Concept;
  skos:altLabel "RHI"@en;
  skos:broader ontolidar:SimpleScan;
  skos:definition "A simple scan geometry with variable elevation angle."@en, "Geometría de escaneo simple que sólo depende del ángulo de elevación."@es,
    "Una geometria di scansione dello spazio in cui l'angolo di elevazione varia."@it,
    "具有可变仰角的简单扫描方式"@cn;
  skos:editorialNote "La tassonomia della geometria di scansione è basata sulla figura 3 di NREL/TP-5000-64634 https://www.nrel.gov/docs/fy16osti/64634.pdf"@it,
    "La taxonomía de la geometría de escaneo se basa en la Figura 3 en NREL/TP-5000-64634 https://www.nrel.gov/docs/fy16osti/64634.pdf"@es,
    "The scanning geometry taxonomy is based on Figure 3 in NREL/TP-5000-64634 https://www.nrel.gov/docs/fy16osti/64634.pdf"@en;
  skos:inScheme <http://vocab.ieawindtask32.org/wind-lidar-ontology/>;
  skos:narrower ontolidar:VerticalSlice;
  skos:prefLabel "Geometria ad elevazione variabile"@it, "Geometría de elevación variable"@es,
    "Scan mit variabler Höhe"@de, "Variable elevation scan"@en, "可变仰角扫描法"@cn .

ontolidar:CompoundScan a skos:Concept;
  skos:broader ontolidar:SingleLidar;
  skos:definition "Compound scans include more degrees of freedom and are typically made up of a sequence of simple scans."@en,
    "Los escaneos compuestos incluyen más grados de libertad y suelen estar formados por una secuencia de escaneos simples."@es,
    "Una scansione composita include più gradi di libertà ed è tipicamente il risultato di una combinazione di più sequenze di scansioni semplici."@it,
    "复合扫描包括更多的自由度，通常由一系列简单的扫描方法组成"@cn;
  skos:inScheme <http://vocab.ieawindtask32.org/wind-lidar-ontology/>;
  skos:narrower ontolidar:SequentialScan;
  skos:prefLabel "Compound scan"@en, "Escaneo compuesto"@es, "Scansione composita"@it,
    "Zusammengesetzter Scan"@de, "复合扫描扫描法"@cn .

ontolidar:ArbitraryTrajectory a skos:Concept;
  skos:broader ontolidar:SingleLidar;
  skos:definition "Scans can be made where the beam is swept through an arbitrary combination of elevation and azimuth angles to follow a desired trajectory. This could be considered analagous to tracking the path of a flying bird from a fixed location."@en,
    "Se pueden realizar escaneos en los que el haz realiza un barrido variando arbitrariamente los ángulos de elevación y acimut para seguir una trayectoria determinada. Esto podría considerarse análogo al seguimiento de la trayectoria de un pájaro en vuelo desde una ubicación fija."@es,
    "Una geometria di misurazione dove il fascio laser è mosso lungo una combinazione arbitraria di angoli di elevazione e azimutali per seguire una specifica traiettoria spaziale. Questo è del tutto analogo ad una situazione in cui si volesse descrivere in termini geometrici il volo di un uccello utilizzando un punto di riferimento fisso."@it,
    "一种测风激光雷达的扫描方法，可以通过仰角和方位角的任意组合，跟踪所需轨迹进行扫描。比如：站在一个固定位置跟踪飞鸟的路径。"@cn;
  skos:inScheme <http://vocab.ieawindtask32.org/wind-lidar-ontology/>;
  skos:prefLabel "Arbitrary trajectory"@en, "Traiettoria arbitraria"@it, "Trayectoria arbitraria"@es,
    "Willkürliche Flugbahn"@de, "任意运动轨迹扫描法"@cn .

ontolidar:StopStare a skos:Concept;
  skos:broader ontolidar:SingleLidar;
  skos:definition "Line-of-sight data are acquired while the beam remains stationary in one of the pre-determined orientations comprising the scan geometry. No data are acquired while the beam is moved to its next position."@en,
    "Los datos de la línea de visión (line-of-sight o LOS, por sus siglas en inglés) son adquiridos mientras el rayo permanece estacionario en una de las orientaciones predeterminada a lo largo de la secuencia de escaneo. Ninguna medida se realiza durante la fase de reposicionamiento del laser a su siguiente posición."@es,
    "Metodo di acquisizione dati in cui la misurazione avviene mentre il fascio laser è mantenuto fermo nello spazio in una direzione predefinita. Nessuna misurazione è effettuata durante la fase di riposizionamento del fascio laser."@it,
    "一种测风激光雷达的扫描方法，只有当光束在预设扫描方向上保持静止时，才获取视线方向(LOS)的数据。当光束在预设位置之间切换移动时，不获取数据。"@cn;
  skos:inScheme <http://vocab.ieawindtask32.org/wind-lidar-ontology/>;
  skos:prefLabel "Geometria \"osserva da fisso\""@it, "Geometría de punto fijo"@es,
    "Stop-stare"@en, "Stop-starren"@de, "停止-凝视扫描法"@cn .

ontolidar:SweepStare a skos:Concept;
  skos:broader ontolidar:SingleLidar;
  skos:definition "Line-of-sight data are acquired continuously as the beam is scanned between pre-determined positions."@en,
    "Los datos de la línea de visión (line-of-sight o LOS, por sus siglas en inglés) son adquiridos continuamente, mientras el rayo recorre las posiciones de escaneo programadas."@es,
    "Metodo di acquisizione dati in cui la misurazione avviene mentre il fascio laser è costantemente mosso nello spazio."@it,
    "一种测风激光雷达的扫描方法，当光束在预定位置之间移动时，也会连续获取视线方向(LOS)的数据。"@cn;
  skos:inScheme <http://vocab.ieawindtask32.org/wind-lidar-ontology/>;
  skos:prefLabel "Geometria \"osserva in movimento\""@it, "Geometría de barrido"@es,
    "Sweep-stare"@en, "Sweep-starren"@de, "扫视扫描法"@cn .

ontolidar:Staring a skos:Concept;
  skos:broader ontolidar:SingleLidar;
  skos:definition "A scan geometry comprised of a single beam orientation."@en, "Geometría de escaneo que comprende una sola orientación del rayo de medición."@es,
    "Un lidar con orientazione del fascio laser fissa nello spazio."@it, "光束仅在单一方向扫描的扫描方式。"@cn;
  skos:inScheme <http://vocab.ieawindtask32.org/wind-lidar-ontology/>;
  skos:prefLabel "Geometria fissa"@it, "Geometría fija"@es, "Glotzend"@de, "Staring"@en,
    "凝视（单向）扫描法"@cn .

ontolidar:MultiLidar a skos:Concept;
  skos:altLabel "multilidar"@en, "multistatic"@en;
  skos:broader ontolidar:ScanGeometry;
  skos:definition "Coordinated measurements made in the same region by multiple lidar. Measurements may or may not be synchronised in time."@en,
    "Medidas coordinadas relizadas en la misma región por diferentes dispositivos lidar. Las medidas pueden estar sincronizadas en el tiempo."@es,
    "Misurazioni coordinate effettuate nella stessa regione da più sistemi lidar. Le misurazioni possono essere sincronizzate nel tempo."@it,
    "多个激光雷达在同一区域进行的协调测量。测量结果在时间上可能会（或不会）同步。"@cn;
  skos:inScheme <http://vocab.ieawindtask32.org/wind-lidar-ontology/>;
  skos:narrower ontolidar:ConvergentScan, ontolidar:VirtualMetMast;
  skos:prefLabel "Multi-Lidar"@de, "Multi-lidar"@en, "Multi-lidar"@es, "Multi-lidar"@it,
    "多激光雷达"@cn .

ontolidar:MeasurementVolume a skos:Concept;
  skos:broader ontolidar:ScanGeometry;
  skos:definition "Lo spazio illuminato dai fasci laser del lidar. Corresponde all'unione di tutte le regioni investigata dai singoli fasci laser (e loro singole aree di misurazione - probe volumes) che possono costituire un sistema lidar da cui le misurazioni grezze sono prese e combinate per costruire la misurazione finale."@it,
    "Región caracterizada por el lidar de viento. Corresponde a la región en la que los diferentes rayos con diversas orientaciones (o líneas de visión, LOS por sus siglas en inglés) penetran en la atmósfera tomando datos a lo largo de un volumen de muestreo. A lo largo de estos volúmenes de muestreo, cada uno correspondiente a una orientación (o línea de visión) el sistema adquiere datos intermedios de los que se extraen las mediciones finales."@es,
    "The region characterised by the wind lidar. Corresponds to the region penetrated by the various beam orientations / lines of sight and probe volumes where intermediate data are acquired to produce a final measurement."@en,
    "测风激光雷达采集信号的空间范围。具体来说，由光束预设的扫描位置所围成的空间，激光雷达将在这个空间内进行测量。"@cn;
  skos:inScheme <http://vocab.ieawindtask32.org/wind-lidar-ontology/>;
  skos:prefLabel "Measurement volume"@en, "Messvolumen"@de, "Volume di misurazione"@it,
    "Volumen de medición"@es, "测量范围"@cn .

ontolidar:Probe a skos:Concept;
  skos:broader ontolidar:MeasurementSetup;
  skos:definition "En el caso de un lidar pulsado, el sondeo es un pulso láser emitido a lo largo de la línea de visión (line-of-sight o LOS, por sus siglas en inglés) cuya orientación se determina por la configuración del lidar. En el caso de un lidar de onda continua el sondeo es una región relativamenta sensible a lo largo de la línea de visión determinada por la distancia focal del sistema."@es,
    "In the case of pulsed lidar, the probe is a laser pulse emitted along a line of sight whose orientation is determined by the configuration of the lidar. In the case of a continuous wave lidar, the probe is a part of the laser beam that has a highest power density along the line of sight determined by the optical focus of the system."@en,
    "Parte del lidar che interagisce con lo spazio esterno e permette di effettuare la misurazione. In un sistema pulsato, questo corrisponde ad un impulso di luce laser; in un sistema ad onda continua, è definita in modo statistico sulla distribuzione in potenza della luce emessa dal lidar nella direzione di misurazione."@it,
    "对于脉冲激光雷达，探测是沿视线发射的激光脉冲，其方向和位置由激光雷达的设置决定。对于连续波激光雷达，探测是沿视线方向聚集灵敏度相对较高的区域，由取决于系统的光学焦点。"@cn;
  skos:inScheme <http://vocab.ieawindtask32.org/wind-lidar-ontology/>;
  skos:narrower ontolidar:ProbeVolume, ontolidar:Range;
  skos:prefLabel "Probe"@en, "Sonda"@es, "Sonda"@it, "Sonde"@de, "探测"@cn .

ontolidar:Range a skos:Concept;
  skos:broader ontolidar:Probe;
  skos:definition "Distancia máxima a partir de la cual la detección está limitada por un criterio de disponibilidad de datos, por ejemplo, la SNR."@es,
    "La distanza massima oltre cui la misurazione è inibita a causa di criteri sulla disponibilità di segnale (ad esemçpio, insufficiente SNR)."@it,
    "The maximum distance beyond which detection is limited by a data availability criterion, for example, SNR."@en,
    "探测的最大距离。超过这个距离，数据可用性会降低，例如，信噪比超出正常范围。"@cn;
  skos:inScheme <http://vocab.ieawindtask32.org/wind-lidar-ontology/>;
  skos:narrower ontolidar:FocusDistance, ontolidar:RangeResolution, ontolidar:TimeOfFlight;
  skos:prefLabel "Bereich"@de, "Range"@en, "Range"@it, "探测距离"@cn .

ontolidar:FocusDistance a skos:Concept;
  skos:broader ontolidar:Range;
  skos:definition "Distancia desde el lidar hasta la distancia focal del telescopio. Idealmente coincide con el punto de convergencia máxima de luz del rayo."@es,
    "La distanza fra il centro della lente ottica e il suo fuoco."@it, "The distance from the lidar to the telescope focal length. Ideally coincides with the laser beam waist."@en,
    "从测风激光雷达到激光束汇聚点的距离，由望远镜的焦距规定。"@cn;
  skos:inScheme <http://vocab.ieawindtask32.org/wind-lidar-ontology/>;
  skos:prefLabel "Distanza di messa a fuoco"@it, "Focus distance"@en, "Fokus-Distanz"@de,
    "焦距"@cn .

ontolidar:TimeOfFlight a skos:Concept;
  skos:altLabel "TOF"@en;
  skos:broader ontolidar:Range;
  skos:definition "El tiempo empleado por un sistema de lidar pulsado desde el momento en que es emitido hasta que es recibio por el sistema, durante el cual interacciona con la atmósfera a lo largo de un volumen de muestreo desde el cual la señal se retrodispersa."@es,
    "In un sistema lidar pulsato, il tempo necessario fra l'istante dell'emissione di un impulso laser emissione e della ricezione del segnale riflesso."@it,
    "The time taken for a lidar pulse to be emitted, interact with the atmosphere in a probe volume such that it is backscattered, and return to be detected by the system."@en,
    "从激光雷达脉冲发射，到反射信号返回并被系统检测到所需要的时间。"@cn;
  skos:inScheme <http://vocab.ieawindtask32.org/wind-lidar-ontology/>;
  skos:prefLabel "Flugzeit"@de, "Tempo di volo"@it, "Tiempo de vuelo"@es, "Time of flight"@en,
    "飞行时间"@cn .

ontolidar:RangeResolution a skos:Concept;
  skos:broader ontolidar:Range;
  skos:definition "Distancia que puede ser resuelta por la longitud del pulso láser. Viene dada por la relación entre la velocidad de la luz y la mitad de la duración del pulso."@es,
    "La distanza che può essere risolta dalla lunghezza dell'impulso laser. E' data dalla metà del prodotto fra la velocità della luce e la durata dall'impulso."@it,
    "The range resolution is the distance that can be resolved by the laser pulse length. This is given by (half) the speed of light multiplied by the pulse duration."@en,
    "探测间隔分辨率是激光脉冲波所覆盖的距离。数值上等于光速乘以脉冲持续时间除以二。"@cn;
  skos:inScheme <http://vocab.ieawindtask32.org/wind-lidar-ontology/>;
  skos:prefLabel "Bereichsauflösung"@de, "Range resolution"@en, "Resolución de distancia"@es,
    "Risoluzione della distanza"@it, "探测间隔分辨率"@cn .

ontolidar:ProbeVolume a skos:Concept;
  skos:broader ontolidar:Probe;
  skos:definition "The volume in which the probe interacts with the atmosphere resulting in the measurement of a radial velocity."@en,
    "Volume spaziale investito dalla sonda del lidar (probe). In questa regione avviene l'interazione fra il sistema lidar e l'atmosfera e da questa regione di deriva la velocità radiale del vento."@it,
    "Volumen a lo largo del cual la sonda interactúa con la atmósfera dando como resultado la medida de la velocidad radial."@es,
    "测风激光雷达测量视线方向速度所覆盖的空间范围。"@cn;
  skos:inScheme <http://vocab.ieawindtask32.org/wind-lidar-ontology/>;
  skos:narrower ontolidar:BeamDiameter, ontolidar:RayleighLength;
  skos:prefLabel "Probe volume"@en, "Sondenvolumen"@de, "Volume della sonda"@it, "Volumen de la sonda"@es,
    "探测体积"@cn .

ontolidar:RayleighLength a skos:Concept;
  skos:broader ontolidar:ProbeVolume;
  skos:definition "Distance, from the beam waist in the propagation direction, where the area of the beam section is increased by a factor of 2, or the radius is increased by a factor of the squared root of 2. The Rayleigh length is used to characterise the probe volume and corresponds to the half of the probe length. It also can be defined as half of the full-width half-maximum (FWHM) of the weighting function characterising the probe volume."@en,
    "Distancia, tomando como referencia la distancia focal del haz, en la dirección de propagación del mismo, donde el área de la sección del haz se duplica, o dicho de otro modo, el radio se incrementa en un factor raíz de 2. La longitud de Rayleigh se utiliza para caracterizar el volumen de la sonda y corresponde a la mitad de la longitud de muestreo."@es,
    "Distanza lungo la direzione di propagazione del raggio laser fra il punto di minima apertura radiale del raggio laser al punto di apertura radiale doppia rispetto al valor minimo. La distanza di Rayleigh è usata per caratterizzare il volume della sonda di misurazione e corrisponde a metà della lunghezza della sonda di prova."@it,
    "一种距离的表示方式，从传播方向的光束腰部开始，光束部分的截面积面积增加了2倍，或者截面半径增加了根号2倍。瑞利长度用于描述探测体积的特征，相当于探测体长度的一半。"@cn;
  skos:inScheme <http://vocab.ieawindtask32.org/wind-lidar-ontology/>;
  skos:prefLabel "Longitud Rayleigh"@es, "Lunghezza Rayleigh"@it, "Rayleigh Länge"@de,
    "Rayleigh length"@en, "瑞利长度"@cn;
  skos:related ontolidar:FullWidthAtHalfMaximum .

ontolidar:BeamDiameter a skos:Concept;
  skos:broader ontolidar:ProbeVolume;
  skos:definition "Diameter of the laser beam."@en, "Diametro del raggio laser."@it,
    "Diámetro del rayo láser."@es;
  skos:inScheme <http://vocab.ieawindtask32.org/wind-lidar-ontology/>;
  skos:prefLabel "Beam diameter"@en, "Diametro del fascio"@it, "Strahldurchmesser"@de .

ontolidar:MeasurementHeight a skos:Concept;
  skos:broader ontolidar:MeasurementSetup;
  skos:definition "Altezza nominale sopra il piano di riferimento. Ad essa viene associato il processo di ricostruzione del campo eolico e la misurazione della velocità del vento ad essa associata. Spesso usato nei lidar eolici ad asse verticale per confronto fra le misurazioni dal lidar e da anemometri tradizionali."@it,
    "Altura nominal sobre el plano de referencia donde la reconstrucción del viento devuelve la velocidad del viento. Normalmente utilizado para lidar de viento de perfil vertical en comparación con medidas de viento procedentes de un anemómetro."@es,
    "The nominal height above the datum plane at which a windfield reconstruction process returns a wind speed."@en,
    "气流流场重建生成风速的位置相距基准平面的标称高度。 通常用于计算激光雷达所测的垂直剖面测量值，以与风速计的点风速测量值进行比较。"@cn;
  skos:editorialNote "A menudo se utiliza para los lidares de viento de perfil vertical, para compararlos con las mediciones de velocidad del viento puntuales de un anemómetro."@es,
    "Often used for vertically-profiling wind lidars for comparison to point wind speed measurements from an anemometer."@en;
  skos:inScheme <http://vocab.ieawindtask32.org/wind-lidar-ontology/>;
  skos:narrower ontolidar:DatumElevation, ontolidar:DatumFeature, ontolidar:DatumPlane;
  skos:prefLabel "Altezza di misurazione"@it, "Altura de medición"@es, "Measurement height"@en,
    "Messhöhe"@de, "测量高度"@cn .

ontolidar:DatumFeature a skos:Concept;
  skos:altLabel "Reference marker"@en;
  skos:broader ontolidar:MeasurementHeight;
  skos:definition "A distinguishing feature used to recognise or define the datum plane from which the measurement height is defined."@en,
    "Característica específica utilizada para distinguir o definit el plano de referencia desde el que se define la medida de altura."@es,
    "Un elemento ben distinguibile atto a riconoscere o definire un piano di riferimento per la definizione dell'altezza di misurazione."@it,
    "用于识别或定义测量高度的基准平面的主要特征(值)"@cn;
  skos:inScheme <http://vocab.ieawindtask32.org/wind-lidar-ontology/>;
  skos:prefLabel "Característica de referencia"@es, "Datum feature"@en, "Elemento di riferimento"@it,
    "基准特征"@cn .

ontolidar:DatumElevation a skos:Concept;
  ontolidar:units "meters"@en;
  skos:broader ontolidar:MeasurementHeight;
  skos:definition "Altezza di un piano di riferimento sul livello del mare."@it, "Altura de plano de referencia sobre el nivel del mar."@es,
    "The height of the datum plane above sea level."@en, "基准面相距海平面的高度"@cn;
  skos:editorialNote "El nivel del mar debe definirse según el proyecto y está fuera del alcance de este esquema."@es,
    "Il livello del mare dovrebbe essere definito progetto per progetto e farlo non è fra gli obiettivi di questo progetto."@it,
    "Sea level should be defined on a project basis and is out of scope of this schema."@en;
  skos:inScheme <http://vocab.ieawindtask32.org/wind-lidar-ontology/>;
  skos:prefLabel "Datum elevation"@en, "Elevación de referencia"@es, "Elevazione di riferimento"@it,
    "基准高程"@cn .

ontolidar:DatumPlane a skos:Concept;
  skos:altLabel "Reference height"@en;
  skos:broader ontolidar:MeasurementHeight;
  skos:definition "Piano orizzontale di riferimento per la misurazione delle altezze locali. Tipicamente la finestra del lidar, il piano terra locale, la parte superiore di una piattaforma o un qualsiasi altro riferimento."@it,
    "Plano horizontal desde el que se definen la alrura de referencia. Típicamente ventana del lidar, plano local de tierra, parte superior de una plataforma u otra referencia."@es,
    "The horizontal plane from which the measurement height is defined, e.g., lidar window, local ground, a platform top surface, or other reference."@en,
    "各种测量高度的参考水平面，例如激光雷达窗口、本地地面、平台顶面或其他高度值的参考。"@cn;
  skos:inScheme <http://vocab.ieawindtask32.org/wind-lidar-ontology/>;
  skos:prefLabel "Datum plane"@en, "Piano di riferimento"@it, "Plano de referencia"@es,
    "基准面"@cn .

ontolidar:MeasurementPrinciples a skos:Concept;
  skos:definition "Assunti concettuali alla base della misurazione del vento da parte di un sistema lidar."@it,
    "Medios utilizados por el lidar para realizar medidas de viento."@es, "The means by which a lidar makes a measurement of the wind."@en,
    "激光雷达的测风方法"@cn;
  skos:inScheme <http://vocab.ieawindtask32.org/wind-lidar-ontology/>;
  skos:narrower ontolidar:DetectionType, <http://vocab.ieawindtask32.org/wind-lidar-ontology/Emitter/ReceiverConfiguration>,
    ontolidar:LidarSampleRate, ontolidar:LineOfSight, ontolidar:Scattering, ontolidar:WindSpeedEvaluation;
  skos:prefLabel "Measurement principles"@en, "Messprinzipien"@de, "Principi di misurazione"@it,
    "Principios de medición"@es, "测量原则"@cn;
  skos:topConceptOf <http://vocab.ieawindtask32.org/wind-lidar-ontology/> .

<http://vocab.ieawindtask32.org/wind-lidar-ontology/Emitter/ReceiverConfiguration>
  a skos:Concept;
  skos:broader ontolidar:MeasurementPrinciples;
  skos:definition "Die Positionierung und Anordnung der Sende- und Empfangsgeräte."@de,
    "El posicionamiento y disposición de los dispositivos emisores y receptores."@es,
    "Il posizionamento e la disposizione dei dispositivi emettitore e ricevitore."@it,
    "The positioning and arrangement of the emitter and receiver devices."@en, "发射器和接收器在雷达中的安装和配置。"@cn;
  skos:editorialNote "Puede ser monoestático (con una configuración coaxial o biaxial) o biestático."@es,
    "This can be monostatic (with biaxial or a coaxial sensor arrangement) or bistatic"@en;
  skos:inScheme <http://vocab.ieawindtask32.org/wind-lidar-ontology/>;
  skos:prefLabel "Configurazione dell'emettitore/ricevitore"@it, "Emitter/receiver configuration"@en,
    "Sender-/Empfängerkonfiguration"@de, "发射器/接收器配置"@cn .

ontolidar:Monostatic a skos:Concept;
  skos:broader <http://vocab.ieawindtask32.org/wind-lidar-ontology/Emmiter/ReceiverConfiguration>;
  skos:definition "A lidar configuration where the transmitter and receiver are positioned in close proximity, the transmit and receive paths share common optics, and range determination is achieved by pulsed laser timing."@en,
    "Eine Lidar-Konfiguration, bei der Sender und Empfänger in unmittelbarer Nähe positioniert sind und die Entfernungsbestimmung durch gepulstes Laser-Timing erreicht wird."@de,
    "Una configuración lidar en la que el transmisor y el receptor se colocan en estrecha proximidad, y la determinación del alcance se logra mediante la temporización de láser pulsado."@es,
    "Una configurazione lidar in cui il trasmettitore e il ricevitore sono posizionati nelle immediate vicinanze e la determinazione della portata è ottenuta mediante la temporizzazione del laser pulsato."@it,
    "一种激光雷达配置，发射器和接收器的位置很近，通过脉冲激光计时来确定范围。"@cn;
  skos:inScheme <http://vocab.ieawindtask32.org/wind-lidar-ontology/>;
  skos:prefLabel "Monostatic"@en, "Monostatico"@it, "Monostatisch"@de, "单稳态"@cn .

ontolidar:Bistatic a skos:Concept;
  skos:broader <http://vocab.ieawindtask32.org/wind-lidar-ontology/Emmiter/ReceiverConfiguration>;
  skos:definition "A lidar configuration where the transmitter and receiver are arranged to have considerable spatial separation, and the transmit and receive paths do not share common optics."@en,
    "Eine Lidar-Konfiguration, bei der Sender und Empfänger so angeordnet sind, dass sie eine beträchtliche räumliche Trennung aufweisen, was zu einer direkten räumlichen Auflösung bei der optischen Sondierung führt."@de,
    "Una configuración lidar en la que el transmisor y el receptor están dispuestos para tener una separación espacial considerable, lo que lleva a una resolución espacial directa en el sondeo óptico."@es,
    "Una configurazione lidar in cui il trasmettitore e il ricevitore sono disposti in modo da avere una notevole separazione spaziale, portando a una risoluzione spaziale diretta nel sondaggio ottico."@it,
    "一种激光雷达配置，发射器和接收器被安排成具有相当大的空间距离，导致光学探测的直接空间分辨率。"@cn;
  skos:inScheme <http://vocab.ieawindtask32.org/wind-lidar-ontology/>;
  skos:prefLabel "Bistatic"@en, "Bistatico"@it, "Bistatisch"@de, "双稳态"@cn .

ontolidar:Scattering a skos:Concept;
  skos:broader ontolidar:MeasurementPrinciples;
  skos:definition "Die Änderung der Bewegungsrichtung eines Teilchens oder einer Welle durch Kollision mit einem anderen Teilchen."@de,
    "El cambio en la dirección del movimiento de una partícula u onda debido a la colisión con otra partícula."@es,
    "Il cambiamento nella direzione del movimento di una particella o di un'onda a causa della collisione con un'altra particella."@it,
    "The change in direction of motion of a particle or wave due to collision with another particle."@en,
    "一个粒子或波由于与另一个粒子的碰撞而改变运动方向。"@cn;
  skos:inScheme <http://vocab.ieawindtask32.org/wind-lidar-ontology/>;
  skos:narrower ontolidar:Mie, ontolidar:Raman, ontolidar:Rayleigh;
  skos:prefLabel "Scattering"@en, "Scattering"@it, "Streuung"@de, "散射"@cn .

ontolidar:Raman a skos:Concept;
  skos:broader ontolidar:Scattering;
  skos:definition "Diffusione anelastica della luce da oggetti per cui il fotone diffuso ha un'energia superiore o inferiore rispetto al fotone incidente."@it,
    "Dispersión inelástica de la luz de los objetos en la que el fotón dispersado tiene una energía mayor o menor que el fotón incidente."@es,
    "Inelastic scattering of light from objects whereby the scattered photon has a higher or lower energy than the incident photon."@en,
    "Inelastische Streuung von Licht an Objekten, wobei das gestreute Photon eine höhere oder niedrigere Energie hat als das einfallende Photon."@de,
    "光的非弹性散射，散射的光子比入射的光子有更高或更低的能量。"@cn;
  skos:inScheme <http://vocab.ieawindtask32.org/wind-lidar-ontology/>;
  skos:prefLabel "Raman"@de, "Raman"@en, "Raman"@it, "拉曼"@cn .

ontolidar:Mie a skos:Concept;
  skos:broader ontolidar:Scattering;
  skos:definition "Diffusione elastica della luce in cui il diametro delle particelle di dispersione è maggiore della lunghezza d'onda della luce incidente."@it,
    "Dispersión elástica de la luz donde el diámetro de las partículas dispersas es mayor que la longitud de onda de la luz incidente."@es,
    "Elastic scattering of light where the scattering particles diameter is larger than about the wavelength of the incident light."@en,
    "Elastische Lichtstreuung, bei der der Durchmesser der Streupartikel größer ist als etwa die Wellenlänge des einfallenden Lichts."@de,
    "光的弹性散射，散射粒子的直径大于入射光的波长。"@cn;
  skos:inScheme <http://vocab.ieawindtask32.org/wind-lidar-ontology/>;
  skos:prefLabel "Mie"@en, "Mie"@it, "米氏"@cn .

ontolidar:Rayleigh a skos:Concept;
  skos:broader ontolidar:Scattering;
  skos:definition "Diffusione elastica della luce in cui il diametro delle particelle di dispersione è inferiore a circa un decimo della lunghezza d'onda della luce incidente."@it,
    "Dispersión elástica de la luz en la que el diámetro de las partículas dispersas es inferior a aproximadamente una décima parte de la longitud de onda de la luz incidente."@es,
    "Elastic scattering of light where the scattering particles diameter is less than about one-tenth of the wavelength of the incident light."@en,
    "Elastische Lichtstreuung, bei der der Durchmesser der Streupartikel kleiner als etwa ein Zehntel der Wellenlänge des einfallenden Lichts ist."@de,
    "光的弹性散射，其中散射粒子的直径小于入射光波长的十分之一。"@cn;
  skos:inScheme <http://vocab.ieawindtask32.org/wind-lidar-ontology/>;
  skos:prefLabel "Raylegih"@it, "Rayleigh"@de, "Rayleigh"@en, "瑞利"@cn .

ontolidar:DetectionType a skos:Concept;
  skos:broader ontolidar:MeasurementPrinciples;
  skos:definition "Das Verfahren, mit dem die Frequenzverschiebung der gestreuten Strahlung bestimmt wird."@de,
    "El método por el cual se determina el cambio de frecuencia de la radiación dispersada."@es,
    "Il metodo con cui viene determinato lo spostamento di frequenza della radiazione diffusa."@it,
    "The method by which the frequency shift of the scattered radiation is determined."@en,
    "确定散射辐射的频移的方法。"@cn;
  skos:inScheme <http://vocab.ieawindtask32.org/wind-lidar-ontology/>;
  skos:narrower ontolidar:Coherent, ontolidar:DetectionConfiguration, ontolidar:Incoherent;
  skos:prefLabel "Art der Erkennung"@de, "Detection type"@en, "Tipo di rilevamento"@it,
    "检测类型"@cn .

ontolidar:Coherent a skos:Concept;
  skos:broader ontolidar:DetectionType;
  skos:definition "A lidar system where the frequency shift is measured by comparing the return signal to a reference signal."@en,
    "Ein Lidar-System, bei dem die Frequenzverschiebung gemessen wird, indem das Rücksignal mit einem Referenzsignal verglichen wird."@de,
    "Sistema lidar donde el cambio de frecuencia se mide comparando la señal de retorno con una señal de referencia."@es,
    "Un sistema lidar in cui lo spostamento di frequenza viene misurato confrontando il segnale di ritorno con un segnale di riferimento."@it,
    "一种激光雷达系统，其中频率偏移是通过比较返回信号和参考信号来测量的。"@cn;
  skos:inScheme <http://vocab.ieawindtask32.org/wind-lidar-ontology/>;
  skos:prefLabel "Coerente"@it, "Coherent"@en, "Kohärent"@de, "相干"@cn .

ontolidar:Incoherent a skos:Concept;
  skos:altLabel "Direct"@en;
  skos:broader ontolidar:DetectionType;
  skos:definition "A lidar system where the return signal is filtered or resolved into its spectral components to obtain the frequency shift. Also known as time-of-flight lidar or direct-detection lidar."@en,
    "Ein Lidar-System, bei dem das Rücksignal gefiltert oder in seine Spektralkomponenten aufgelöst wird, um die Frequenzverschiebung zu erhalten. Auch bekannt als Time-of-Flight-Lidar oder Direkterkennungs-Lidar."@de,
    "Sistema lidar donde la señal de retorno se filtra o se resuelve en sus componentes espectrales para obtener el cambio de frecuencia. También conocido como lidar de tiempo de vuelo o lidar de detección directa."@es,
    "Un sistema lidar in cui il segnale di ritorno viene filtrato o risolto nelle sue componenti spettrali per ottenere lo spostamento di frequenza. Conosciuto anche come lidar del tempo di volo o lidar a rilevamento diretto."@it,
    "一种激光雷达系统，其中返回信号被过滤或分解成其光谱成分以获得频移。也被称为飞行时间激光雷达或直接探测激光雷达。"@cn;
  skos:inScheme <http://vocab.ieawindtask32.org/wind-lidar-ontology/>;
  skos:prefLabel "Incoerente"@it, "Incoherent"@en, "Inkohärent"@de, "非相干"@cn .

ontolidar:DetectionConfiguration a skos:Concept;
  skos:broader ontolidar:DetectionType;
  skos:definition "The process of detecting a radio wave by the aid of a locally generated current or wave of exactly the same frequency as that of the incoming wave. A signal frequency that is created by combining or mixing two other frequencies using a signal processing technique called heterodyning."@en;
  skos:inScheme <http://vocab.ieawindtask32.org/wind-lidar-ontology/>;
  skos:prefLabel "Configurazione"@it, "Detection Configuration"@en, "Konfiguration der Erkennung"@de,
    "配置"@cn .

ontolidar:Homodyne a skos:Concept;
  skos:broader ontolidar:Configuration;
  skos:definition "A frequency shift detection method. The lidar directly downmixes the reference and the backscattered signals retrieving a (Doppler) frequency shift. Only the magnitude of the Doppler shift can be known, but not the sign. This means that we can infer only the module (and not the direction) of the wind speed vector."@en,
    "Ein Lidar-Detektionsverfahren, bei dem die Referenzstrahlung vor dem Modulationsprozess von derselben Quelle stammt wie das Signal."@de,
    "Un metodo di rilevamento lidar in cui la radiazione di riferimento è derivata dalla stessa sorgente del segnale prima del processo di modulazione."@it,
    "Un método de detección de desplazamiento de frecuencia. El lidar mezcla directamente la señal de referencia y la retrodispersada, obteniendo un desplazamiento de frecuencia (Doppler). Sólo se puede conocer la magnitud del desplazamiento de la frecuencia, pero no la dirección del mismo. Esto significa que sólo podemos inferir el módulo (y no la dirección) del vector de velocidad del viento."@es,
    "一种激光雷达检测方法，其中参考辐射在调制过程之前来自与信号相同的来源。"@cn;
  skos:inScheme <http://vocab.ieawindtask32.org/wind-lidar-ontology/>;
  skos:prefLabel "Homodyne"@en, "Omodinamico"@it, "同位素"@cn .

ontolidar:Heterodyne a skos:Concept;
  skos:broader ontolidar:Configuration;
  skos:definition "A frequency shift detection method. Prior to the dowmix of the original and the backscattered signals, the original one is frequency-shifted. This allows to retrieve not only the magnitude of the frequency shift between the original and the backscattered signals, but also the direction of the change. This means that we can infer both module and direction of the wind speed vector."@en,
    "Ein Lidar-Detektionsverfahren, bei dem die Referenzstrahlung vor dem Modulationsprozess von einer anderen Quelle als das Signal stammt."@de,
    "Un metodo di rilevamento lidar in cui la radiazione di riferimento è derivata da una sorgente diversa come il segnale prima del processo di modulazione."@it,
    "Un método de detección de desplazamiento de frecuencia. Antes de la mezcla de las señales original y retrodispersada, la original se desplaza en frecuencia. Esto permite obtener no sólo la magnitud del cambio de frecuencia entre la señal original y la retrodispersa, sino también la dirección del cambio. Esto significa que podemos inferir tanto el módulo como la dirección del vector de velocidad del viento."@es,
    "一种激光雷达检测方法，其中参考辐射在调制过程之前来自与信号不同的来源。"@cn;
  skos:inScheme <http://vocab.ieawindtask32.org/wind-lidar-ontology/>;
  skos:prefLabel "Eterodinamico"@it, "Heterodyne"@en, "Überlagern"@de, "异频雷达"@cn .

ontolidar:WindSpeedEvaluation a skos:Concept;
  skos:broader ontolidar:MeasurementPrinciples;
  skos:definition "Berechnung der Windgeschwindigkeit mit einem Windfeld-Rekonstruktionsverfahren."@de,
    "Calcolo della velocità del vento mediante un metodo di ricostruzione del campo eolico."@it,
    "Calculation of the wind velocity using a wind field reconstruction method."@en, "Cálculo de la velocidad del viento mediante un método de reconstrucción del campo de viento."@es,
    "使用气流(风)流场重建方法计算风速。"@cn;
  skos:inScheme <http://vocab.ieawindtask32.org/wind-lidar-ontology/>;
  skos:narrower ontolidar:CrossCorrelation, ontolidar:ParticleTracking;
  skos:prefLabel "Valutazione della velocità del vento"@it, "Wind speed evaluation"@en,
    "Windgeschwindigkeitsevaluation"@de, "风速评估"@cn .

ontolidar:ParticleTracking a skos:Concept;
  skos:broader ontolidar:WindSpeedEvaluation;
  skos:definition "Applicazione dove il raggio laser segue le singole prticelle nel loro moto nell'aria (statistica Lagrangiana)."@it,
    "Particle tracking as a method where the lidar beam follows the particle in the flow (refer to Langrangian statistics)."@en,
    "Seguimiento de partículas como método en la que el haz lidar sigue a la partícula en el flujo."@es,
    "一种气流流场模型：粒子跟踪作为一种应用，激光雷达光束在流动中跟随粒子（参考Langrangian统计）。"@cn;
  skos:inScheme <http://vocab.ieawindtask32.org/wind-lidar-ontology/>;
  skos:prefLabel "Particle tracking"@en, "Partikel-Tracking"@de, "Tracciamento di particella"@it,
    "粒子跟踪"@cn .

ontolidar:CrossCorrelation a skos:Concept;
  skos:broader ontolidar:WindSpeedEvaluation;
  skos:definition "Correlación cruzada como método para describir la turbulencia en el campo utilizando la estadística."@es,
    "Cross-correlation as a method to describe turbulence in the field using statistics."@en,
    "Metodo per calcolare la turbolenza con metodi prettamente statistici ."@it, "一种气流流场模型：交叉相关作为一个术语，用统计学描述流场中的湍流情况"@cn;
  skos:inScheme <http://vocab.ieawindtask32.org/wind-lidar-ontology/>;
  skos:prefLabel "Correlazione incrociata"@it, "Cross-correlation"@en, "Kreuzkorrelation"@de,
    "交叉相关"@cn .

ontolidar:DopplerPeak a skos:Concept;
  skos:broader ontolidar:DopplerSpectra;
  skos:definition "Doppler peak as a method to describe the amplitude of the wind speed asumming that the aerosols flow at the same speed as the wind."@en,
    "Pico Doppler como método para describir la amplitud de la velocidad del viento asumiendo que los aerosoles se desplazan a la misma velocidad que el viento."@es;
  skos:inScheme <http://vocab.ieawindtask32.org/wind-lidar-ontology/>;
  skos:prefLabel "Doppler peak"@en .

ontolidar:LineOfSight a skos:Concept;
  skos:broader ontolidar:MeasurementPrinciples;
  skos:definition "La direzione lungo cui il raggio laser del lidar è emesso e riflesso dall'atmosfera verso il lidar."@it,
    "Línea a lo largo de la cual las señales lidar son emitidas y retrodispersadas para ser detectadas por el sistema."@es,
    "The line along which lidar signals are emitted and backscattered to be detected by the system."@en,
    "激光雷达信号沿其发射和反射（以被系统识别）的路径。"@cn;
  skos:inScheme <http://vocab.ieawindtask32.org/wind-lidar-ontology/>;
  skos:prefLabel "Line of sight"@en, "Linea di visuale"@it, "Línea de visión"@es, "Sichtlinie"@de,
    "光束视线（视向线）"@cn .

ontolidar:LidarSampleRate a skos:Concept;
  rdfs:label "Hz"@en;
  skos:broader ontolidar:MeasurementPrinciples;
  skos:definition "Frecuencia de medición lidar. Número de muestras por segundo."@es,
    "Frequenza di campionamento. Numero di misurazioni al secondo."@it, "Sample rate frequency. Number of samples per second."@en,
    "采样率频率。每秒采样的样本数。"@cn;
  skos:inScheme <http://vocab.ieawindtask32.org/wind-lidar-ontology/>;
  skos:prefLabel "Frequenza di campionamento del lidar"@it, "Lidar sample rate"@en,
    "Lidar-Abtastrate"@de, "Tasa de muestreo lidar"@es, "激光雷达采样率"@cn .

ontolidar:VerticalSlice a skos:Concept;
  skos:altLabel "RHI"@en, "Range-height indicator"@en;
  skos:broader ontolidar:VariableElevationScan;
  skos:definition "Geometría de medida en la que el haz realiza un barrido en sentido vertical variando el ángulo de elevación pero no el ángulo de azimut. Estos barridos también se conocen como RHI (del inglés, range-high-indicator). Esta geometría de escaneo puede utilizarse para observar los detalles del flujo en la superficie de la sección transversal muestreada por el escaneo."@es,
    "Scans can be made where the beam is swept through a vertical slice by varying the elevation angle but not the azimuth angle. These scans are also known as range-height-indicator (RHI) scans. This scan geometry may be used to look at details in the flow in the cross-sectional surface sampled by the scan."@en,
    "Una geometria di misurazione dove il fascio laser è mosso verticalmente variando solo l'angolo di elevazione ma non l'angolo azimutale. Questo tipo di scansioni sono anche note come scansioni RHI - range-height-indicator. E' comune utilizzare questo tipo di scansioni per osservare dettagli nel flusso nella sezione trasversa al piano di scansione."@it,
    "通过改变仰角而非方位角，可以在光束扫过垂直切面的情况下进行扫描。这些扫描也称为范围高度指示器 (RHI) 扫描。该种扫描方式可用于观察采样横截面中的流场详细信息"@cn;
  skos:inScheme <http://vocab.ieawindtask32.org/wind-lidar-ontology/>;
  skos:prefLabel "Geometria a taglio verticale"@it, "Geometría de corte vertical"@es,
    "Vertical slice"@en, "Vertikale Scheibe"@de, "垂直切面扫描法"@cn .

ontolidar:SequentialScan a skos:Concept;
  skos:broader ontolidar:CompoundScan;
  skos:definition "En un barrido secuencial, se ejecutan escaneos simples y/o compuestos, uno tras otro, realizados por el mismo dispositivo para revelar las características del flujo."@es,
    "In a sequential scan, simple and/or compound scans are executed one after another by the same device to reveal flow characteristics."@en,
    "In una scansione sequenziale, scansioni semplici e/o combinate, sono eseguite in sequenza una dopo l'altra per ricostruire le caratteristiche del flusso ventoso."@it,
    "在顺序扫描中，由同一个设备依次执行简单和/或复合扫描，以捕捉流场特性。"@cn;
  skos:editorialNote "La tassonomia della geometria di scansione è basata sulla figura 3 di NREL/TP-5000-64634 https://www.nrel.gov/docs/fy16osti/64634.pdf"@it,
    "La taxonomía de la geometría de escaneo se basa en la Figura 3 en NREL/TP-5000-64634 https://www.nrel.gov/docs/fy16osti/64634.pdf"@es,
    "The scanning geometry taxonomy is based on Figure 3 in NREL/TP-5000-64634 https://www.nrel.gov/docs/fy16osti/64634.pdf"@en;
  skos:inScheme <http://vocab.ieawindtask32.org/wind-lidar-ontology/>;
  skos:prefLabel "Escaneo secuencial"@es, "Scansione sequenziale"@it, "Sequential scan"@en,
    "Sequenzieller Scan"@de, "顺序扫描扫描法"@cn .

ontolidar:ConvergentScan a skos:Concept;
  skos:altLabel "Convergent beam"@en, "convergent-beam lidar"@en;
  skos:broader ontolidar:MultiLidar;
  skos:definition "A measurement configuration involving multiple lidar units which are operated in a coordinated and synchronised manner so that their beams converge and intersect at a succession of probe volumes. If three or more lidar units are used, it is possible to characterise the wind velocity vector in the probe volume where the beams intersect within the limitations prescribed by the probe length, sampling interval, and scan geometry."@en,
    "Una configuración de medición que incluye múltiples unidades lidar que funcionan de forma coordinada y sincronizada para que sus haces converjan y se crucen en una sucesión de volúmenes de muestreo. Si se utilizan tres o más unidades lidar, es posible caracterizar el vector de la velocidad del viento en el volumen de muestreo donde se cruzan los haces, dentro de las limitaciones prescritas por la longitud del muestreo, el intervalo de muestreo y la geometría de escaneo."@es,
    "Una configurazione di misurazione che coinvolge più unità lidar operate in un modo coordinato e sincronizzato in modo tale che i loro fasci convergano e si intersechino in specifici punti dello spazio. Se sono utilizzate tre o più unità lidar, è possibile ricostruire integralmente il vettore velocità del vento nelle aree dove i fasci laser si intersecano, fatto salvi i limiti definiti dalla lunghezza dell'area sensivile, l'intervallo di campionamento e la geometria di misurazione."@it,
    "一种涉及多个激光雷达单元的测量配置，这些单元以协调和同步的方式运行，使其光束在连续的探测体积中汇聚并相交。如果使用三个或更多激光雷达单元，则可以在探测体长度、采样间隔和扫描规定的空间内表征光束相交处的探测体积中的风速矢量。"@cn;
  skos:inScheme <http://vocab.ieawindtask32.org/wind-lidar-ontology/>;
  skos:prefLabel "Convergent scan"@en, "Escaneo convergente"@es, "Konvergente Suche"@de,
    "Scansione convergente"@it, "聚合扫描"@cn .

ontolidar:Parameters a skos:Concept;
  skos:definition "Parámetros específicos del lidar de viento."@es, "Specifici parametri del lidar."@it,
    "Wind lidar-specific parameters."@en, "Wind-Lidar spezifische Parameter."@de, "测风激光雷达特定参数。"@cn;
  skos:inScheme <http://vocab.ieawindtask32.org/wind-lidar-ontology/>;
  skos:narrower ontolidar:CarrierToNoiseRatio, ontolidar:SignalToNoiseRatio;
  skos:prefLabel "Parameter"@de, "Parameters"@en, "Parametri"@it, "Parámetros"@es, "参数"@cn;
  skos:topConceptOf <http://vocab.ieawindtask32.org/wind-lidar-ontology/> .

ontolidar:CarrierToNoiseRatio a skos:Concept;
  skos:altLabel "CNR"@en;
  skos:broader ontolidar:Parameters;
  skos:definition "En una señal modulada (ej. pulsada), cociente entre la potencia de la señal y la potencia del ruido de esa señal."@es,
    "In a modulated signal (i.e. the pulse), the carrier to noise ratio is the ratio of the signal power to the signal noise power."@en,
    "Una misura della forza del segnale di ritorno al lidar."@it, "在调制信号中，载波噪声比是信号功率与信号噪声功率的比值。"@cn;
  skos:editorialNote "A measure of lidar return signal quality. Is the signal to noise ratio of the modulated signal sent to probe the atmosphere and defines the lidar data availability. If CNR is below a certain threshold the information carried by the backscattered (modulated) light is discarded. Often used interchangably with SNR."@en,
    "Spesso usato in modo interscambiabile con SNR"@it, "Una medida de la calidad de la señal de retorno del lidar. Es la relación señal/ruido de la señal modulada enviada para sondear la atmósfera y define la disponibilidad de los datos lidar. Si el CNR está por debajo de un determinado umbral, la información transportada por la luz retrodispersada (modulada) se descarta. A menudo se utiliza de forma intercambiable con SNR."@es;
  skos:inScheme <http://vocab.ieawindtask32.org/wind-lidar-ontology/>;
  skos:prefLabel "Carrier to noise ratio"@en, "Rapporto portante-rumore"@it, "Relación portadora-ruido"@es,
    "载噪比"@cn .

ontolidar:SignalToNoiseRatio a skos:Concept;
  skos:altLabel "SNR"@en;
  skos:broader ontolidar:Parameters;
  skos:definition "SNR es el cociente entre la potencia de la señal y la potencia del ruido de esa señal."@es,
    "The ratio of signal power to signal noise power before modulation."@en, "Una misura della forza del segnale di ritorno al lidar."@it,
    "信号功率与信号噪声功率之比。"@cn;
  skos:editorialNote "A menudo se usa de forma intercambiable con CNR."@es, "Often used interchangably with CNR."@en,
    "Spesso usato in modo interscambiabile con CNR"@it;
  skos:inScheme <http://vocab.ieawindtask32.org/wind-lidar-ontology/>;
  skos:prefLabel "Rapporto segnale-rumore"@it, "Relación señal-ruido"@es, "Signal to noise ratio"@en,
    "Signal-Rausch-Verhältnis"@de, "信噪比"@cn .

ontolidar:DataFormats a skos:Concept;
  skos:definition "Format of the lidar data file. It is generally common across products from the same lidar manufacturer."@en,
    "Formatierung der Lidardaten. Diese ist normalerweise identisch bei Produkten vom gleichen Hersteller."@de,
    "Formato de datos lidar. Esto suele ser común para todo tipo de lidares desarrollados por un mismo fabricante."@es,
    "Formato del file dati prodotto dal lidar. Questo è tipicamente comune per tutti i tipi di lidars prodotti dallo stesso costruttore."@it,
    "激光雷达数据文件的格式。一般来说，它在同一激光雷达制造商的产品中是通用的。"@cn;
  skos:inScheme <http://vocab.ieawindtask32.org/wind-lidar-ontology/>;
  skos:narrower ontolidar:EWindlidar, ontolidar:HaloPhotonics, ontolidar:Leosphere,
    ontolidar:Zx;
  skos:prefLabel "Data formats"@en, "Datenformate"@de, "Formato dei dati"@it, "数据格式"@cn;
  skos:topConceptOf <http://vocab.ieawindtask32.org/wind-lidar-ontology/> .

ontolidar:Leosphere a skos:Concept;
  skos:broader ontolidar:DataFormats;
  skos:definition "Common data format for the products of the company Leosphere."@en,
    "Formato dati comune per i prodotti dell'azienda Leosphere."@it, "Formato de datos común para productos de la compañía Leosphere."@es,
    "Leosphere公司产品的通用数据格式。"@cn, "Übliches Datenformat für Produkte des Herstellers Leosphere."@de;
  skos:inScheme <http://vocab.ieawindtask32.org/wind-lidar-ontology/>;
  skos:prefLabel "Leosphere"@cn, "Leosphere"@de, "Leosphere"@en, "Leosphere"@it .

ontolidar:Zx a skos:Concept;
  skos:broader ontolidar:DataFormats;
  skos:definition "Common data format for the products of the company ZX lidars (.zph extension)."@en,
    "Formato dati comune per i prodotti dell'azienda ZX lidars (estensione .zph)."@it,
    "Formato de datos común para productos de la compañía Leosphere."@es, "ZX激光雷达公司产品的通用数据格式（.zph扩展）。"@cn,
    "Übliches Datenformat für Produkte des Herstellers ZX lidars (.zph Dateiendung)."@de;
  skos:inScheme <http://vocab.ieawindtask32.org/wind-lidar-ontology/>;
  skos:prefLabel "ZX"@cn, "ZX"@de, "ZX"@en, "ZX"@it .

ontolidar:HaloPhotonics a skos:Concept;
  skos:broader ontolidar:DataFormats;
  skos:definition "Common data format for the products of the company Halo photonics."@en,
    "Formato dati comune per i prodotti dell'azienda Halo photonics."@it, "Formato de datos común para productos de la compañía Halo photonics."@es,
    "Halo photonics公司产品的通用数据格式。"@cn, "Übliches Datenformat für Produkte des Herstellers Halo photonics."@de;
  skos:inScheme <http://vocab.ieawindtask32.org/wind-lidar-ontology/>;
  skos:narrower ontolidar:Streamline, ontolidar:Verticalpro, ontolidar:Windpro;
  skos:prefLabel "Halo photonics"@cn, "Halo photonics"@en, "Halo photonics"@it, "Halo-Photonik"@de .

ontolidar:EWindlidar a skos:Concept;
  skos:broader ontolidar:DataFormats;
  skos:definition "An attempt to standardize wind lidar data formats and making them to follow the FAIR principle (Findable, Accessible, Interoperable, Reusable)."@en,
    "Intento de estandarización de los datos de los lidares de viento construidos según el principio FAIR (datos al alcance (Findable), accesibles (Accesible), interoperables (Interoperable) y reproducibles (reproducible))."@es,
    "Un tentativo di standardizzare il formato dati dei lidar e di costruirlo secondo i principi FAIR (dati ricercabili, accessibili, interoperabili e riutilizzabili)."@it,
    "Wind Lidar Daten-Standard der das FAIR-Prinzip befolgt."@de, "测风雷达数据的一种标准化格式，并使其遵循FAIR（Findable, Accessible, Interoperable, Reusable）原则。"@cn;
  skos:editorialNote "https://zenodo.org/record/2478051/files/e_WindLidar.pdf?download=1"@en,
    "https://zenodo.org/record/2478051/files/e_WindLidar.pdf?download=1"@es, "https://zenodo.org/record/2478051/files/e_WindLidar.pdf?download=1"@it;
  skos:inScheme <http://vocab.ieawindtask32.org/wind-lidar-ontology/>;
  skos:prefLabel "e-windLidar"@cn, "e-windLidar"@de, "e-windLidar"@en, "e-windLidar"@it .

ontolidar:DataCommunication a skos:Concept;
  skos:definition "数据通信"@cn;
  skos:inScheme <http://vocab.ieawindtask32.org/wind-lidar-ontology/>;
  skos:narrower ontolidar:DataAveragingPeriod, ontolidar:DataTransferFrequency, ontolidar:FileGranulity,
    ontolidar:FtpDataTransfer, ontolidar:Lan, ontolidar:LoggingFrequency, ontolidar:NtpTimeSynchronisation,
    ontolidar:SamplingFrequency, ontolidar:UserInterface, ontolidar:Wifi;
  skos:prefLabel "Comunicazione dati"@it, "Data communication"@en, "Datenübertragung"@de,
    "数据通信"@cn;
  skos:topConceptOf <http://vocab.ieawindtask32.org/wind-lidar-ontology/> .

ontolidar:NtpTimeSynchronisation a skos:Concept;
  ontolidar:units "milliseconds"@en;
  skos:broader ontolidar:DataCommunication;
  skos:definition "A networking protocol for clock synchronization between computer systems and Lidar computer over packet-switched, variable-latency data networks. The maximum difference in the clock times between systems."@en,
    "Das Netzwerk-Protokoll für Uhrzeit-Synchronisation zwischen Lidar und Rechner ist NTP."@de,
    "Un protocollo di rete per la sincronizzazione dei compute e del lidar."@it, "Un protocolo de red para la sincronización del reloj entre los sistemas informáticos y el ordenador del lidar a través de redes de datos con conmutación de paquetes y latencia variable. Corresponde a la diferencia máxima en los tiempos de reloj entre los sistemas."@es,
    "一种网络协议，用于通过分组交换、可变延迟的数据网络实现计算机系统和激光雷达计算机之间的时钟同步。"@cn;
  skos:inScheme <http://vocab.ieawindtask32.org/wind-lidar-ontology/>;
  skos:prefLabel "NTP time synchronisation"@en, "NTP-Zeitsynchronisation"@de, "NTP时间同步"@cn,
    "Sincronizzazione temporale NTP"@it .

ontolidar:FtpDataTransfer a skos:Concept;
  ontolidar:units "text"@en;
  skos:broader ontolidar:DataCommunication;
  skos:definition "Das Datenübertragungs-Protokoll ist FTP."@de, "Data transfer protocol based on FTP."@en,
    "Protocollo di trasferimento dati basato sul sistema FTP."@it, "Protocolo de transferencia de datos basado en FTP."@es,
    "基于FTP的数据传输协议"@cn;
  skos:inScheme <http://vocab.ieawindtask32.org/wind-lidar-ontology/>;
  skos:prefLabel "FTP data transfer"@en, "FTP-Datenübertragung"@de, "FTP数据传输"@cn, "Trasferimento dati FTP"@it .

ontolidar:UserInterface a skos:Concept;
  ontolidar:units "text"@en;
  skos:broader ontolidar:DataCommunication;
  skos:definition "A graphical user interface implemented for Lidar data at Lidar end or at user end."@en,
    "Die grafische Benutzeroberfläche zu den Lidar-Daten auf Seiten des Lidar oder des Endnutzers."@de,
    "Interfaccia grafica per la visualizzazione e l'interpretazione dei dati lidar."@it,
    "Interfaz gráfica de usuario implementada para los datos lidar en el extremo del lidar o en el extremo del usuario."@es,
    "用户和激光雷达交互的图形界面"@cn;
  skos:inScheme <http://vocab.ieawindtask32.org/wind-lidar-ontology/>;
  skos:prefLabel "Benutzeroberfläche"@de, "Interfaccia utente"@it, "User interface"@en,
    "用户界面"@cn .

ontolidar:Wifi a skos:Concept;
  ontolidar:units "text"@en;
  skos:broader ontolidar:DataCommunication;
  skos:definition "Data transfer over WLAN protocol."@en, "Datenübertragung mittels WLAN Protokoll."@de,
    "Protocollo di trasferimento dati basato sul sistema WLAN."@it, "Transferencia de datos a través del protocolo WLAN."@es,
    "通过WLAN协议的数据传输"@cn;
  skos:inScheme <http://vocab.ieawindtask32.org/wind-lidar-ontology/>;
  skos:prefLabel "WIFI"@cn, "WIFI"@en, "Wi-Fi"@de, "Wi-Fi"@it .

ontolidar:Lan a skos:Concept;
  ontolidar:units "text"@en;
  skos:broader ontolidar:DataCommunication;
  skos:definition "Data transfer over LAN protocol."@en, "Datenübertragung mittels LAN Protokoll."@de,
    "Protocollo di trasferimento dati basato sul sistema LAN."@it, "Transferencia de datos a través del protocolo LAN."@es,
    "通过局域网协议的数据传输"@cn;
  skos:inScheme <http://vocab.ieawindtask32.org/wind-lidar-ontology/>;
  skos:prefLabel "LAN"@de, "LAN"@en, "LAN"@it, "局域网"@cn .

ontolidar:SamplingFrequency a skos:Concept;
  ontolidar:units "Hz"@en;
  skos:broader ontolidar:DataCommunication;
  skos:definition "Frecuencia máxima de muestreo del dispositivo de medición lidar."@es,
    "Frequenza massima di campionamento dei dati di un lidar."@it, "Maximale Abtastfrequenz des Lidar-Messgerätes."@de,
    "Maximum sampling frequency of the Lidar measurement device."@en, "激光雷达的最大采样频率"@cn;
  skos:inScheme <http://vocab.ieawindtask32.org/wind-lidar-ontology/>;
  skos:prefLabel "Abtastfrequenz"@de, "Frequenza di campionamento"@it, "Sampling frequency"@en,
    "采样频率"@cn .

ontolidar:LoggingFrequency a skos:Concept;
  ontolidar:units "Hz"@en;
  skos:broader ontolidar:DataCommunication;
  skos:definition "Frecuencia máxima de registro del dispositivo de medición lidar."@es,
    "Frequenza massima di scrittura dei logs di un lidar."@it, "Maximale Aufzeichnungsfrequenz des Lidar-Messgerätes."@de,
    "Maximum logging frequency of the logger or the Lidar measurement device."@en, "记录器或激光雷达的最大记录频率"@cn;
  skos:inScheme <http://vocab.ieawindtask32.org/wind-lidar-ontology/>;
  skos:prefLabel "Frequenza di registrazione"@it, "Häufigkeit der Protokollierung"@de,
    "Logging frequency"@en, "记录频率"@cn .

ontolidar:FileGranulity a skos:Concept;
  ontolidar:units "samples"@en;
  skos:broader ontolidar:DataCommunication;
  skos:definition "Die Größe der von Dateien abgedeckten Zeitintervalle der Messung, z.B. 10-min oder 1-h Dateien."@de,
    "El tamaño del archivo en términos de período de tiempo o muestras, por ejemplo, archivos de 10 minutos o archivos de 1 hora."@es,
    "Intervallo temporale coperto da dei dati contenuti in un file dati."@it, "The size of the file in terms of time period or samples e.g. 10-min files or 1 hour files."@en,
    "以时间或采样单位来表示的文件大小，例如，10分钟文件或1小时文件"@cn;
  skos:inScheme <http://vocab.ieawindtask32.org/wind-lidar-ontology/>;
  skos:prefLabel "File granulity"@en, "Granularita' del file"@it, "Granularität der Datei"@de,
    "文件颗粒度"@cn .

ontolidar:DataTransferFrequency a skos:Concept;
  ontolidar:units "Hz"@en;
  skos:broader ontolidar:DataCommunication;
  skos:definition "Die Frequenz der Datenübertragung zwischen Messgerät (Primär) und Sekundär-Geräten."@de,
    "Frequenza di trasferimento dati da un sistema di misurazione (principale) ad uno secondario."@it,
    "La frecuencia con la que se transfieren los datos entre el dispositivo de medición (primario) y un dispositivo secundario."@es,
    "The frequency at which data is transferred between the measurement device (primary) and a secondary device."@en,
    "测量设备（主设备）和辅助设备之间传输数据的频率"@cn;
  skos:inScheme <http://vocab.ieawindtask32.org/wind-lidar-ontology/>;
  skos:prefLabel "Data transfer frequency"@en, "Frequenza di trasferimento dati"@it,
    "Häufigkeit der Datenübertragung"@de, "数据传输频率"@cn .

ontolidar:DataAveragingPeriod a skos:Concept;
  ontolidar:units "seconds"@en;
  skos:broader ontolidar:DataCommunication;
  skos:definition "Data averaging period for the data, e.g., 20 Hz data can be averaged to 10 min data."@en,
    "Die Mittelungszeit der Daten, z.B. für 20 Hz gemittelt als 10 min Daten."@de, "Periodo de promediación de los datos, por ejemplo, los datos de 20 Hz se pueden promediar a datos de 10 minutos."@es,
    "Periodo temporale di media delle misurazioni grezze."@it, "计算均值所设定的周期，例如，用20赫兹的数据计算出10分钟平均的数据，10分钟就是数据均值周期"@cn;
  skos:inScheme <http://vocab.ieawindtask32.org/wind-lidar-ontology/>;
  skos:prefLabel "Data averaging period"@en, "Durata del periodo di media"@it, "Zeitraum der Datenmittelung"@de,
    "数据均值周期"@cn .

ontolidar:Installation a skos:Concept;
  skos:definition "Data, luogo e posizione della installazione di un lidar."@it, "Datum, Uhrzeit und Ort des Aufbaus"@de,
    "Fecha y hora de instalación, ubicación (gps)."@es, "Installation date and time, location (gps)."@en,
    "安装日期和时间，位置（gps）"@cn;
  skos:inScheme <http://vocab.ieawindtask32.org/wind-lidar-ontology/>;
  skos:narrower ontolidar:Decommission, ontolidar:Deployment, ontolidar:Relocation,
    ontolidar:Repair;
  skos:prefLabel "Installation"@de, "Installation"@en, "Installazione"@it, "安装"@cn;
  skos:topConceptOf <http://vocab.ieawindtask32.org/wind-lidar-ontology/> .

ontolidar:Deployment a skos:Concept;
  ontolidar:units "DateTime, GPS coordinates"@en;
  skos:broader ontolidar:Installation;
  skos:definition "Data, luogo e posizione della messa in opera di un lidar."@it, "Datum, Uhrzeit und Ort der Bereitstellung"@de,
    "Deployment date and time, location (gps)."@en, "Fecha y hora de instalación, ubicación (gps)."@es,
    "部署日期和时间，位置（gps）"@cn;
  skos:inScheme <http://vocab.ieawindtask32.org/wind-lidar-ontology/>;
  skos:prefLabel "Deployment"@en, "Einsatz"@de, "Messa in opera"@it, "部署"@cn .

ontolidar:Repair a skos:Concept;
  ontolidar:units "DateTime, GPS coordinates"@en;
  skos:broader ontolidar:Installation;
  skos:definition "Data, luogo e posizione della riparazione di un lidar."@it, "Datum, Uhrzeit und Ort der Reparatur"@de,
    "Fecha y hora de reparación, ubicación (gps)."@es, "Repair date and time, location (gps)."@en,
    "维修日期和时间，位置（gps）"@cn;
  skos:inScheme <http://vocab.ieawindtask32.org/wind-lidar-ontology/>;
  skos:prefLabel "Repair"@en, "Reparieren"@de, "Riparazione"@it, "修复"@cn .

ontolidar:Relocation a skos:Concept;
  ontolidar:units "DateTime, GPS coordinates"@en;
  skos:broader ontolidar:Installation;
  skos:definition "Data, luogo e posizione di una nuova messa in opera di un lidar."@it,
    "Datum, Uhrzeit und Ort des neuen Standortes"@de, "Fecha de la reubicación y hora, ubicación (gps)."@es,
    "Relocation date and time, location (gps)."@en, "搬迁日期和时间，地点（gps）"@cn;
  skos:inScheme <http://vocab.ieawindtask32.org/wind-lidar-ontology/>;
  skos:prefLabel "Relocation"@en, "Rilocalizzazione"@it, "Standortwechsel"@de, "搬迁"@cn .

ontolidar:Decommission a skos:Concept;
  ontolidar:units "DateTime, GPS coordinates"@en;
  skos:broader ontolidar:Installation;
  skos:definition "Data, luogo e posizione di una rimozione di un lidar."@it, "Datos y hora de desmantelamiento, ubicación (gps)."@es,
    "Datum, Uhrzeit und Ort der Stilllegung"@de, "Decommission date and time, location (gps)."@en,
    "退役日期和时间，地点(gps)"@cn;
  skos:inScheme <http://vocab.ieawindtask32.org/wind-lidar-ontology/>;
  skos:prefLabel "Decommission"@en, "Ritiro"@it, "Stilllegung"@de, "退役"@cn .

ontolidar:PhotoDetector skos:narrower ontolidar:PhotodetectorActiveArea, ontolidar:PhotodetectorGain,
    ontolidar:PhotodetectorSnr, ontolidar:PhotodetectorVoltageNoise .

ontolidar:UninterruptiblePowerSupply skos:narrower ontolidar:UpsBatteryCapacity, ontolidar:UpsBatteryIntensity,
    ontolidar:UpsBatteryPower, ontolidar:UpsBatteryVoltage .

ontolidar:MoveLaser skos:narrower ontolidar:MolasB300, ontolidar:MolasNl .

ontolidar:Galion skos:narrower ontolidar:GalionScanningLidarG4000 .

<http://vocab.ieawindtask32.org/wind-lidar-ontology/Emmiter/ReceiverConfiguration>
  skos:narrower ontolidar:Bistatic, ontolidar:Monostatic .

ontolidar:Configuration skos:narrower ontolidar:Heterodyne, ontolidar:Homodyne .
